@prefix : <http://ontology.causeex.com/ontology/odps/CauseEffect#> .
@prefix causal: <http://ontology.causeex.com/ontology/odps/CauseEffect#> .
@prefix dcterms: <http://purl.org/dc/terms/> .
@prefix event: <http://ontology.causeex.com/ontology/odps/Event#> .
@prefix owl: <http://www.w3.org/2002/07/owl#> .
@prefix rdf: <http://www.w3.org/1999/02/22-rdf-syntax-ns#> .
@prefix rdfs: <http://www.w3.org/2000/01/rdf-schema#> .
@prefix xml: <http://www.w3.org/XML/1998/namespace> .
@prefix xsd: <http://www.w3.org/2001/XMLSchema#> .

<http://ontology.causeex.com/ontology/odps/CauseEffect> rdf:type owl:Ontology ;
    dcterms:description "Ontology defining various causal relationships (cause-effect, catalyst for effect, preventative for effect, ...), as well as the ability to define 'no effect'."@en ;
    dcterms:created "January 28, 2017"^^xsd:string ;
    dcterms:modified "November 16, 2018"^^xsd:string ;
    rdfs:comment """November 16th 2018 revisions:
                    Added has_no_effect.
                  October 28th 2018 revisions:
                    Corrected the domain of references_event, and the domain and text of latency and strength.
                    Added the regex pattern for latency.
                    Corrected causal: prefix definition, and added UnionOfEventQualifiedEvent blank node.
                    Corrected is_similar to have a domain of SimilarAssertion and range of Event.
                    Added QualifiedEvent and changed the domain of the latency and strength properties to reference it.
                    Added the references_event property (between QualifiedEvent and the actual Event).
                    Changed the has_catalyst/cause/migigating_factor/precondition/preventative properties' ranges to 
                      reference either Event or QualifiedEvent.
                    Updated CausalAssertion and SimilarAssertion to reference the GeneralConcepts ontology.
                  May 16th 2018 revisions:
                    Added the strength and latency properties.
                  April 16th revisions:
                    Added the SimilarAssertion and is_similar object property.
                  Jan 29th revisions:
                    Added has_mitigating_factor.
                    Correctly referenced CausalAssertion (versus CausalExplanation) in the object properties."""@en ;
    owl:imports <http://ontology.causeex.com/ontology/odps/Event> ;
    owl:imports <http://purl.org/dc/terms> ;
    owl:versionInfo "Version 1.3"^^xsd:string .


#################################################################
#    Object Properties
#################################################################

:has_catalyst a owl:ObjectProperty ;
    rdfs:label "has catalyst"@en ;
    rdfs:comment "Property indicating that the referenced Event (occurrence, factor, etc.) or QualifiedEvent increases the intensity of the 'effect' Event, but is not a 'cause' of the 'effect'."@en; 
    rdfs:domain :CausalAssertion ;
    rdfs:range _:UnionOfEventQualifiedEvent .

:has_cause a owl:ObjectProperty ;
    rdfs:label "has cause"@en ;
    rdfs:comment "Property indicating that the referenced Event (occurrence, factor, etc.) or QualifiedEvent is needed for the 'effect' Event to happen."@en ;
    rdfs:domain :CausalAssertion ;
    rdfs:range _:UnionOfEventQualifiedEvent .

:has_effect a owl:ObjectProperty ;
    rdfs:label "has effect"@en ;
    rdfs:comment "Property indicating that the referenced Event (occurrence, factor, etc.) will 'happen' if the 'cause' Event(s) occur, and if the 'preventative' Event(s) do not occur or are not too significant."@en ; 
    rdfs:domain :CausalAssertion ;
    rdfs:range event:Event .

:has_mitigating_factor a owl:ObjectProperty ;
    rdfs:label "has mitigating factor"@en ;
    rdfs:comment "Property indicating that the referenced Event (occurrence, factor, etc.) or QualifiedEvent decreases the intensity of the 'effect' Event, but is not a 'cause'/'preventative' of the 'effect'."@en; 
    rdfs:domain :CausalAssertion ;
    rdfs:range _:UnionOfEventQualifiedEvent .

:has_no_effect a owl:ObjectProperty ;
    rdfs:label "has no effect"@en ;
    rdfs:comment "Property indicating that the referenced Event (occurrence, factor, etc.) is not affected by/is not vulnerable to/is not caused by the 'cause' Event(s)."@en ; 
    rdfs:domain :CausalAssertion ;
    rdfs:range event:Event .

:has_precondition a owl:ObjectProperty ;
    rdfs:label "has precondition"@en ;
    rdfs:comment "Property indicating that the referenced Event (occurrence, factor, etc.) or QualifiedEvent must have occurred/begun for the 'effect' Event to happen."@en; 
    rdfs:domain :CausalAssertion ;
    rdfs:range _:UnionOfEventQualifiedEvent .

:has_preventative a owl:ObjectProperty ;
    rdfs:label "has preventative"@en ;
    rdfs:comment "Property indicating that the referenced Event (occurrence, factor, etc.) or QualifiedEvent will stop, prevent or reduce the intensity of the 'effect' Event."@en; 
    rdfs:domain :CausalAssertion ;
    rdfs:range _:UnionOfEventQualifiedEvent .

:is_similar a owl:ObjectProperty, owl:IrreflexiveProperty, owl:TransitiveProperty ;
    rdfs:label "is similar"@en ;
    rdfs:comment "Property indicating that the referenced Event (occurrence, factor, etc.) is inferred to be comparable to other Events identified in the same SimilarAssertion entity. This might occur if the same Event is reported from different sources."@en ; 
    rdfs:domain :SimilarAssertion ;
    rdfs:range event:Event .

:references_event a owl:ObjectProperty, owl:FunctionalProperty ;
    rdfs:label "references event"@en ;
    rdfs:comment "Property defining the actual Event 'behind' a reified QualifiedEvent. The reification is needed in order to define the latency and/or strength of the Event relative to the CausalAssertion's 'effect'."@en ; 
    rdfs:domain :QualifiedEvent ;
    rdfs:range event:Event .


#################################################################
#    Datatype Properties
#################################################################

:latency a owl:DatatypeProperty, owl:FunctionalProperty ;
    rdfs:label "latency of the cause/catalyst/... on the effect"@en ;
    rdfs:comment "A string indicating the time lag between a cause/catalyst/preventative/... Event and its influence on the effect Event. The value must end with either 'ms' (milliseconds), 's' (seconds), 'm' (minutes), 'h' (hours), 'd' (days) or 'y' (years). The property's domain is (typically) a QualifiedEvent that is identified as the cause/catalyst/..., and which in turn, points to the actual Event using the references_event property. However, in cases where the CausalAssertion has only a single cause/catalyst/precondition/... and a single effect, then the latency property can be directly added to the CausalAssertion individual (reification is not needed)."@en ;
    rdfs:domain [ a owl:Class ;
                 owl:unionOf ( :CausalAssertion :QualifiedEvent ) ] ;
    rdfs:range [ a rdfs:Datatype ;
                 owl:onDatatype xsd:string ;
                 owl:withRestrictions ( [ xsd:pattern "^[0-9]+(ms|s|m|h|d|y)$" ] ) ] .

:strength a owl:DatatypeProperty, owl:FunctionalProperty ;
    rdfs:label "strength of the influence of the cause/catalyst/... on the effect"@en ;
    rdfs:comment "A decimal value indicating the degree to which the cause/catalyst/preventative/... Event influences the effect Event. The value must be in the range of 0.00-1.00, where 0.0 indicates no effect and 1.0 indicates a very strong correlation. The property's domain is (typically) a QualifiedEvent that is identified as the cause/catalyst/..., and which in turn, points to the actual Event using the references_event property. However, in cases where the CausalAssertion has only a single cause/catalyst/precondition/... and a single effect, then the strength property can be directly added to the CausalAssertion individual (reification is not needed)."@en ;
    rdfs:comment "To map a qualitative strength level (such as weak-medium-strong) to the  0.00-1.00 scale, it is recommended that the following values are used: 'no influence' = 0.00, 'very weak influence' = 0.10, 'very weak to weak influence' = 0.20, 'weak influence' = 0.3, 'weak to medium influence' = 0.40, 'medium influence' = 0.50, 'medium to strong influence' = 0.60, 'strong influence' = 0.70, 'strong to very strong influence' = 0.8, 'very strong influence' = 0.90, and 'complete influence' = 1.0."@en ;
    rdfs:domain [ a owl:Class ;
                 owl:unionOf ( :CausalAssertion :QualifiedEvent ) ] ;
    rdfs:range [ a rdfs:Datatype ;
                 owl:onDatatype xsd:decimal ;
                 owl:withRestrictions ( [ owl:minInclusive "0.00"^^xsd:decimal ]
                                        [ owl:maxInclusive "1.00"^^xsd:decimal ] ) ] .


#################################################################
#    Classes
#################################################################

:CausalAssertion a owl:Class ;
    rdfs:label "Causal Assertion"@en ;
    rdfs:comment "A class that relates one or more causal Events to one or more resulting Events, where the individual events are related using the 'cause' and 'effect' properties. The 'effect' Event may be prevented or enhanced by any related 'preventative' or 'catalyst' Events. In addition, 'precondition' Events may also be defined. The confidence in the relationship of 'cause' to 'effect' is defined using the General Concepts ontology's numeric_confidence datatype property."@en .

:QualifiedEvent a owl:Class ;
    rdfs:label "Qualified Event"@en ;
    rdfs:comment "A reification of event:Event. It is needed in order to define the latency and/or strength of the Event relative to the CausalAssertion's 'effect'. The Event that is reified is identified using the references_event property."@en .

:SimilarAssertion a owl:Class ;
    rdfs:label "Similar Assertion"@en ;
    rdfs:comment "A class that relates one or more Events (related using the is_similar object property), indicating that the Events are alike/comparable and may produce similar causes/effects. The confidence in the relationship of 'similarity' is defined using the General Concepts ontology's numeric_confidence datatype property."@en .

_:UnionOfEventQualifiedEvent a owl:Class ;
    owl:unionOf ( event:Event :QualifiedEvent ) .
