@prefix : <http://ontology.causeex.com/ontology/odps/DataProvenance#> .
@prefix actor: <http://ontology.causeex.com/ontology/odps/Actor#> .
@prefix cco: <http://www.ontologyrepository.com/CommonCoreOntologies/> .
@prefix data-prov: <http://ontology.causeex.com/ontology/odps/DataProvenance#> .
@prefix dcterms: <http://purl.org/dc/terms/> .
@prefix doco: <http://purl.org/spar/doco/> .
@prefix event: <http://ontology.causeex.com/ontology/odps/Event#> .
# @prefix prov: <http://www.w3.org/ns/prov#> .
@prefix owl: <http://www.w3.org/2002/07/owl#> .
@prefix rdf: <http://www.w3.org/1999/02/22-rdf-syntax-ns#> .
@prefix rdfs: <http://www.w3.org/2000/01/rdf-schema#> .
@prefix xsd: <http://www.w3.org/2001/XMLSchema#> .

<http://ontology.causeex.com/ontology/odps/DataProvenance> rdf:type owl:Ontology ;
    dcterms:description "Ontology simplifying the W3C Data Provenance ontology for the Causal Exploration program."@en ;
    dcterms:created "December 18, 2017"^^xsd:string ;
    dcterms:modified "February 5, 2019"^^xsd:string ;
    rdfs:comment """February 5th 2019 revisions:
                    Adjusted the modified date.
                    Corrected the regex for date_created and date_modified.
                  January 22nd 2019 revisions:
                    Added time_generated and the rdfs:range definition for event:communicated_in.
                    Added the software_or_algorithm property. Clarified Activity. Removed the ExtractionPipeline enumeration as it is
                      not needed/implied.
                    Added import of the Actor ontology to allow references to the Actor and Organization classes. Deprecated Organization
                      since its semantics align with actor:Organization and this gives more flexibility.
                    Removed individual definitions for Organization since these are too restrictive.
                    Moved description to the GeneralConcepts ontology.
                  December 19th 2018 revisions:
                    Updated the comment/description for date_created.
                  October 27th 2018 revisions:
                    Corrected regex pattern for data_created/modified.
                    Added the UserInput class, and the trigger_words, pronoun_mention, proper_name_mention and common_noun_mention 
                      datatype properties (preparing to deprecate MentionSpan, MentionTabularReference, MentionType and has_mention_type). 
                    Modified the sourced_from property's range to include UserInput.
                    Commented out references to prov: and dcterms: classes and properties that are only used in equivalencies and 
                      sub-class or sub-property declarations. 
                    Reduced the prefixes and imports to those that are explicitly referenced.
                    Removed ontology history older than 6 months.
                  September 24th 2018 revisions:
                    Added FunctionalProperty to time_retrieved.
                    Changed xsd:long to the more generic xsd:integer.
                    Added Seed to the domain list for author. Changed all rdfs:Literals to xsd:string.
                    Changed the text of the description/comment for time_completed.
                  August 3rd 2018 revisions:
                    Moved the equivalentClass definition for Document to the EventArtifact ontology (to avoid cyclic imports).
                  July 29th 2018 revisions:
                    Added the seed_type and citation datatype properties. 
                    Modified the definition of generated_by to add the range of Organization, which modifies the semantic from
                      that defined by W3C prov, wasGeneratedBy.
                    Added owl:FunctionalProperty to several properties, and updated the comments of several entities.
                  June 11th 2018 revisions:
                    Added a domain to text_value.
                    Added classes and properties to capture seed information so that it is queriable in the ontology store. 
                    Added text to the Worksheet class to describe how to identify the sheet (via its rdfs:label).
                    Added the property, online_source, and updated the comments for original_source and time_retrieved.
                  April 16th 2018 revisions:
                    Added the Worksheet class. Removed the fabio prefix since it is not used.
                    Modified the domain of time_completed to be any activity."""@en ;
#   owl:imports <http://www.ontologyrepository.com/CommonCoreOntologies/Mid/AllCoreOntology>;
    owl:imports <http://www.ontologyrepository.com/CommonCoreOntologies/Mid/ArtifactOntology> ;
    owl:imports <http://purl.org/dc/terms>;
    owl:imports <http://purl.org/spar/doco>;
    owl:imports <http://ontology.causeex.com/ontology/odps/Event> ;
#   owl:imports <http://www.w3.org/ns/prov>;
    owl:versionInfo "Version 2.5"^^xsd:string .


#################################################################
#    Object Properties
#################################################################

:contains a owl:ObjectProperty, owl:IrreflexiveProperty, owl:TransitiveProperty ;
    rdfs:label "contains"@en ;
    rdfs:comment "Defines the structural components of a Document. Document and DocumentComponents may in turn be broken down into more discrete entities. For example, a Document may 'contain' another Document (such as a SpreadSheet or Figure) or may 'contain' various Sections and Appendices. And the Sections may themselves 'contain' lower-level sub-sections, figures, spreadsheet tables, etc. Alternately, a Document/DocumentComponent may be broken down by specific Spans or TabularReferences."@en ;
    rdfs:domain _:UnionOfDocDocComp ;
    rdfs:range _:UnionOfDocDocComp .
#   rdfs:subPropertyOf dcterms:hasPart .

:generated_by a owl:ObjectProperty ;
    rdfs:label "generated by"@en ;
    rdfs:comment "Indicates the Actor that created the referenced individual, or the specific Activity by which an individual statement was constructed/derived. An individual may be 'generated by' a combination of different activities/algorithms."@en ;
    rdfs:range [ a owl:Class ;
                 owl:unionOf (:Activity event:Actor) ] .

:has_document_type a owl:ObjectProperty, owl:FunctionalProperty ;
    rdfs:label "has document type"@en ;
    rdfs:comment "Indicates that the referenced Document/DocumentComponent is 'Structured' (for example, a spreadsheet) or 'Unstructured' (e.g., free-form text)."@en ;
    rdfs:domain _:UnionOfDocDocComp ;
    rdfs:range :DocumentType .

:has_mention_type a owl:ObjectProperty, owl:FunctionalProperty ;
    rdfs:label "has mention type (deprecated)"@en ;
    rdfs:comment "Indicates that the referenced MentionSpan/MentionReference identifies an entity/thing and indicates its part of speech - a proper name (NAM), a pronoun (PRO) or a common noun or nominal (NOM)."@en ;
    rdfs:domain [ a owl:Class ;
                  owl:unionOf (:MentionSpan :MentionTabularReference) ] ;
    rdfs:range :MentionType .

:inferred_from a owl:ObjectProperty ;
    rdfs:label "inferred from"@en ;
    rdfs:comment "Indicates that the individual was deduced from the referenced Document/DocumentCompomnent, but was not specifically stated. For example, if text indicates that '50 protesters were injured' in an Event, then it is clear that there was an individual of type, event:DemonstrationOrProtest, that preceded the injury Event."@en ;
    rdfs:range _:UnionOfDocDocComp .

:performed_by a owl:ObjectProperty ;
    rdfs:label "performed by"@en ;
    rdfs:comment "Indicates an Organization which performed (or collaborated to perform) an Activity."@en ;
    rdfs:domain :Activity ;
    rdfs:range event:Actor .
#   rdfs:subPropertyOf prov:wasAssociatedWith .

:sourced_from a owl:ObjectProperty ;
    rdfs:label "sourced from"@en ;
    rdfs:comment "Indicates the most specific Document/DocumentCompomnent or UserInput details from which an individual or triple was constructed/derived. For example, an individual may be 'sourced from' a specific sentence in a specific section of a document, or from multiple offsets across several documents."@en ;
    rdfs:range [ a owl:Class ;
                 owl:unionOf ( :Document :DocumentComponent :UserInput ) ] .
#   rdfs:subPropertyOf prov:hadPrimarySource, dcterms:source .

event:communicated_in rdfs:range [ a owl:Class ;
                                   owl:unionOf (data-prov:Document data-prov:DocumentComponent) ] .


#################################################################
#    Data Properties
#################################################################

:author a owl:DatatypeProperty ; 
    rdfs:label "author"@en ;
    rdfs:comment "The name of an originator (a person or organizational unit) of a Document or one of its components. More than one author may be defined for a Document/DocumentComponent."@en ;
    rdfs:domain [ a owl:Class ;
        owl:unionOf ( :Document :DocumentComponent :Seed ) ] ;
    rdfs:range xsd:string .

:char_length a owl:DatatypeProperty, owl:FunctionalProperty ;
    rdfs:label "character length"@en ;
    rdfs:comment "An xsd:integer indicating the length of text (the number of characters), starting at the char_offset in a Document/DocumentComponent, from which a concept is extracted. Although usually applied to unstructured Documents/DocumentComponents, this property may also apply to structured ones. For example, it can be used to specify the total number of characters considered (starting from the char_offset) in a CSV file."@en ;
    rdfs:domain :Span ;
    rdfs:range xsd:integer .

:char_offset a owl:DatatypeProperty, owl:FunctionalProperty ;
    rdfs:label "character offset"@en ;
    rdfs:comment "An xsd:integer indicating the character offset in a Document/DocumentComponent where a concept is extracted. Although usually applied to unstructured Documents/DocumentComponents, this property may also apply to structured ones. For example, it can be used to specify a character offset into a CSV file."@en ;
    rdfs:comment "An offset is always calculated from the beginning of the document/file."@en ;
    rdfs:domain :Span ;
    rdfs:range xsd:integer .

:citation a owl:DatatypeProperty ;
    rdfs:label "citation"@en ;
    rdfs:comment "A reference to another Document or DocumentComponent that provided the detail behind or source of some information."@en ; 
    rdfs:domain _:UnionOfDocDocComp ;
    rdfs:range xsd:string .

:classification a owl:DatatypeProperty, owl:FunctionalProperty ;
    rdfs:label "classification"@en ;
    rdfs:comment "The classification of a Document/DocumentComponent or individual statement. Although defined as a string, in an implementation, the value will be checked against a controlled vocabulary. For example, for the US Government, the classification levels are UNCLASSIFIED, FOR OFFICIAL USE ONLY, RESTRICTED, CONFIDENTIAL, SECRET or TOP SECRET."@en ;
    rdfs:range xsd:string .

:column_ref a owl:DatatypeProperty, owl:FunctionalProperty ;
    rdfs:label "column reference"@en ;
    rdfs:comment "A string indicating the column in a TabularReference. Typically, both a column_ref and a line_number define the document location where a concept is extracted from a structured document/component (i.e., a spreadsheet). However, the same text_value may be listed tens or hundreds of times in a specific column. In that case, it may be beneficial/expedient to simply list the column_ref without a line_number."@en ;
    rdfs:comment "The value of column_ref is a string since the column may be defined by name, by a spreadsheet column reference (such as 'AA'), or by a numeric value."@en ;
    rdfs:comment"Note that the use of a column_ref is not restricted to structured documents. It may also be applicable to a 'Table' in an unstructured document."@en ;
    rdfs:domain :TabularReference ;
    rdfs:range xsd:string .

:common_noun_mention a owl:DatatypeProperty, owl:FunctionalProperty ;
    rdfs:label "common noun mention"@en ;
    rdfs:comment "The specific common noun (or nominal) in a Span or TabularReference that resulted in a particular actor, event, location, relationship, etc. being defined."@en ;
    rdfs:domain _:UnionOfSpanTabularReference ;
    rdfs:range xsd:string .

:contributor a owl:DatatypeProperty ;
    rdfs:label "contributor"@en ;
    rdfs:comment "The name of an entity (a person or organizational unit) that provided input to, or writing for, a Document or one of its components. More than one contributor may be defined for a Document or its components."@en ;
    rdfs:domain _:UnionOfDocDocComp ;
    rdfs:range xsd:string .

:date_created a owl:DatatypeProperty, owl:FunctionalProperty ;
    rdfs:label "date created"@en ;
    rdfs:comment "String defining the date when the Document/DocumentComponent came into existence. The value must conform to one of the formats, yyyy-mm-dd, yyyy-mm or yyyy. This restriction will be validated using a constraint."@en ;
    rdfs:domain _:UnionOfDocDocComp ;
    rdfs:range [ a rdfs:Datatype ;
                 owl:onDatatype xsd:string ;
                 owl:withRestrictions ( [ xsd:pattern "^[0-9]{4}(\\-(0[1-9]|1[012])(\\-(0[1-9]|[12][0-9]|3[01]))?)?$" ] ) ] .
#   rdfs:subPropertyOf dcterms:created .

:date_modified a owl:DatatypeProperty ;
    rdfs:label "date modified"@en ;
    rdfs:comment "String defining the date when an individual was modified. An individual may be modified more than once. The value must conform to one of the formats, yyyy-mm-dd, yyyy-mm or yyyy. This restriction will be validated using a constraint."@en ;
    rdfs:domain _:UnionOfDocDocComp ;
    rdfs:range [ a rdfs:Datatype ;
                 owl:onDatatype xsd:string ;
                 owl:withRestrictions ( [ xsd:pattern "^[0-9]{4}(\\-(0[1-9]|1[012])(\\-(0[1-9]|[12][0-9]|3[01]))?)?$" ] ) ] .
#   rdfs:subPropertyOf dcterms:modified .

:keyword a owl:DatatypeProperty ;
    rdfs:label "keyword"@en ;
    rdfs:comment "A word indicating the subject matter, time frame and/or topic of a Document or one of its components. More than one keyword may be related to a Document or its components."@en ;
    rdfs:domain _:UnionOfDocDocComp ;
    rdfs:range xsd:string .

:language a owl:DatatypeProperty ;
    rdfs:label "language"@en ;
    rdfs:comment "The language in which a Document or one of its component is written. This string should be set to one of the values defined in RFC 5646. It will be checked against the 'language' values recorded in the IANA Registry (located at http://www.iana.org/assignments/language-subtag-registry/language-subtag-registry). Note that more than one language may be declared for a Document or its components."@en ;
    rdfs:domain _:UnionOfDocDocComp ;
    rdfs:range xsd:string .

:line_number a owl:DatatypeProperty, owl:FunctionalProperty ;
    rdfs:label "line or row number"@en ;
    rdfs:comment "An xsd:integer indicating the line/row number in a TabularReference where a concept is extracted. Typically, this property is applied to a structured document/component (i.e., a spreadsheet), although it may be applied to a 'Table' in an unstructured document."@en ;
    rdfs:domain :TabularReference ;
    rdfs:range xsd:integer .

:local_source a owl:DatatypeProperty, owl:FunctionalProperty ;
    rdfs:label "local source file name/path"@en ;
    rdfs:comment "The name of the 'local system' file that holds the Document/DocumentComponent. Note that this information is provided for the mapping teams' usage. For example, it can be used to capture when a web page was last retrieved/crawled or to remove all individuals that were extracted from a page if an updated web page is provided. There is no need for commonality in the local_source values across the teams. Note also that a team is not required to use this property. It would not be needed for DocumentComponents that are NOT separate files from their containing Documents (for example, sections in a Word document). If the local file is saved from, or is a copy of a document from another location, that information can be specified using the original_source property and the retrieved_at timestamp property."@en ;
    rdfs:domain _:UnionOfDocDocComp ;
    rdfs:range xsd:string .

:online_source a owl:DatatypeProperty, owl:FunctionalProperty ;
    rdfs:label "online source"@en ;
    rdfs:comment "The URL of a Document/DocumentComponent retrieved from the web. If a file is only retrieved from the web (and not stored in any local document repository), the original_source and the online_source properties have the same values. Also, the time_retrieved property is required."@en ;
    rdfs:comment "Note that a source document may be retained in a document repository, but also have an online location. If so, define the original_source property as its repository location and use this property, online_source, to supply its online location."@en ;
    rdfs:domain _:UnionOfDocDocComp ;
    rdfs:range xsd:string .

:original_source a owl:DatatypeProperty, owl:FunctionalProperty ;
    rdfs:label "original source"@en ;
    rdfs:comment "The full path name/location of the source file representing the Document/DocumentComponent. This should be the file location and name as retained in a document repository, or the URL if the document was obtained directly from the web. Note that this information is not needed for DocumentComponents that are NOT separate files from their containing Documents (for example, sections in a Word document)."@en ;
    rdfs:comment "If a file is in a document repository, but can also be obtained from an online location, define the original_source property as its repository location and use the property, online_source, to supply its online location."@en ;
    rdfs:comment "If a file is only retrieved from the web, the original_source and the online_source properties have the same values. And, the time_retrieved property is also required."@en ;
    rdfs:domain _:UnionOfDocDocComp ;
    rdfs:range xsd:string .

:pronoun_mention a owl:DatatypeProperty, owl:FunctionalProperty ;
    rdfs:label "pronoun mention"@en ;
    rdfs:comment "The specific pronoun in a Span or TabularReference that resulted in a particular actor, event, location, relationship, etc. being defined."@en ;
    rdfs:domain _:UnionOfSpanTabularReference ;
    rdfs:range xsd:string .

:proper_name_mention a owl:DatatypeProperty, owl:FunctionalProperty ;
    rdfs:label "proper name mention"@en ;
    rdfs:comment "The specific proper name in a Span or TabularReference that resulted in a particular actor, event, location, relationship, etc. being defined."@en ;
    rdfs:domain _:UnionOfSpanTabularReference ;
    rdfs:range xsd:string .

:publisher a owl:DatatypeProperty ;
    rdfs:label "publisher"@en ;
    rdfs:comment "The name of an entity (a person or organizational unit) that made a Document available. Typically, there is a single publisher, but this is not required."@en ;
    rdfs:domain :Document ;
    rdfs:range xsd:string .

:seed_milestone a owl:DatatypeProperty, owl:FunctionalProperty ;
    rdfs:label "seed milestone"@en ;
    rdfs:comment "String identifying the CauseEx milestone data which was used to generate the Seed individual - for example, 'm9'."@en ;
    rdfs:domain :Seed ;
    rdfs:range xsd:string .

:seed_type a owl:DatatypeProperty, owl:FunctionalProperty ;
    rdfs:label "seed type"@en ;
    rdfs:comment "String identifying the type of documents that were processed - for example, 'news', 'abstracts', 'structured' documents, etc."@en ;
    rdfs:domain :Seed ;
    rdfs:range xsd:string .

:seed_version a owl:DatatypeProperty, owl:FunctionalProperty ;
    rdfs:label "seed version"@en ;
    rdfs:comment "String identifying the version of the Seed individual within the CauseEx milestone - for example, 'v7'."@en ;
    rdfs:domain :Seed ;
    rdfs:range xsd:string .

:software_or_algorithm a owl:DatatypeProperty ;
    rdfs:label "software or algorithm"@en ;
    rdfs:comment "String identifying the specific software or algorithm used to generate some entity."@en ;
    rdfs:range xsd:string .

:text_value a owl:DatatypeProperty ;
    rdfs:label "text value"@en ;
    rdfs:comment "A string providing the text from which an Event, Actor, Location, ... individual was extracted."@en ;
    rdfs:domain :DocumentComponent ;
    rdfs:range xsd:string .

:time_completed a owl:DatatypeProperty, owl:FunctionalProperty ;
    rdfs:label "time completed"@en ;
    rdfs:comment "The date/time when an Activity finished."@en ;
    rdfs:domain :Activity ;
    rdfs:range xsd:dateTime .
#   rdfs:subPropertyOf prov:endedAtTime .

:time_generated a owl:DatatypeProperty, owl:FunctionalProperty ;
    rdfs:label "time generated"@en ;
    rdfs:comment "The date/time when a particular entity was generated/defined. This property could apply to any individual."@en ;
    rdfs:range xsd:dateTime .

:time_retrieved a owl:DatatypeProperty, owl:FunctionalProperty ;
    rdfs:label "time retrieved"@en ;
    rdfs:comment "The date/time when a particular document was accessed on the web or from the document repository. Typically, this property is only used with top-level Documents and not DocumentComponents. But, if a Document is separated into different files, and these may be modified/accessed/retrieved at different times, then the property is relevant for Components."@en ;
    rdfs:comment "Note that this property is required when retrieving a document from an online source."@en ;
    rdfs:domain _:UnionOfDocDocComp ;
    rdfs:range xsd:dateTime .

:title a owl:DatatypeProperty, owl:FunctionalProperty ;
    rdfs:label "title"@en ;
    rdfs:comment "A (distinguishing) name of a Document or one of its components."@en ;
    rdfs:domain _:UnionOfDocDocComp ;
    rdfs:range xsd:string .
#   rdfs:subPropertyOf dcterms:title .

:trigger_words a owl:DatatypeProperty, owl:FunctionalProperty ;
    rdfs:label "trigger words"@en ;
    rdfs:comment "The specific words in a Span or TabularReference that resulted in a particular actor, event, location, relationship, etc. to be defined."@en ;
    rdfs:domain _:UnionOfSpanTabularReference ;
    rdfs:range xsd:string .


#################################################################
#    Classes
#################################################################

:Activity a owl:Class ;
    rdfs:label "Activity"@en ;
    rdfs:comment "Something that is done which 'acts upon or with entities; it may include consuming, processing, transforming, modifying, relocating, using, or generating entities' (from W3C's PROV-O ontology)."@en .
#   rdfs:subClassOf prov:Activity .

:DataSet a owl:Class ;
    rdfs:label "Data Set"@en ;
    rdfs:comment "A collection of related information/data, published together. Examples include linked data sets, research data results, etc."@en ;
    rdfs:subClassOf cco:InformationBearingArtifact .

:Document a owl:Class ;
    rdfs:label "Document"@en ;
    rdfs:comment "A representation of the thinking of one or more persons or organizations, captured as text or diagrams, in the form of physical pieces of paper, an electronic file or a digital artifact (identified by a Uniform Resource Identifier (URI), and made accessible to a user by means of the Hypertext Transport Protocol, HTTP)."@en ;
    rdfs:subClassOf cco:InformationBearingArtifact ;
#   rdfs:subClassOf prov:Entity, dcterms:Text ;
    owl:disjointWith :DocumentComponent .

:DocumentComponent a owl:Class ;
    rdfs:label "Document Component"@en ;
    rdfs:comment "An identifiable portion of a Document. A Document 'contains' DocumentComponents."@en ;
    rdfs:subClassOf cco:InformationBearingArtifact ;
#   rdfs:subClassOf prov:Entity, dcterms:Text ;
    owl:equivalentClass [ a owl:Class ;
                          owl:unionOf ( doco:Abstract doco:Foreword doco:Preface doco:Afterword doco:Appendix doco:Chapter doco:Figure 
                                        doco:Footnote doco:Paragraph doco:Section doco:Sentence doco:Table doco:TextChunk ) ] .

:DocumentType a owl:Class ;
    rdfs:label "Document Type"@en ;
    rdfs:comment "An enumeration whose individuals indicate that a Document/DocumentComponent is Structured (such as a spreadsheet) or Unstructured (free-form text)."@en ;
    owl:equivalentClass [ a owl:Class ;
                          owl:oneOf ( :Structured :Unstructured ) ] .

:ExtractionActivity a owl:Class ;
    rdfs:label "Extraction Activity"@en ;
    rdfs:comment "The activity of consuming a source document and generating triples representing its information."@en ;
    rdfs:subClassOf :Activity .

:InferenceActivity a owl:Class ;
    rdfs:label "Inference Activity"@en ;
    rdfs:comment "The activity of inferring new information based on reasoning and evidence from one or more source documents."@en ;
    rdfs:subClassOf :Activity .

:MentionSpan a owl:Class ;
    rdfs:label "Mention Span (deprecated)"@en ;
    rdfs:comment "A portion of a Document, defined by a specific character offset and char_length, that specifically identifies an entity. Individuals of type, MentionSpan, have a related MentionType indicating whether the referenced text is a proper name (data-prov:NAM), a pronoun (data-prov:PRO) or a nominal/common noun (data-prov:NOM). The specific, identifying text is captured using the text_value property. For example, the text, 'Amnesty International (AI) published a report,' identifies an Organization named Amnesty International. The Organization would be 'sourced_from' a MentionSpan individual, and that individual would be defined with properties/values of: data-prov:text_value 'Amnesty International (AI)', data-prov:has_mention_type data-prov:NAM, and the data-prov:char_offset and char_length of the text_value. A subsequent reference to Amnesty International may simply use the pronoun, 'they'. This would be captured as another MentionSpan individual of with a MentionType of data-prov:PRO, and a text_value of 'they'."@en ;
    rdfs:subClassOf :Span .

:MentionTabularReference a owl:Class ;
    rdfs:label "Mention Tabular Reference (deprecated)"@en ;
    rdfs:comment "A portion of a structured Document/DocumentComponent or a table in an unstructured document/component, identified by a line/row number and/or a column reference, that specifically identifies an entity. Individuals of type, MentionTabularReference, have a related MentionType indicating whether the referenced text is a proper name (data-prov:NAM), a pronoun (data-prov:PRO) or a nominal/common noun (data-prov:NOM). The specific, identifying text is captured using the text_value property. For example, the text, 'Amnesty International (AI)' in a specific row and column in a spreadsheet identifies an Organization with the name, Amnesty International. The Organization would be 'sourced_from' a MentionTabularReference individual, and that individual would be defined with properties/values of: data-prov:text_value 'Amnesty International (AI)', data-prov:has_mention_type data-prov:NAM, and the appropriate data-prov:line_number and column_ref."@en ;
    rdfs:subClassOf :TabularReference .

:MentionType a owl:Class ;
    rdfs:label "Mention Type (deprecated)"@en ;
    rdfs:comment "An enumeration whose individuals indicate that a 'MentionSpan' is a proper name (NAM), a pronoun (PRO) or a common name/nominal (NOM)."@en ;
    owl:equivalentClass [ a owl:Class ;
                          owl:oneOf ( :NAM :NOM :PRO ) ] . 

:Organization a owl:Class ;
    rdfs:label "Organization (deprecated)"@en ;
    rdfs:comment "An entity responsible for publications or CauseEx extractions/inference. This is a more restricted definition of Organization than specified in the Actor ontology."@en .
#   rdfs:subClassOf actor:Organization .
#   rdfs:subClassOf prov:Organization .

:Seed a owl:Class ;
    rdfs:label "Seed"@en ;
    rdfs:comment "An entity representing and describing the set of triples provided by a CauseEx TA1 performer. A Seed individual has properties identifying its name (rdfs:label, a string), date/time generated (data-prov:time_completed, an xsd:dateTime), milestone and version information (data-prov:seed_milestone and seed_version, respectively, strings), the seed type (seed_type, for example, 'news' or 'abstracts'), citations and keywords for abstracts (data-prov:citation and keyword, respectively), and the TA1 performer/organization (data-prov:author, reference to 'bbn', 'isi' or 'lcc')."@en .

:Span a owl:Class ;
    rdfs:label "Span"@en ;
    rdfs:comment "An identifiable portion of a Document, defined by a specific character offset and char_length. Note that a char_offset property must be defined for a Span, which will be validated by constraint checking. A char_length may also be defined."@en ;
    rdfs:subClassOf :DocumentComponent ;
    owl:equivalentClass doco:TextChunk .

:TabularReference a owl:Class ;
    rdfs:label "Tabular Reference"@en ;
    rdfs:comment "A portion of a structured Document/DocumentComponent (such as a spreadsheet or CSV file) or a table in an unstructured document/component, identified by a line/row number and/or a column reference. Note that at least one of the properties, line_number or column_ref must be defined for a TabularReference, which will be validated by constraint checking."@en ;
    rdfs:subClassOf :DocumentComponent .

:UserInput a owl:Class ;
    rdfs:label "User Input"@en ;
    rdfs:comment "Identifies an individual user as the source of information. The individual would be referenced by the sourced_from property and could use the author and date_created properties to capture the user details."@en .

:Worksheet a owl:Class ;
    rdfs:label "Worksheet"@en ;
    rdfs:comment "A single page/spreadsheet in a structured document. If a structured document consists of a single page, then it is not necessary to identify a Worksheet. However, if a document includes multiple pages, then a Worksheet individual should be defined for each one, to uniquely identify it and scope its contents. The label/name of the worksheet page should be defined as the rdfs:label of the Worksheet individual."@en ;
    rdfs:subClassOf :DocumentComponent .

_:UnionOfDocDocComp a owl:Class ;
    owl:unionOf ( :Document :DocumentComponent ) .

_:UnionOfSpanTabularReference a owl:Class ;
    owl:unionOf ( :Span :TabularReference ) .

#################################################################
#    Individuals
#################################################################

:NAM a owl:NamedIndividual, :MentionType ;
    rdfs:label "Proper Name (deprecated)"@en .

:NOM a owl:NamedIndividual, :MentionType ;
    rdfs:label "Nominal/Common Noun (deprecated)"@en .

:PRO a owl:NamedIndividual, :MentionType ;
    rdfs:label "Pronoun (deprecated)"@en .

:Structured a owl:NamedIndividual, :DocumentType ;
    rdfs:label "Structured Document"@en .

:Unstructured a owl:NamedIndividual, :DocumentType ;
    rdfs:label "Unstructured Document"@en .

_:diff2 rdf:type owl:AllDifferent ; 
    owl:members ( :NAM :NOM :PRO :Structured :Unstructured) .
