@prefix : <http://ontology.causeex.com/ontology/odps/GeneralConcepts#> .
@prefix dcterms: <http://purl.org/dc/terms/> .
@prefix general: <http://ontology.causeex.com/ontology/odps/GeneralConcepts#> .
@prefix owl: <http://www.w3.org/2002/07/owl#> .
@prefix rdf: <http://www.w3.org/1999/02/22-rdf-syntax-ns#> .
@prefix rdfs: <http://www.w3.org/2000/01/rdf-schema#> .
@prefix xsd: <http://www.w3.org/2001/XMLSchema#> .

<http://ontology.causeex.com/ontology/odps/GeneralConcepts-Time> rdf:type owl:Ontology ;
    dcterms:description "Ontology defining time-related general concepts used in the Causal Exploration program."@en ;
    dcterms:created "January 7, 2019"^^xsd:string ;
    dcterms:modified "January 29, 2019"^^xsd:string ;
    rdfs:comment """January 29th 2019 revision:
                      Updated the import statememnt for GeneralConcepts to correct typo.
                      All changes prior to January 7th 2019 are documented in the GeneralConcepts ontology."""@en ;
    owl:imports <http://purl.org/dc/terms> ;
    owl:imports <http://ontology.causeex.com/ontology/odps/GeneralConcepts> ;
    owl:versionInfo "Version 1.1"^^xsd:string .


#################################################################
#    Object Properties
#################################################################

:has_day_of_week a owl:ObjectProperty ;
    rdfs:label "has day of week"@en ;
    rdfs:comment "Indicates a specific day of the week (Sunday, Monday, ..., Saturday) for a RecurrencePattern individual."@en ;
    rdfs:domain :RecurrencePattern ;
    rdfs:range :DayOfWeek .

:has_recurrence_interval a owl:ObjectProperty, owl:FunctionalProperty ;
    rdfs:label "has recurrence interval"@en ;
    rdfs:comment "Indicates a specific interval (minutes, hourly, daily, weekly, monthly or yearly) for a RecurrencePattern individual."@en ;
    rdfs:domain :RecurrencePattern ;
    rdfs:range :RecurrenceInterval .

:recurs a owl:ObjectProperty, owl:IrreflexiveProperty ;
    rdfs:label "recurs"@en ;
    rdfs:comment "Relates an individual, which may have earliest/latest_possible_start/end_time properties, with an instance of RecurrencePattern. The latter refines the definition of time from anything between the earliest and latest times, to a specific pattern within that timeframe. The pattern is based on a closed enumeration identifying either minutes, hourly, daily, weekly, monthly or yearly recurrence (indicated by the RecurrenceInterval), further constrained by the has_day_of_week, beginning/ending_month_and_day, beginning/ending_hour_and_minute, day/week_of_month, and/or separation_interval properties."@en ;
    rdfs:range :RecurrencePattern .


#################################################################
#    Data Properties
#################################################################

:beginning_hour_and_minute a owl:DatatypeProperty, owl:FunctionalProperty ;
    rdfs:label "beginning hour and minute"@en ;
    rdfs:comment "String defining the 2 digit hour and 2 digit minute (within a day) that is the beginning of a RecurrencePattern interval. The value must conform to the format, hh:mm, and use a 24 hour clock. This restriction will be validated using a constraint."@en ;
    rdfs:domain :RecurrencePattern ;
    rdfs:range [ a rdfs:Datatype ;
                 owl:onDatatype xsd:string ;
                 owl:withRestrictions ( [ xsd:pattern "^([01][0-9]|2[0123]):[0-5][0-9]$" ] ) ] .

:beginning_month_and_day a owl:DatatypeProperty, owl:FunctionalProperty ;
    rdfs:label "beginning month and day"@en ;
    rdfs:comment "String defining the 2 digit month and 2 digit day (within a year) that is the beginning of a RecurrencePattern interval. The value must conform to the format, mm-dd. This restriction will be validated using a constraint."@en ;
    rdfs:domain :RecurrencePattern ;
    rdfs:range [ a rdfs:Datatype ;
                 owl:onDatatype xsd:string ;
                 owl:withRestrictions ( [ xsd:pattern "^(0[1-9]|1[012])\\-(0[1-9]|[12][0-9]|3[01])$" ] ) ] .

:day_of_month a owl:DatatypeProperty ;
    rdfs:label "day_of_month"@en ;
    rdfs:comment "day_of_month indicates occurrences that happen on a particular day of the month. For example, workers may be paid on the 15th and the last day of a month. Those days can be indicated by declaring two day_of_month property values for a RecurrencePattern individual. The values would be set to 15 and -1 (where a positive number counts from the beginning of the month and a negative number counts back from the end)."@en ;
    rdfs:domain :RecurrencePattern ;
    rdfs:range xsd:integer .

:earliest_possible_end_time a owl:DatatypeProperty, owl:FunctionalProperty ;
    rdfs:label "earliest possible end time"@en ;
    rdfs:comment "A dateTime specifying the earliest end time of an individual."@en ;
    rdfs:range xsd:dateTime .

:earliest_possible_start_time a owl:DatatypeProperty, owl:FunctionalProperty ;
    rdfs:label "earliest possible start time"@en ;
    rdfs:comment "A dateTime specifying the earliest start time of an individual."@en ;
    rdfs:range xsd:dateTime .

:ending_hour_and_minute a owl:DatatypeProperty, owl:FunctionalProperty ;
    rdfs:label "ending hour and minute"@en ;
    rdfs:comment "String defining the 2 digit hour and 2 digit minute (within a day) that is the end bound of a RecurrencePattern interval. The value must conform to the format, hh:mm, and use a 24 hour clock. This restriction will be validated using a constraint."@en ;
    rdfs:domain :RecurrencePattern ;
    rdfs:range [ a rdfs:Datatype ;
                 owl:onDatatype xsd:string ;
                 owl:withRestrictions ( [ xsd:pattern "^([01][0-9]|2[0123]):[0-5][0-9]$" ] ) ] .

:ending_month_and_day a owl:DatatypeProperty, owl:FunctionalProperty ;
    rdfs:label "ending month and day"@en ;
    rdfs:comment "String defining the 2 digit month and 2 digit day (within a year) that is the end bound of a RecurrencePattern interval. The value must conform to the format, mm-dd. This restriction will be validated using a constraint."@en ;
    rdfs:domain :RecurrencePattern ;
    rdfs:range [ a rdfs:Datatype ;
                 owl:onDatatype xsd:string ;
                 owl:withRestrictions ( [ xsd:pattern "^(0[1-9]|1[012])\\-(0[1-9]|[12][0-9]|3[01])$" ] ) ] .

:latest_possible_end_time a owl:DatatypeProperty, owl:FunctionalProperty ;
    rdfs:label "latest possible end time"@en ;
    rdfs:comment "A dateTime specifying the latest end time of an individual."@en ;
    rdfs:range xsd:dateTime .

:latest_possible_start_time a owl:DatatypeProperty, owl:FunctionalProperty ;
    rdfs:label "latest possible start time"@en ;
    rdfs:comment "A dateTime specifying the latest start time of an individual."@en ;
    rdfs:range xsd:dateTime .

:longest_possible_duration_milliseconds a owl:DatatypeProperty, owl:FunctionalProperty ;
    rdfs:label "longest possible duration in milliseconds"@en ;
    rdfs:comment "An unsigned long specifying the longest time extent/duration of an individual."@en ;
    rdfs:range xsd:unsignedLong .

:separation_interval a owl:DatatypeProperty, owl:FunctionalProperty ;
    rdfs:label "separation interval"@en ;
    rdfs:comment "A decimal specifying the time between occurrences for a RecurrencePattern individual. This time is relative to the individual's RecurrenceInterval. For example, if the RecurrenceInterval is minutes, and the separation interval is 10, then something occurs/recurs every 10 minutes. If a separation_interval is not specified, then a value of 1 is assumed."@en ;
    rdfs:domain :RecurrencePattern ;
    rdfs:range xsd:decimal .

:shortest_possible_duration_milliseconds a owl:DatatypeProperty, owl:FunctionalProperty ;
    rdfs:label "shortest possible duration in milliseconds"@en ;
    rdfs:comment "An unsigned long specifying the shortest time extent/duration of an individual."@en ;
    rdfs:range xsd:unsignedLong .

:time a owl:DatatypeProperty ;
    rdfs:label "time "@en ;
    rdfs:comment "A string specifying a time or interval related to an individual. This is a different technique for defining time than using the earlist/lastest_possible_xxx properties. When parsing text, it may be valuable to simply capture the text related to the time (for example, a reference to the 'Elizabethan era' or to the 'time before the death of the president')."@en ;
    rdfs:range xsd:string .

:week_of_month a owl:DatatypeProperty ;
    rdfs:label "week_of_month"@en ;
    rdfs:comment "week_of_month indicates occurrences that happen in a particular week of the month. For example, a meeting may occur on the first and last Fridays of a month. That can be indicated by setting a RecurrencePattern individual's has_day_of_week to Friday and also declaring two week_of_month property values, 1 and -1 (where a positive number counts from the beginning of the month and a negative number counts back from the end)."@en ;
    rdfs:domain :RecurrencePattern ;
    rdfs:range xsd:integer .


#################################################################
#    Classes
#################################################################

:DayOfWeek a owl:Class ;
    rdfs:label "Day of Week"@en ;
    rdfs:comment "An enumeration indicating the day of week (Sunday, Monday, ..., Saturday). This class is used with a RecurrencePattern individual to indicate a pattern that involves a specific day of the week. That day is associated with the RecurrencePattern individual using the has_day_of_week property."@en ;
    owl:equivalentClass [ a owl:Class ;
                          owl:oneOf ( :Sunday :Monday :Tuesday :Wednesday :Thursday :Friday :Saturday ) ] .

:RecurrencePattern a owl:Class ;
    rdfs:label "Recurrence Pattern"@en ;
    rdfs:comment "Reifies information defining a recurring time interval. The recurrence pattern is based on a closed enumeration identifying either minutes, hourly, daily, weekly, monthly or yearly (indicated by the RecurrenceInterval), further constrained by the beginning/ending_month_and_day, beginning/ending_hour_and_minute, has_day_of_week, week/day_of_month and/or separation_interval properties."@en ;
    rdfs:comment "An example is to describe a recurring pattern of every other Saturday from June 1 to September 1, every year starting in 2016. This is defined by specifying an earliest_possible_start_time for an individual ('2016-06-01T00:00:00') and also associating (via the 'recurs' property) a RecurrencePattern instance whose RecurrenceInterval is weekly, separation_interval is 2 (e.g., 2 weeks between occurrences), day of week is Saturday, beginning_month_and_day is '06-01', and ending_month_and_day is '09-01'."@en ;
    rdfs:comment "Other examples are to define a recurring pattern of the first and last Friday of every month, or every year on Dec 25th. The first example is defined by creating a RecurrencePattern individual where the RecurrenceInterval is monthly, the day of week is Friday, and two week_of_month values are defined, 1 and -1 (negative indicates that the Friday is determined from the end of the month). The second example is defined by creating an individual where the RecurrenceInterval is yearly and the beginning/ending_month_and_day are '12-25'."@en ;
    rdfs:comment "A last example is to define a recurring pattern of every 15 minutes, from 8am to 5pm, Monday-Friday. This would be specified by creating a RecurrencePattern individual where the RecurrenceInterval is minutes, the beginning and ending hour and minute is 08:00 and 17:00 (respectively), the separation interval is 15, and 5 days of the week are referenced - Monday, Tuesday, Wednesday, Thursday and Friday."@en .

:RecurrenceInterval a owl:Class ;
    rdfs:label "Recurrence Interval"@en ;
    rdfs:comment "An enumeration indicating whether something occurs/recurs on an interval of Minutes, Hourly, Daily, Weekly, Monthly or Yearly. A RecurrenceInterval individual is associated with a RecurrencePattern instance using the has_recurrence_interval property."@en ;
    owl:equivalentClass [ a owl:Class ;
                          owl:oneOf ( :Minutes :Hourly :Daily :Weekly :Monthly :Yearly ) ] .


#################################################################
#    Individuals
#################################################################

:Daily a owl:NamedIndividual, :RecurrenceInterval ;
    rdfs:label "Daily"@en .

:Friday a owl:NamedIndividual, :DayOfWeek ;
    rdfs:label "Friday"@en .

:Hourly a owl:NamedIndividual, :RecurrenceInterval ;
    rdfs:label "Hourly"@en .

:Minutes a owl:NamedIndividual, :RecurrenceInterval ;
    rdfs:label "Minutes"@en .

:Monday a owl:NamedIndividual, :DayOfWeek ;
    rdfs:label "Monday"@en .

:Monthly a owl:NamedIndividual, :RecurrenceInterval ;
    rdfs:label "Monthly"@en .

:Saturday a owl:NamedIndividual, :DayOfWeek ;
    rdfs:label "Saturday"@en .

:Sunday a owl:NamedIndividual, :DayOfWeek ;
    rdfs:label "Sunday"@en .

:Thursday a owl:NamedIndividual, :DayOfWeek ;
    rdfs:label "Thursday"@en .

:Tuesday a owl:NamedIndividual, :DayOfWeek ;
    rdfs:label "Tuesday"@en .

:Wednesday a owl:NamedIndividual, :DayOfWeek ;
    rdfs:label "Wednesday"@en .

:Weekly a owl:NamedIndividual, :RecurrenceInterval ;
    rdfs:label "Weekly"@en .

:Yearly a owl:NamedIndividual, :RecurrenceInterval ;
    rdfs:label "Yearly"@en .

_:diff1 rdf:type owl:AllDifferent ; 
    owl:members ( :Minutes :Hourly :Daily :Weekly :Monthly :Yearly 
                  :Sunday :Monday :Tuesday :Wednesday :Thursday :Friday :Saturday ) .
