@prefix : <http://ontology.causeex.com/ontology/odps/Actor#> .
@prefix actor: <http://ontology.causeex.com/ontology/odps/Actor#> .
@prefix cco: <http://www.ontologyrepository.com/CommonCoreOntologies/> .
@prefix dcterms: <http://purl.org/dc/terms/> .
@prefix event: <http://ontology.causeex.com/ontology/odps/Event#> .
@prefix general: <http://ontology.causeex.com/ontology/odps/GeneralConcepts#> .
# @prefix oeceo: <http://www.ontologylibrary.mil/OperationalEnvironment/Mid/OECausalExplorationOntology#> .
# @prefix oeorg: <http://www.ontologylibrary.mil/OperationalEnvironment/Mid/OEOrganizationOntology#> .
@prefix oereligion: <http://www.ontologylibrary.mil/OperationalEnvironment/Mid/OEReligionOntology#> .
@prefix owl: <http://www.w3.org/2002/07/owl#> .
@prefix rdf: <http://www.w3.org/1999/02/22-rdf-syntax-ns#> .
@prefix rdfs: <http://www.w3.org/2000/01/rdf-schema#> .
@prefix xsd: <http://www.w3.org/2001/XMLSchema#> .

<http://ontology.causeex.com/ontology/odps/Actor-Hierarchy> rdf:type owl:Ontology ;
    dcterms:description "Ontology extending the event:Actor sub-classing hierarchy."@en ;
    dcterms:created "January 28, 2018"^^xsd:string ;
    dcterms:modified "May 13, 2019"^^xsd:string ;
    rdfs:comment """May 13th 2019 revisions:
                    Modified _:UnionOfPersonGroupOfPersons to be _:UnionOfPersonGroupOfPersons1, to be unique.
                    Added the classes, PartiallyRecognizedOrUnrecognizedGeopoliticalEntity and Air/Ground/NavalForce.
                    Corrected rdfs:label and :comment for 2 classes.
                    Modified all blank node sub-classes of PopulationOfConcern to use that class directly.
                  February 11th 2019 revisions:
                    Added the _:UnionOfPersonGroupOfPersons1 blank node to correct an error when importing the ontologies using Protege.
                  January 22nd 2019 revisions:
                    Separated the Actor ontology into two separate ontologies - Actor-ReificationsAndProperties and Actor-Hierarchy. 
                      This ontology is the latter.
                    Adjusted the imports based on the ontology separation.
                  November 13th 2018 revisions:
                    Added AdvocacyGroup and InterGovernmentalOrganization.
                  October 28th 2018 revisions:
                    Removed cco:Government since it is not a white-listed class. Added SupportSystemOrNetwork. 
                    Added that a GPE can include the concept of a Continent or Subcontinent as the group of their governments. 
                    Changed equivalent class to subClassOf for CCO GeopoliticalEntity, Continent/Subcontinent and Government.
                    Commented out references to cco:, oeceo: and oeorg: classes that are only used in equivalency declarations. 
                    Removed ontology history older than 6 months. 
                  September 17th 2018 revisions:
                    Corrected several descriptions/comments.
                  July 10th 2018 revisions:
                    Changed subclassing (where it was for documentation) involving CCO and OE classes, to a comment.
                  June 12th 2018 revisions:
                    Added/modified sub-classing to reduce false positives in constraint violations and better align with usage.
                    Added the class, EthnicGroup.
                  April 21st 2018 revisions:
                    Added the CyberSpecialist and Gender classes.
                    Subclassed cco:GPE from :Organization and general:PhysicalLocation to reduce the number of domain/range mismatches 
                      (without reasoning)."""@en ;
#   owl:imports <http://www.ontologyrepository.com/CommonCoreOntologies/Mid/AllCoreOntology> ;
    owl:imports <http://www.ontologyrepository.com/CommonCoreOntologies/Mid/GeospatialOntology> ;
#   owl:imports <http://www.ontologylibrary.mil/OperationalEnvironment/Mid/OEOntology> ;
    owl:imports <http://purl.org/dc/terms> ;
    owl:imports <http://ontology.causeex.com/ontology/odps/Event> ;
    owl:versionInfo "Version 1.93"^^xsd:string .

#################################################################
#    Sub-classes of event:Actor
#################################################################

:AdvocacyGroup a owl:Class ;
    rdfs:label "Advocacy Group"@en ;
    rdfs:comment "Advocacy groups attempt to influence public opinion and government policy. They are also known as pressure groups, lobby groups, campaign groups, interest groups, and special interest groups."@en ;
    rdfs:subClassOf :Organization .

:AgriculturalOrganization a owl:Class ;
    rdfs:label "Agricultural Organization"@en ;
    rdfs:comment "Organization dealing with growing crops and/or with agricultural issues"@en ;
    rdfs:subClassOf :Organization .
#   owl:equivalentClass oeorg:Agriculture.

:AidOrReliefOrganization a owl:Class ;
    rdfs:label "Aid or Relief Organization"@en ;
    rdfs:comment "Organization dealing with providing aid to people in need"@en ;
    rdfs:subClassOf :Organization .

:AirForce a owl:Class ;
    rdfs:label "Air Force"@en ;
    rdfs:subClassOf :MilitaryForce .

:Allies a owl:Class ;
    rdfs:label "Allies"@en ;
    rdfs:comment "Sub-class of GroupOfActors, indicating that the members of the Group are cooperating and/or united as regards a specific activity or goal."@en ;
    rdfs:subClassOf :GroupOfActors .

:Anti-Government a owl:Class ;
    rdfs:label "Anti-Government"@en ;
    rdfs:subClassOf event:Actor .

:ArmedForce a owl:Class ;
    rdfs:label "Armed Force"@en ;
    rdfs:subClassOf :Organization .
#   owl:equivalentClass cco:ArmedForce .

:AsylumSeekers a owl:Class ;
    rdfs:label "Asylum Seekers"@en ;
    rdfs:comment "Asylum seekers are people who leave their home country for another country, and apply for asylum in this other country. The act of moving to the new country can be defined as either a LocationChange or ForcedMove in the EventHierarchy ontology."@en ;
    rdfs:subClassOf :DisplacedPersons .

:BranchOfGovernment a owl:Class ;
    rdfs:label "Branch of Government"@en ;
    rdfs:subClassOf :Organization .

:CivilSocietyOrganization a owl:Class ;
    rdfs:label "Civil Society Organization (CSO)"@en ;
    rdfs:comment "A sub-class of Organization indicating that its members are working together in the interest of citizens. A Civil Society Organization (CSO) is distinct from government and business, and includes community-based organizations as well as non-governmental organizations (NGOs)."@en ;
    rdfs:subClassOf :Organization .
#   owl:equivalentClass cco:CivilOrganization .

:CommercialOrganization a owl:Class ;
    rdfs:label "Commerical Organization"@en ;
    rdfs:comment "An Organization 'with a particular skill set, strategy, resources, or priorities in place designed to turn a profit' (from http://www.businessdictionary.com/definition/commercial-organization.html)."@en ;
    rdfs:subClassOf :Organization .
#   owl:equivalentClass cco:CommercialOrganization, oeorg:Business .

:ConstructionOrganization a owl:Class ;
    rdfs:label "Construction Organization"@en ;
    rdfs:subClassOf :CommercialOrganization ;
    rdfs:comment "Organization concerned with building structures/infrastructures."@en .

:Crew a owl:Class ;
    rdfs:label "Crew"@en ;
    rdfs:comment "A GroupOfActors working together and assigned as a unit to perform a task. This is (logically) the super-class of cco:Crew since the latter is only related to operating a vehicle, while this class is defined more broadly."@en ;
    rdfs:subClassOf :GroupOfPersons .
# cco:Crew rdfs:subClassOf :Crew .

:CriminalOrganization a owl:Class ;
    rdfs:label "Criminal Organization"@en ;
    rdfs:subClassOf :Organization .
#   owl:equivalentClass oeorg:Criminal .

:CyberSpecialist a owl:Class ;
    rdfs:label "Cyber Specialist"@en ;
    rdfs:subClassOf :Person .

:DisplacedPersons a owl:Class ;
    rdfs:label "Displaced Person(s)"@en ;
    rdfs:comment "Displaced persons are any person or people forced to move from their home or home region. The act of displacement is defined as a LocationChange or ForcedMove in the EventHierarchy ontology."@en ;
    rdfs:subClassOf :PopulationOfConcern .

:EducationalOrganization a owl:Class ;
    rdfs:label "Educational Organization"@en ;
    rdfs:comment "An Organization supplying educational services. An EducationalOrganization's 'primary function is the presentation of formal instruction and it normally maintains a regular faculty and curriculum and normally has a regularly enrolled body of pupils or students in attendance' (https://www.law.cornell.edu/cfr/text/26/1.170A-9)."@en ;
    rdfs:subClassOf :Organization .
#   owl:equivalentClass cco:EducationalOrganization, oeorg:Education .

:Enemies a owl:Class ;
    rdfs:label "Enemies"@en ;
    rdfs:comment "Sub-class of GroupOfActors, indicating that the members of the Group are opposed to/hostile towards each other."@en ;
    rdfs:subClassOf :GroupOfActors .

:EntertainmentOrganization a owl:Class ;
    rdfs:label "Entertainment Organization"@en ;
    rdfs:subClassOf :CommercialOrganization ;
    rdfs:comment "Organization dealing with the creation, production or provision of music, movies, performances, podcasts, sports, exhibitions, etc."@en .

:EnvironmentalOrganization a owl:Class ;
    rdfs:label "Environmental Organization"@en ;
    rdfs:subClassOf :Organization ;
    rdfs:comment "Organization dealing with protecting the environment and/or concerned with environmental issues such as wildlife preservation or climate change"@en .
#   owl:equivalentClass oeorg:Environmental .

:EthnicGroup a owl:Class ;
    rdfs:label "Ethnic Group"@en ;
    rdfs:subClassOf :Populace ;
    rdfs:comment "Defines a Populace/GroupOfPersons all having the same ethnicity. If the ethnicity is known, it should be specified using the has_ethnicity property."@en .

:ExecutiveBranchOfGovernment a owl:Class ;
    rdfs:label "Executive Branch of Government"@en ;
    rdfs:subClassOf :BranchOfGovernment .
#   owl:equivalentClass oeorg:Executive .

:Family a owl:Class ;
    rdfs:label "Family"@en ;
    rdfs:subClassOf :GroupOfPersons .
#   owl:equivalentClass cco:Family .

:FinanceOrganization a owl:Class ;
    rdfs:label "Finance Organization"@en ;
    rdfs:subClassOf :CommercialOrganization ;
    rdfs:comment "Organization dealing with investments and financial issues"@en .

:ForestryOrganization a owl:Class ;
    rdfs:label "Forestry Organization"@en ;
    rdfs:subClassOf :Organization ;
    rdfs:comment "Organization dealing with growing or harvesting trees or with forestry issues"@en .

:GeopoliticalEntity a owl:Class ;
    rdfs:label "Geopolitical Entity"@en ;
    rdfs:comment "An Actor identified as a political structure governing a geographical area. It is defined as a sub-class of both Organization and general:PhysicalLocation, since there is ambiguity in speech acts and a tendency to reference a Country/City/... as synonymous with its government (with an implicit assumption made about its area, and that assumption can change over time as boundaries evolve)."@en ;
    rdfs:comment "cco:GeopoliticalEntity (and its sub-classes, cco:Country, cco:City, ..., cco:First/Second/...AdministrativeOrder), as well as cco:Continent/Subcontinent, can be used to further classify an actor:GeopoliticalEntity, indicating its geographical area."@en ;
    rdfs:subClassOf :Organization, general:PhysicalLocation .
cco:GeopoliticalEntity rdfs:subClassOf :GeopoliticalEntity .
cco:Continent rdfs:subClassOf :GeopoliticalEntity .
cco:Subcontinent rdfs:subClassOf :GeopoliticalEntity .

:GovernmentAgency a owl:Class ;
    rdfs:label "Government Agency"@en ;
    rdfs:subClassOf :Organization .
#   owl:equivalentClass cco:GovernmentAgency .

:GroundForce a owl:Class ;
    rdfs:label "Ground Force"@en ;
    rdfs:subClassOf :MilitaryForce .

:GroupOfActors a owl:Class ;
    rdfs:label "Group of Actors"@en ;
    rdfs:comment "A Collection of two or more Actors performing activities/working/living together and/or having similar beliefs, ways of life, etc. The members of the group are defined using the inherited has_member object property, defined in the GeneralConcepts ontology. A GroupOfActors is always assumed to have the plural property (from the GeneralConcepts ontology) set to true."@en ;
    rdfs:subClassOf event:Actor, general:Collection ; 
#   owl:equivalentClass cco:GroupOfAgents ;
    owl:equivalentClass [ a owl:Restriction ;
                          owl:onProperty general:has_member ;
                          owl:allValuesFrom event:Actor ] .

:GroupOfOrganizations a owl:Class ;
    rdfs:label "Group of Organizations"@en ;
    rdfs:subClassOf :GroupOfActors ;
#   owl:equivalentClass cco:GroupOfOrganizations ;
    owl:equivalentClass [ a owl:Restriction ;
                          owl:onProperty general:has_member ;
                          owl:allValuesFrom :Organization ] .

:GroupOfPersons a owl:Class ;
    rdfs:label "Group of Persons"@en ;
    rdfs:subClassOf :GroupOfActors ;
#   owl:equivalentClass cco:GroupOfPersons ;
    owl:equivalentClass [ a owl:Restriction ;
                          owl:onProperty general:has_member ;
                          owl:allValuesFrom _:UnionOfPersonGroupOfPersons1 ] .

:HealthcareOrganization a owl:Class ;
    rdfs:label "Healthcare Organization"@en ;
    rdfs:subClassOf :Organization ;
    rdfs:comment "Organization providing mental and/or physical health services and/or dealing with health issues"@en .
#   owl:equivalentClass oeorg:Health .

:Household a owl:Class ;
    rdfs:label "Household"@en ;
    rdfs:subClassOf :GroupOfPersons .

:HumanRightsOrganization a owl:Class ;
    rdfs:label "Human Rights Organization"@en ;
    rdfs:subClassOf :Organization ;
    rdfs:comment "Organization concerned with defining and/or documenting concerns regarding human rights"@en .
#   owl:equivalentClass oeorg:HumanRights .

:InterGovernmentalOrganization a owl:Class ;
    rdfs:label "Inter-Governmental Organization"@en ;
    rdfs:comment "Examples of InterGovernmentalOrganizations are the World Health Organization, the United Nations and the World Trade Organization."@en ;
    rdfs:subClassOf :Organization .

:InternallyDisplacedPersons a owl:Class ;
    rdfs:label "Internally Displaced Persons"@en ;
    rdfs:comment "Internally displaced persons are 'people who have been forced to leave their homes to escape armed conflict, violence, violations of human rights, or natural disasters, and who have not crossed an international border' (UNHCR definition). The act of relocating can be defined as a ForcedMove in the EventHierarchy ontology."@en ;
    rdfs:subClassOf :DisplacedPersons .

:JihadistOrganization a owl:Class ;
    rdfs:label "Jihadist Organization"@en ;
    rdfs:comment "A JihadistOrganization is a type of TerroristOrganization that supports the 'jihadist' movement."@en ;
    rdfs:subClassOf :TerroristOrganization .

:JudicialBranchOfGovernment a owl:Class ;
    rdfs:label "Judicial Branch of Government"@en ;
    rdfs:subClassOf :BranchOfGovernment .
#   owl:equivalentClass oeorg:Judiciary .

:LaborOrganization a owl:Class ;
    rdfs:label "Labor Organization"@en ;
    rdfs:subClassOf :Organization ;
    rdfs:comment "Organization that is a trade union or otherwise concerned with labor issues"@en .
#   owl:equivalentClass oeorg:Labor .

:LegalOrganization a owl:Class ;
    rdfs:label "Legal Organization"@en ;
    rdfs:subClassOf :CommercialOrganization ;
    rdfs:comment "Organization concerned with providing legal services such as businesses providing bail bonds, attorney services, etc."@en .

:LegislativeBranchOfGovernment a owl:Class ;
    rdfs:label "Legislative Branch of Government"@en ;
    rdfs:subClassOf :BranchOfGovernment .
#   owl:equivalentClass oeorg:Legislature .

:ManufacturingOrganization a owl:Class ;
    rdfs:label "Manufacturing Organization"@en ;
    rdfs:subClassOf :CommercialOrganization ;
    rdfs:comment "Organization concerned with the creation of goods for use or sale. The types of goods created are defined using the involves_goods_or_property predicate defined in the GeneralConcepts ontology."@en .

:MediaOrganization a owl:Class ;
    rdfs:label "Media Organization"@en ;
    rdfs:subClassOf :CommercialOrganization ;
    rdfs:comment "Organization dealing with the various forms of mass information dissemination such as newspapers, radio, cable television, etc."@en .
#   owl:equivalentClass oeorg:Media .

:MilitaryForce a owl:Class ;
    rdfs:label "Military Force"@en ;
    rdfs:subClassOf :ArmedForce .
#   owl:equivalentClass cco:MilitaryPersonnelForce .

:MiningOrDrillingOrganization a owl:Class ;
    rdfs:label "Mining or Drilling Organization"@en ;
    rdfs:subClassOf :CommercialOrganization ;
    rdfs:comment "Organization dealing with mining or drilling for resources or with related issues"@en .

:NavalForce a owl:Class ;
    rdfs:label "Naval Force"@en ;
    rdfs:subClassOf :MilitaryForce .

:NonGovernmentalOrganization a owl:Class ;
    rdfs:label "Non-Governmental Organization (NGO)"@en ;
    rdfs:comment "A sub-class of CivilSocietyOrganization. According to NGO.org (http://www.ngo.org/ngoinfo/define.html), 'NGOs perform a variety of service and humanitarian functions, bring citizen concerns to Governments, advocate and monitor policies and encourage political participation through provision of information.'"@en ;
    rdfs:subClassOf :CivilSocietyOrganization .

:Organization a owl:Class ;
    rdfs:label "Organization"@en ;
    rdfs:comment "Identifies an organized GroupOfActors with a particular purpose related to business, society, personal interests, etc."@en ;
    rdfs:subClassOf :GroupOfActors .
#   owl:equivalentClass cco:Organization .

:OrganizationalUnit a owl:Class ;
    rdfs:label "Organizational Unit"@en ;
    rdfs:subClassOf :Organization ;
    rdfs:comment "A work team or functional or business unit within an Organization. It is recommended that the parent Organization of an OrganizationalUnit be defined using the general:has_component property, where the appropriate triple is specified as Organization - general:has_component - OrganizationalUnit."@en .

:Refugees a owl:Class ;
    rdfs:label "Refugees"@en ;
    rdfs:comment "Refugees are displaced persons who has been forced to move to another country (from their home country). There is a formal, legal definition of the term given by the UNHCR as including 'individuals recognized under the 1951 Convention relating to the Status of Refugees; its 1967 Protocol; the 1969 OAU Convention Governing the Specific Aspects of Refugee Problems in Africa; those recognized in accordance with the UNHCR Statute; individuals granted complementary forms of protection; or, those enjoying temporary protection'. The act of moving to another country can be defined as a ForcedMove in the EventHierarchy ontology."@en ;
    rdfs:subClassOf :DisplacedPersons .

:ReturnedInternallyDisplacedPersons a owl:Class ;
    rdfs:label "Returned Internally Displaced Persons"@en ;
    rdfs:comment "Returned Internally Displaced Persons are former IDPs who have returned to their home/home region. The act of returning can be defined as a LocationChange in the EventHierarchy ontology. The return event can be linked to an earlier displacement event using the event:preceded_by object property."@en ;
    rdfs:subClassOf :Returnees .

:ReturnedRefugees a owl:Class ;
    rdfs:label "Returned Refugees"@en ;
    rdfs:comment "Returned refugees are 'former refugees who have returned to their country of origin spontaneously or with assistance but are yet to be fully integrated' (UNHCR definition). The act of returning can be defined as a LocationChange in the EventHierarchy ontology. The return event can be linked to an earlier displacement event using the event:preceded_by object property."@en ;
    rdfs:subClassOf :Returnees .

:Returnees a owl:Class ;
    rdfs:label "Returnee(s)"@en ;
    rdfs:comment "Returnees are formerly DisplacedPersons who have returned to their home/home region. The act of returning can be defined as a LocationChange in the EventHierarchy ontology. The return event can be linked to the earlier displacement/location change event using the event:preceded_by object property."@en ;
    rdfs:subClassOf :PopulationOfConcern .

:ParamilitaryForce a owl:Class ;
    rdfs:label "Paramilitary Force"@en ;
    rdfs:comment "Defined by Wikipedia as 'a semi-militarized force whose organizational structure, tactics, training, subculture, and (often) function are similar to those of a professional military, but which is not included as part of a state's formal armed forces'. Examples include militias, guerillas, the US's Federal Protective Forces, etc."@en ;
    rdfs:subClassOf :ArmedForce .
#   owl:equivalentClass cco:ParamilitaryForce .

:PartiallyRecognizedOrUnrecognizedGeopoliticalEntity a owl:Class ;
    rdfs:label "Partially Recognized or Unrecognized Geopolitical Entity"@en ;
    rdfs:comment "Is a geopolitical entity that is claiming/had claimed governmental authority over some land area and wants/wanted recognition as a sovereign country. If in the past, the entity was acknowledged by some other recognized country."@en ;
    rdfs:subClassOf :GeopoliticalEntity .

:Person a owl:Class ;
    rdfs:label "Person"@en ;
    rdfs:comment "Identifies a human being."@en ;
    rdfs:subClassOf event:Actor .
#   owl:equivalentClass cco:Person .

:PoliceForce a owl:Class ;
    rdfs:label "Police Force"@en ;
    rdfs:subClassOf :ArmedForce .
#   owl:equivalentClass oeorg:Police .

:PoliticalParty a owl:Class ;
    rdfs:label "Political Party"@en ;
    rdfs:subClassOf :Organization .

:Populace a owl:Class ;
    rdfs:label "Populace"@en ;
    rdfs:comment "A Populace is a GroupOfPersons living in a particular PhysicalLocation. The location is defined using the GeneralConcepts ontology's property, located_at. Note that a Populace individual is always assumed to have the 'plural' property (from the GeneralConcepts ontology) set to true."@en ;
    rdfs:subClassOf :GroupOfPersons .
#   owl:equivalentClass cco:Populace .

:PopulationOfConcern a owl:Class ;
    rdfs:label "Population of Concern"@en ;
    rdfs:comment "A 'population of concern' is a GroupOfPersons defined by the UNHCR as 'refugees, asylum seekers, internally displaced persons (IDPs) ..., stateless persons, and returnees (returned refugees and IDPs)' (https://www.migrationpolicy.org/programs/data-hub/charts/internally-displaced-persons-idp-stateless-persons-and-other-unhcr)."@en ;
    rdfs:subClassOf :GroupOfPersons .

:Pro-Government a owl:Class ;
    rdfs:label "Pro-Government"@en ;
    rdfs:subClassOf event:Actor .

:RealEstateOrganization a owl:Class ;
    rdfs:label "Real Estate Organization"@en ;
    rdfs:subClassOf :CommercialOrganization ;
    rdfs:comment "Organization concerned with buying, selling or managing real estate/properties"@en .

:ReligiousOrganization a owl:Class ;
    rdfs:label "Religious Organization"@en ;
    rdfs:subClassOf :Organization .
#   owl:equivalentClass oeorg:Religious, oereligion:ReligiousOrganization .

:RetailOrganization a owl:Class ;
    rdfs:label "Retail Organization"@en ;
    rdfs:subClassOf :CommercialOrganization ;
    rdfs:comment "Organization concerned with selling 'consumer goods or services to customers through multiple channels of distribution' (from Wikipedia)"@en .

:SalafistJihadistOrganization a owl:Class ;
    rdfs:label "Salafist Jihadist Organization"@en ;
    rdfs:comment "A Salafist Jihadist Organization is a type of TerroristOrganization that supports 'Salafist jihadism'."@en ;
    rdfs:subClassOf :JihadistOrganization .

:ServiceProvider a owl:Class ;
    rdfs:label "Service Provider"@en ;
    rdfs:subClassOf :CommercialOrganization ;
    rdfs:comment "Organization that provides services. The type of services provided can be defined using the position_or_role property from the GeneralConcepts ontology. For example, the position_or_role can specify 'Application_service_provider', 'Internet_service_provider', 'Managed_services', etc."@en .
#   owl:equivalentClass cco:ServiceProvider .

:SoftwareOrganization a owl:Class ;
    rdfs:label "Software Organization"@en ;
    rdfs:subClassOf :CommercialOrganization ;
    rdfs:comment "Organization concerned with the creation, distribution, use or management of software and data"@en .

:StatelessPersons a owl:Class ;
    rdfs:label "Stateless Person(s)"@en ;
    rdfs:comment "Stateless persons are individuals who are not considered as nationals by any State under the operation of its law."@en ;
    rdfs:subClassOf :PopulationOfConcern .

:SupportSystemOrNetwork a owl:Class ;
    rdfs:label "Support System or Network"@en ;
    rdfs:comment "A group of Actors providing emotional, financial or practical support to another Actor."@en ;
    rdfs:subClassOf :GroupOfActors .

:TaskForce a owl:Class ;
    rdfs:label "Task Force"@en ;
    rdfs:comment "A GroupOfPersons working together on a single task or activity, specifically designated as a 'task force'."@en ;
    rdfs:subClassOf :GroupOfPersons .
# oeceo:JointTaskForce rdfs:subClassOf :TaskForce .

:TerroristOrganization a owl:Class ;
    rdfs:label "Terrorist Organization"@en ;
    rdfs:subClassOf :Organization .
#   owl:equivalentClass oeceo:TerroristOrganization .

:TransportationOrganization a owl:Class ;
    rdfs:label "Transportation Organization"@en ;
    rdfs:comment "Organization dealing with personnel or cargo transportation"@en ;
    rdfs:subClassOf :CommercialOrganization .

:UtilitiesOrganization a owl:Class ;
    rdfs:label "Utilities Organization"@en ;
    rdfs:comment "Organization dealing with infrastructure services such as electricity, natural gas, water, sewage, telephone, internet and mass transportation services"@en ;
    rdfs:subClassOf :Organization .
#   owl:equivalentClass oeorg:Development .

_:UnionOfPersonGroupOfPersons1 a owl:Class ;
    owl:unionOf ( :Person :GroupOfPersons ) .
