@prefix : <http://ontology.causeex.com/ontology/odps/Event#> .
# @prefix cco: <http://www.ontologyrepository.com/CommonCoreOntologies/> .
@prefix dcterms: <http://purl.org/dc/terms/> .
@prefix event: <http://ontology.causeex.com/ontology/odps/Event#> .
@prefix general: <http://ontology.causeex.com/ontology/odps/GeneralConcepts#> .
# @prefix oeceo: <http://www.ontologylibrary.mil/OperationalEnvironment/Mid/OECausalExplorationOntology#> .
# @prefix oeevent: <http://www.ontologylibrary.mil/OperationalEnvironment/Mid/OEEventOntology#> .
@prefix owl: <http://www.w3.org/2002/07/owl#> .
@prefix rdf: <http://www.w3.org/1999/02/22-rdf-syntax-ns#> .
@prefix rdfs: <http://www.w3.org/2000/01/rdf-schema#> .
@prefix xsd: <http://www.w3.org/2001/XMLSchema#> .

<http://ontology.causeex.com/ontology/odps/Event-Hierarchy> rdf:type owl:Ontology ;
    dcterms:description "Ontology defining the sub-classes of Event, extending the top-level hierarchy defined in the Event ontology."@en ;
    dcterms:created "January 28, 2018"^^xsd:string ;
    dcterms:modified "May 17, 2019"^^xsd:string ;
    rdfs:comment """May 17th 2019 revisions:
                      Added the class, ExperimentOrTest.
                      Corrected noun_examplar (should be exemplar) typo.
                      Corrected typo in the super-class of ExhibitionOfPower and Terrorism.
                      Added a description/comment for ContaminatedWater. 
                      Corrected 2nd rdfs:label to be rdfs:comment for Forgiving and WaterManagement.
                   May 13th 2019 revisions:
                     Corrected circular sub-classing references involving JudicialGovernmentActivity and LegalEvent, and 
                       LocationChange and TransportationOfPeopleOrCargo.
                     Updated subclassing where unionOf blank nodes were used as a super-class. Now, an explicit Event class is the 
                       super-class and an owl:equivalentClass defines the unionOf.
                     Corrected references to Wikipedia entries for general:position_or_role.
                     Added AwarenessOrUnderstanding (and its sub-classes), Counteraction, MilitaryOccupation, ProtectionOrPreservation,
                       LocatingOrTargeting, Neutralization, TrespassOrIncursion and UnexpectedAct.
                     Deprecated ExpulsionDeportationOrWithdrawal in lieu of Withdrawal, MeetingEncounterOrNegotiation in lieu of 
                       MeetingOrEncounter, and ManufacturingOrBuilding in lieu of ManufacturingCreatingOrBuilding.
                     Simplified the class hierarchy, making sure that all classes directly sub-classed from :EventOrFactor (but still 
                       defined unionOf statements where appropriate).
                     Added CropFailure, InsestInfestation, Confirmation, Deterrence, Biological/Chemical/ElectromagneticRadiation/Explosive/
                       Nuclear/RadiologicalHazard.
                     Added rdfs:comments/descriptions (when not defined) for many event classes, and added JP1-02 definitions where they were
                       applicable. Updated other descriptions/comments to clarify semantics. 
                     Deprecated EmploymentRelatedEvent in lieu of Employment, and ConsumerSpending in lieu of Spending.
                     Deprecated the class, LackOfOrNegativeSupport, since its semantics overlap with DisapprovalOrDenunciation OR are not 
                       actually a Communication at all (lack of support is an absence of support), but a Factor. LackOfSupport is newly 
                       defined to capture the latter.
                     Deprecated the class, NeedOrRequirement, since this semantic can be represented by Dependence/Independence.
                     Deprecated the classes, ViolationOfCeasefire and ViolationOfTruce, in lieu of using ViolationOfCeasefireOrTruce.
                     Deprecated the class, Confession, in lieu of using ClaimingOfResponsibility since the semantics are roughly equivalent.
                     Added the super-class, Modifier, to convey the semantic of an additional classification and provide a specific class 
                       for extension.
                     Deprecated the class, RepresentativeCommunication, since its semantics are too similar to DeclarativeCommunication.
                     Deprecated the classes, Contempt and Disgust in lieu of ContemptOrDisgust, ApprehensionAnxietyOrWorry and Fear in lieu of 
                       ApprehensionAnxietyFearOrWorry, and Distrust and Suspicion in lieu of DistrustOrSuspicion, since their semantics 
                       are similar. Also deprecated CommunicationViaVideo in lieu of CommunicationViaConferencing, and FindingOfInnocent in 
                       lieu of FindingOfNotGuilty.
                     Removed ontology history older than 6 months. 
                   February 16th 2019 revisions:
                     Added Curiosity (sub-class of EmotionalResponse), and added Access (and its sub-class AirAccess), Trade/PowerBalance, 
                       LivingCondition, RelevanceOrImportance, Taxation and PhysicalSeparation (all sub-classes of Factor).
                     Corrected a non-UTF8 character in the description of EthnicCleansing.
                     Added Death to the super-classes of MurderOrHomicide.
                   February 5th 2019 revisions:
                     Corrected super-class of Indictment. Corrected variations of PersonalOrPassengerTransportation to be consistent.
                     Changed the super-class of RoadBlocked to BlockadeOrRestrictionOfMovement, and corrected typo in the label for 
                       ExpressionOfCondolenceOrSympathy.
                   January 24th 2019 revisions:
                     Added the classes, EnvironmentalProtection and PublicTransportation. Added an explanatory comment for SocialServices.
                     Generalized WaterManagementLandUse to WaterManagement (since the original semantics can be conveyed using multiple
                       inheritance). 
                     Added classes from the NATO Geospatial Feature Concept List and other concepts derived from that list.
                     Added the NaturalDisaster class and updated several classes to use it as their super-class.
                     Added the TransportationOfPeopleOrCargo class.
                     Updated the ontology name.
                   November 15th, 2018 revisions: 
                     Added new sub-classes to further address the Kaliningrad AO (Immigration, CultureTransformationOrLoss, Deployment, 
                       Influence, Communication/MilitaryFactor, ...).
                     Renamed to indicate the full semantics - Accusation -> AccusationOrAssigningOfResponsibility and PersonalTransportation
                       -> PersonalOrPassengerTransportation.
                     Created separate semantics for ImportAndExport - Import, Export. 
                     Added CommunicationViaVideo.
                     Corrected the super-class of BlackMarketTrade.
                   October 23rd 2018 revisions:
                     Corrected sub-classing for several classes.
                     Added ElectromagneticActivity, InformationHandling, InformationOperation, RecruitmentActivity and RecruitmentOperation.
                     Renamed DeceptiveCommunication to Deception, ReleaseOfPropaganda to PropagandaActivity (to expand its semantics 
                       and changed its subclassing), Preparedness to PreparednessOrCapability.
                     Removed MeasurementFactor since it is not needed (a TimeSeries is defined as CollectionOfEventsOrFactors and can subclass
                       directly to define its semantics/use it as an Event, and a ReportedValue is related using meas:has_reported_value). 
                     Added PhysicalMeasurement to indicate a Factor that based on some TimeSeries or ReportedValue that involves a physical property.
                     Renamed/generalized EnvironmentalDegradation to EnvironmentalFactor, since its direction can be defined by the SeriesTrend.
                     Added many concepts from the ReportedPropertyHierarchy (which is removed) to guarantee that all semantics are addressed.
                     Changed some equivalentClass definitions to subClassOf, and updated descriptions/comments.
                     Removed Marriage (the ceremony) since Wedding is equivalent. 
                     Added Oligarchy to the GovernmentalFactors (Democracy and Autocracy).
                     Commented out references to cco:, oeevent: and oeceo: classes that are only used in equivalencies and sub-class declarations. 
                     Removed ontology history older than 6 months."""@en ;
#   owl:imports <http://www.ontologyrepository.com/CommonCoreOntologies/Mid/AllCoreOntology> ;
#   owl:imports <http://www.ontologylibrary.mil/OperationalEnvironment/Mid/OEOntology> ;
    owl:imports <http://ontology.causeex.com/ontology/odps/Event> ;
    owl:imports <http://purl.org/dc/terms> ;
    owl:versionInfo "Version 2.96"^^xsd:string .

#################################################################
#    Sub-classes of event:EventOrFactor
#################################################################


# Following are descriptive events/tags that can be added to any individual
# to further clarify the Event

:Anti-Government a owl:Class ;
    rdfs:label "Anti-Government"@en ;
    rdfs:comment "An additional classification on an Event/Factor (such as an event:DemonstrationOrProtest or event:RequestOrAppeal) to indicate that it was targeted against/opposed to the government or current administration. Anti-Government should not be used alone to classify an Event/Factor individual."@en ;
    rdfs:subClassOf :DisapprovalOrDenunciation, :Modifier .

:Attempt a owl:Class ;
    rdfs:label "Attempt to commit act"@en ;
    rdfs:comment "An additional classification on an Event to indicate that an Actor tried to cause the Event to occur, but did not succeed. Attempt should not be used alone to classify an Event individual."@en ;
    rdfs:subClassOf :Modifier .

:InitiationOrStart a owl:Class ;
    rdfs:label "Initiation/start"@en ;
    rdfs:comment "An additional classification on an Event to indicate that an ongoing Event/Factor began. InitiationOrStart should not be used alone to classify an Event individual."@en ;
    rdfs:subClassOf :Modifier .
#   owl:equivalentClass cco:ProcessBeginning .

:Modifier a owl:Class ;
    rdfs:label "Modifier (abstract)"@en ;
    rdfs:comment "Conveys the semantic of an additional classification of an Event that further clarifies/modifies the type. The Modifier class is considered 'abstract' meaning that it should not be used for classification. It exists as a location in the EventOrFactor hierarchy for extension. In addition, any of the Modifier sub-classes should not be used alone to classify an Event/Factor individual. Examples of modifier classes are Attempt (indicating a failed event) or StrongOrIntense."@en ;
    rdfs:subClassOf :EventOrFactor .

:Pro-Government a owl:Class ;
    rdfs:label "Pro-Government"@en ;
    rdfs:comment "An additional classification on an Event/Factor (such as an event:DemonstrationOrProtest or event:RequestOrAppeal) to indicate that it was in support of the government or current administration. Pro-Government should not be used alone to classify an Event/Factor individual."@en ;
    rdfs:subClassOf :DefenseOrSupport, :Modifier .

:StrongOrIntense a owl:Class ;
    rdfs:label "Strong or intense"@en ;
    rdfs:comment "An additional classification on an Event/Factor to indicate that the occurrence or Factor was more intense/above conventional standards. StrongOrIntense should not be used alone to classify an Event/Factor individual."@en ;
    rdfs:subClassOf :Modifier .

:TerminationOrEnd a owl:Class ;
    rdfs:label "Termination/end"@en ;
    rdfs:comment "An additional classification on an Event to indicate that an ongoing Event/Factor ended. TerminationOrEnd should not be used alone to classify an Event individual."@en ;
    rdfs:subClassOf :Modifier .
#   owl:equivalentClass cco:ProcessEnding .

:UnexpectedAct a owl:Class ;
    rdfs:label "Unexpected act"@en ;
    rdfs:comment "An additional classification on an Event to indicate that the Event could not have been foretold/was not anticipated. UnexpectedAct should not be used alone to classify an Event individual."@en ;
    general:noun_exemplar "The story is more exciting when the [[unexpected]] happens to the hero."@en ;
    general:noun_exemplar "The attacks were unanticipated and demonstrated the enemy's [[unpredictability]]."@en ;
    general:verb_exemplar "The protesters' reaction was [[unanticipated]]."@en ;
    rdfs:subClassOf :Modifier .

:UnintentionalAct a owl:Class ;
    rdfs:label "Unintentional act"@en ;
    rdfs:comment "An additional classification on an Event to indicate that an 'active' Actor did not intention to cause the Event. UnintentionalAct should not be used alone to classify an Event individual."@en ;
    rdfs:subClassOf :Modifier .

:WeakOrLimited a owl:Class ;
    rdfs:label "Weak"@en ;
    rdfs:comment "An additional classification on an Event/Factor to indicate that it was limited/relatively minor/below conventional standards. WeakOrLimited should not be used alone to classify an Event/Factor individual."@en ;
    rdfs:subClassOf :Modifier .


# The following are specific types of events.

:AbductionHostageTakingOrHijacking a owl:Class ;
    rdfs:label "Abduction, hostage taking and/or hijacking"@en ;
    rdfs:comment "Involves taking one or more persons against their will, and may be coupled with threats to harm those persons. The abduction, hostage taking or hijacking may be motivated by monetary gain, to highlight/support a cause, or to force another Actor to take some desired action (such as a political or administrative concession). Although hijackings involve the seizure of an aircraft or other vehicle (in transit), the goal is usually (but not always) related to using the passengers as hostages. A specific goal (Event) can be defined using the actor:has_objective property."@en ;
    rdfs:subClassOf :Event .
#   owl:equivalentClass oeevent:Abduct\,_hijack\,_take_hostage .

:Access a owl:Class ;
    rdfs:label "Access (to an area/location)"@en ;
    rdfs:comment "Factor dealing with the means of approaching or entering a location which may be affected by blockades, physical perimeters, defensive weapons and actions, etc. From JP1-02, 'In counterintelligence and intelligence use, [access is] a. a way or means of approach to identify a target; or b. exploitable proximity to or ability to approach an individual, facility, or information that enables target to carry out the intended mission.'"@en ;
    rdfs:subClassOf :Factor .

:Accident a owl:Class ;
    rdfs:label "Accident"@en ;
    rdfs:comment "Identifies an Event that happens unexpectedly and unintentionally, and that may result in injury or damage. The individual can be qualified as to what caused the accident using the property, event:has_instrument (for example, event:has_instrument cco:Automobile to indicate a car accident)."@en ;
    rdfs:subClassOf :Event .

:AccusationOrAssigningOfResponsibility a owl:Class ;
    rdfs:label "Accusation or assigning of responsibility"@en ;
    rdfs:comment "When using the AccusationOrAssigningOfResponsibility Event type, it is important to indicate who is accused of/responsible for what. This is accomplished using the event:has_affected_actor and event:has_topic object properties. An example is to accuse a Person of a crime (where the Person is the affected actor), and the crime is referenced using the event:has_topic property. The affected actor in the AccusationOrAssigningOfResponsibility Event is the active actor who supposedly committed the crime. Note that although the example is about criminal accusations, the class can describe any claim that someone did something (positive or negative)."@en ;
    rdfs:subClassOf :DeclarativeCommunication .
#   owl:equivalentClass oeevent:Accuse .

:AdequateSupply a owl:Class ;
    rdfs:label "Adequate supply"@en ;
    rdfs:comment "There can be supplies of things/artifacts (such as a supply of food or fuel) or of services or people in certain roles (such as a supply of trained teachers or firefighters). The details of the first (supplies of things) are described by an AdequateSupply individual that references the thing/artifact (for example, food in general or a particular type of food such as potatoes, fuel, water, etc.) using the general:involves_goods_or_property object property. The details of the second (supplies of people in roles) are described by an AdequateSupply individual that references a GroupOfPersons using the event:has_actor property with their role defined using the general:position_or_role property."@en ;
    rdfs:subClassOf :Factor .

:AdministrativeSanctions a owl:Class ;
    rdfs:label "Administrative sanctions"@en ;
	rdfs:comment "An administrative sanction is any type of formal decree, law or policy aimed at curbing the rights of civilians."@en ;
    rdfs:subClassOf :Sanctions .
#   owl:equivalentClass oeevent:Impose_administrative_sanctions .

:Advising a owl:Class ;
    rdfs:label "Advising"@en ;
    rdfs:comment "Advising is any type of suggestion or providing advice. This is distinct from the semantics of DecisionOrRecommendation which is a conclusion/resolution. The difference can also be seen in the super-classes of Advising versus DecisionOrRecommendation. This class sub-classes from DirectiveCommunication, while DecisionOrRecommendation sub-classes from DeclarativeCommunication. When using the Advising Event type, it is important to indicate who is advised of what. This is accomplished using the event:has_affected_actor and event:has_topic object properties."@en ;
    rdfs:subClassOf :DirectiveCommunication .
#   owl:equivalentClass cco:ActOfAdvising .

:Affiliation a owl:Class ;
    rdfs:label "Affiliation"@en ;
    rdfs:comment "An Affiliation Event is different than defining the long-term affiliation of an Actor to a Group, Organization, Location, etc. The Event describes an occurrence of note such as a new CEO taking over a company, an Organization supporting/affiliating itself with a humanitarian effort, or a pledge of allegiance of a Group to an individual. Typically, an individual Event that is an Affiliation will also be of another type such as InitiationOrStart or TerminationOrEnd. Also, it may be classified with an additional type, such as ContractRelatedEvent or EmploymentRelatedEvent. The semantics of the long-term affiliation mentioned above is described using an instance of the Actor ontology's Affiliation class."@en ;
    rdfs:subClassOf :Event .
#   rdfs:subClassOf cco:ActOfAssociation .

:AgeDemographic a owl:Class ;
    rdfs:label "Age demographic"@en ;
    rdfs:comment "A Factor providing data (typically, an individual meas:ReportedValue or meas:TimeSeries) about the age characteristics of a population or particular sub-groups within it. The population/group whose demographic is reported is identified using the event:has_actor property."@en ;
    rdfs:subClassOf :Demographic .

:Aggression a owl:Class ;
    rdfs:label "Aggression"@en ;
    rdfs:comment "Aggression covers a range of behaviors. It is intended to be about the expression of anger or dominance. If Aggression progresses to an Attack, then it is recommended that 2 Event individuals be created - and the Attack would be related to the Aggression individual via the event:preceded_by property."@en ;
    rdfs:subClassOf :Event .

:AgreementOrPromise a owl:Class ;
    rdfs:label "Agreement or promise"@en ;
    rdfs:comment "AgreementOrPromise characterizes any act where two or more Actors share the same opinion and/or concur to do something. When using the AgreementOrPromise Event type, it is important to indicate what is agreed to and with/to whom the agreement/promise is made. This is accomplished using the event:has_active_actor and event:has_topic object properties."@en ;
    rdfs:subClassOf :CommissiveCommunication .
#   owl:equivalentClass cco:ActOfPromising, oeevent:Express_accord .

:AgriculturalEvent a owl:Class ;
    rdfs:label "Agricultural event"@en ;
    rdfs:comment "AgriculturalEvents deal with any acts such as farming, harvesting, breeding animals, etc."@en ;
    rdfs:subClassOf :Event .

:AgriculturalLandUse a owl:Class ;
    rdfs:label "Agricultural/farming land use"@en ;
    rdfs:comment "AgriculturalLandUse describes how the land/environment is managed or modified for settlements, farming, mining, etc. It does not describe specific acts (these are event:AgriculturalEvents) but general details/factors."@en ;
    rdfs:subClassOf :LandUse .

:AirAccess a owl:Class ;
    rdfs:label "Air access (to an area)"@en ;
    rdfs:comment "Factor dealing with the means of approaching or entering a location by air. This access may be affected by the definition of 'no-fly zones', by the placement of defensive weapons, etc. From JP1-02, 'In counterintelligence and intelligence use, [access is] a. a way or means of approach to identify a target; or b. exploitable proximity to or ability to approach an individual, facility, or information that enables target to carry out the intended mission.'"@en ;
    rdfs:subClassOf :Access .

:AlcoholDrugAndSubstanceAbuse a owl:Class ;
    rdfs:label "Alcohol, drug and substance abuse"@en ;
    rdfs:comment "AlcoholDrugAndSubstanceAbuse may describe either a specific event of abuse, a general condition/factor of increased/decreased abuse (event:Increase/Decrease/Stasis) by a set of people or in a region, or statistics (an individual meas:ReportedValue or meas:TimeSeries) describing abuse in a population/region."@en ;
    rdfs:subClassOf :HealthAndDisease .

:AlertStatus a owl:Class ;
    rdfs:label "Alert status"@en ;
    rdfs:comment "AlertStatus is defined by/for a GeopoliticalEntity (such as a country, city or organization) or for a specific location. The Location (if the alert is for a specific region) is identified using the general:located_at property, while the entity that issued the alert is the active actor."@en ;
    rdfs:subClassOf :Event .

:AmassingAndStockpiling a owl:Class ;
    rdfs:label "Amassing and stockpiling"@en ;
    rdfs:comment "Deals with accumulating goods or materials in order to control a market, have surplus in case of emergency, prepare for some future action, etc. The goods/materials that are accumulated are defined using general:involves_goods_or_property."@en ;
    rdfs:subClassOf :Event .

:Ambush a owl:Class ;
    rdfs:label "Ambush"@en ;
    rdfs:comment "An Ambush is a kind of surprise Attack where the adversary conceals themselves and waits to attack."@en ;
    rdfs:subClassOf :Attack .

:Amusement a owl:Class ;
    rdfs:label "Amusement"@en ;
    rdfs:comment "Amusement is an EmotionalResponse where an Actor is entertained or finds a situation funny. The situation that is found funny can be associated using the event:has_topic property. The Actor is identified using the event:has_active_actor property."@en ;
    rdfs:subClassOf :EmotionalResponse .
#   owl:equivalentClass oeceo:Amusement .

:Anger a owl:Class ;
    rdfs:label "Anger"@en ;
    rdfs:comment "Anger is an EmotionalResponse where an Actor is strongly annoyed or hostile toward another or regarding a situation. The event:has_topic property is used to identify the sitaution. The Actor who is angry is identified using the event:has_active_actor property. If the anger is directed toward another Actor, that individual is identified using event:has_affected_actor."@en ;
    rdfs:subClassOf :StrongOrIntense, :Annoyance .
#   owl:equivalentClass oeceo:Anger .

:AnimalIllnessOrDeath a owl:Class ;
    rdfs:label "Animal illness or death"@en ;
    rdfs:comment "Disease, sickness or death of domestic or wild animals. If the illness/death is in a specific location, that is defined using the general:located_at property. AnimalIllnessOrDeath may describe either a specific event, a general condition/factor of increased/decreased sickness/death (event:Increase/Decrease/Stasis), or statistics (an individual meas:ReportedValue or meas:TimeSeries) related to these semantics."@en ;
    rdfs:subClassOf :HealthAndDisease .

:Announcement a owl:Class ;
    rdfs:label "Announcement"@en ;
    rdfs:comment "Deals with any public statements about future events (such as announcing a new CEO of a company or a government's change in policy). The future events are referenced from the Announcement using the event:has_topic property and would be marked as event:has_tense event:Future (perhaps with a forecasted time)."@en ;
    rdfs:subClassOf :Communication .

:Annoyance a owl:Class ;
    rdfs:label "Annoyance"@en ;
    rdfs:comment "Annoyance is an EmotionalResponse where an Actor is bothered or irritated by someone or by a situation. To identify the situation, the event:has_topic property is used. The Actor who is annoyed is identified using the event:has_active_actor property. If the annoyance is directed toward another Actor, that individual is identified using event:has_affected_actor."@en ;
    rdfs:subClassOf :EmotionalResponse .
#   owl:equivalentClass oeceo:Annoyance .

:Apology a owl:Class ;
    rdfs:label "Apology"@en ;
    rdfs:comment "An expression of regret regarding some trouble/problem that an Actor caused. The Actor making the apology is defined using event:has_active_actor. The Actor to whom the apology is made is identified using event:has_affected_actor. The problem/trouble that was caused is defined using event:has_topic."@en ;
    rdfs:subClassOf :CommunicationConveyingEmpathy .
#   owl:equivalentClass cco:ActOfApologizing .

:ApplicationOfMilitaryOrPoliticalPressure a owl:Class ;
    rdfs:label "Application of military or police pressure"@en ;
    rdfs:comment "Defines a specific sub-class of IntimidationAndCoercion indicating that the active actors (doing the intimidation) are a government and its military."@en ;
    rdfs:subClassOf :IntimidationAndCoercion .

:AppointmentOrNomination a owl:Class ;
    rdfs:label "Appointment or nomination"@en ;
    rdfs:comment "An AppointmentOrNomination proposes a group or individual for some position, award, etc. The entity doing the appointing/nominating is the active actor, the entity that is appointed/nominated is the affected actor and the position (if applicable) is defined using the general:position_or_role property."@en ;
    rdfs:subClassOf :Communication . 

:ApprehensionAnxietyFearOrWorry a owl:Class ;
    rdfs:label "Apprehension, anxiety, fear or worry"@en ;
    rdfs:comment "ApprehensionAnxietyFearOrWorry is an EmotionalResponse where an Actor is troubled by, has misgivings about, or anticipates pain or danger due to a situation or another Actor or thing. The Actor is identified using the event:has_active_actor property. If the response is directed toward another Actor, that individual is identified using the event:has_affected_actor property. If the response concerns a thing, that individual is identified using general:involves_goods_or_property. To associate a situation, the event:has_topic property is used."@en ;
    rdfs:subClassOf :EmotionalResponse .
#   owl:equivalentClass [ a owl:Class ;
#                         owl:unionOf (oeceo:Apprehension oeceo:Worry) ] .

:ApprehensionAnxietyOrWorry a owl:Class ;
    rdfs:label "Apprehension, anxiety or worry (deprecated)"@en ;
    owl:deprecated "true"^^xsd:boolean ;
    rdfs:comment "ApprehensionAnxietyOrWorry is an EmotionalResponse where an Actor is troubled by, has misgivings about, or anticipates pain or danger due to a situation or another Actor or thing. The Actor is identified using the event:has_active_actor property. If the response is directed toward another Actor, that individual is identified using the event:has_affected_actor property. If the response concerns a thing, that individual is identified using general:involves_goods_or_property. To associate a situation, the event:has_topic property is used."@en ;
    rdfs:comment "Note that ApprehensionAnxietyOrWorry is deprecated in lieu of using its super-class, event:ApprehensionAnxietyFearOrWorry."@en ;
    rdfs:subClassOf :ApprehensionAnxietyFearOrWorry .
#   owl:equivalentClass [ a owl:Class ;
#                         owl:unionOf (oeceo:Apprehension oeceo:Worry) ] .

:ArmedConflict a owl:Class ;
    rdfs:label "Armed conflict"@en ;
    rdfs:comment "Conflict between international states, between governmental and non-governmental armed groups, or between non-governmental armed groups only."@en ;
    rdfs:subClassOf :DisagreementOrDispute .

:ArrestOrDetention a owl:Class ;
    rdfs:label "Arrest or detention"@en ;
    rdfs:comment "ArrestOrDetention is a legal/military ('official') action and should be of some (relatively) limited time. This is more semantically related to being stopped/detained or 'in custody', as opposed to being imprisoned for a crime. It is also distinguished from the AbductionHostageTakingOrHijacking Event type (~kidnapping)."@en ;
    rdfs:subClassOf :LegalEvent .
#   owl:equivalentClass oeevent:Arrest\,_detain .

:Arrival a owl:Class ;
    rdfs:label "Arrival"@en ;
    rdfs:comment "The act of getting to a destination. The latter is identified using the general:has_destination property."@en ;
    rdfs:subClassOf :LocationChange .
#   owl:equivalentClass cco:ActOfArrival .

:ArtsAndCulture a owl:Class ;
    rdfs:label "Art and culture"@en ;
    rdfs:comment "Deals with the existence of and access to libraries, museums, theatres, etc, and the ability to create/perform literature, music and art. According the the Arts Council of England, 'When we talk about the value of arts and culture, we should always start with the intrinsic – how arts and culture illuminate our inner lives and enrich our emotional world.  This is what we cherish. But while we do not cherish arts and culture because ofthe impact on our social wellbeing and cohesion, our physical and mental health, our education system, our national status and our economy, they do confer these benefits ... [and are] a strategic national resource."@en ;
    rdfs:subClassOf :Factor .

:Assassination a owl:Class ;
    rdfs:label "Assassination"@en ;
    rdfs:comment "A murder of a public figure by a sudden attack."@en ;
    rdfs:subClassOf :MurderOrHomicide .
#   owl:equivalentClass cco:ActOfAssassination, oeevent:Assassinate .

:Attack a owl:Class ;
    rdfs:label "Attack"@en ;
    rdfs:comment "An offensive act intended to harm an Actor or damage a location, or an emotional assault against an Actor. The Actor taking the offensive/doing the attacking is the active actor, while the Actor that is attaked is the affected actor. If the attack is directed at a location, that is identified using the general:located_at property."@en ;
    rdfs:subClassOf :Violence .

:Autocracy a owl:Class ;
    rdfs:label "Autocracy"@en ;
    rdfs:comment "A type of governement ... an autocracy is a rule by one person. That person has all the power and makes all the decisions."@en ;
    rdfs:subClassOf :GovernmentalFactor .

:Avalanche a owl:Class ;
    rdfs:label "Avalanche"@en ;
    rdfs:comment "A NaturalDisaster involving large masses of snow, ice and mud that rapidly comes down a mountainside."@en ;
    rdfs:subClassOf :NaturalDisaster .

:AwarenessOrUnderstanding a owl:Class ;
    rdfs:label "Awareness or understanding"@en ;
    rdfs:comment "A Factor describing having knowledge/understanding of someone, something or some situation. The latter are described using the properties, event:has_affected_actor, general:involves_goods_or_artifact and event:has_topic, respectively. The Actor who is aware/understands is the active actor."@en ;
    general:verb_exemplar "Japan is [[aware]] that Russia and China have more influence over North Korea than the United States."@en ;
    general:verb_exemplar "The governor [[understands]] that the existence of human rights helps secure the peace and deter aggression."@en ;
    general:noun_exemplar "Situational [[awareness]] is about [[understanding]] what is happening in an area."@en ;
    rdfs:subClassOf :Factor .

:Bankruptcy a owl:Class ;
    rdfs:label "Bankruptcy"@en ;
    rdfs:comment "Bankruptcy is a legal event where an Actor is declared insolvent and unable to pay their debts. In some cases, the Actor's goods and property may be taken and used to pay creditors. The Actor who is bankrupt is defined using the event:has_actor property."@en ;
    rdfs:subClassOf :LegalEvent, :FinancialEvent .

:BanOrProhibition a owl:Class ;
    rdfs:label "Ban or prohibition"@en ;
    rdfs:comment "BanOrProhibition forbids or commands against something. When using this Event type, it is important to indicate who/what is banned. This is accomplished using the event:has_affected_actor and/or event:has_topic object properties."@en ;
    rdfs:subClassOf :DirectiveCommunication .

:Battle a owl:Class ;
    rdfs:label "Battle"@en ;
    rdfs:comment "A fight or combat between opposing forces/groups/persons. Offensive Actors are identified using the event:has_active_actor property, while defensive Actors are identified using the event:has_affected_actor property."@en ;
    rdfs:subClassOf :Attack .

:BiologicalHazard a owl:Class ;
    rdfs:label "Biological hazard"@en ;
    rdfs:comment "A sub-class of EnvironmentalHazard defined by JP1-02 as 'an organism, or substance derived from an organism, that poses a threat to human or animal health."@en;
    general:noun_exemplar "This review concentrates on literatures published after 2010 that attempted to detect [[biological hazards]] to humans, especially workers, and the efforts to protect them against these factors."@en ;
    general:noun_exemplar "A [[biohazard]], also known as a biological hazard, is a biological substance that poses a threat to human and animal health."@en ;
    rdfs:subClassOf :EnvironmentalHazard .

:Birth a owl:Class ;
    rdfs:label "Birth"@en ;
    rdfs:comment "Birth defines a specific life event, relative to either the mother (the active actor), the baby (the affected actor) or both."@en ;
    rdfs:subClassOf :PersonalLifeEvent .
#   owl:equivalentClass cco:Birth .

:BirthsAndFertility a owl:Class ;
    rdfs:label "Births and fertility"@en ;
    rdfs:comment "A Factor providing data (typically, an individual meas:ReportedValue or meas:TimeSeries) about births/birth rates/fertility/etc. of a population or particular sub-groups within it. The population/group whose demographic is reported is identified using the event:has_actor property."@en ;
    rdfs:subClassOf :Demographic .

:BlackMarketTrade a owl:Class ;
    rdfs:label "Black market trade"@en ;
    rdfs:comment "Buying and selling of illegal, illicit, controlled or rationed goods or currencies."@en ;
    rdfs:subClassOf :DomesticTrade .

:BlockadeOrRestrictionOfMovement a owl:Class ;
    rdfs:label "Blockade or restriction of movement"@en ;
    rdfs:comment "BlockadeOrRestrictionOfMovement is related to activities/events to prevent access, or the flow of goods and people, to/from an area. The area that is blockaded/restricted is identified using general:located_at, while the entity imposing or enforcing the blockage/restriction is the active actor. The impacted population is identified as the affected actor. If specific goods are blockaded/restricted, these are identified using the property, general:involves_goods_or_property."@en ;
    rdfs:subClassOf :ReductionRestrictionOrRemoval, :Access .
#   owl:equivalentClass oeevent:Impose_blockade\,_restrict_movement .
#   owl:equivalentClass oeevent:Obstruct_passage\,_block .

:Bombing a owl:Class ;
    rdfs:label "Bombing"@en ;
    rdfs:comment "Bombing is an Attack with an explosive weapon (cco:ExplosiveWeapon)."@en ;
    rdfs:subClassOf :Attack .

:BoycottEmbargoSanctionsOrStrike a owl:Class ;
    rdfs:label "Boycott, embargo, sanctions or strike"@en ;
    rdfs:comment "Deals with either the withdrawal or cessation of trade or relations with another entity, a refusal to work by a group, or the restriction of movement (i.e., a sanction) of items or people. This class is used when the exact nature of the restriction/penalty is unknown."@en ;
    rdfs:subClassOf :ReductionRestrictionOrRemoval ;
    owl:equivalentClass [ a owl:Class ;
                          owl:unionOf ( :BoycottOrEmbargo :Sanctions :Strike ) ] .
# oeevent:Conduct_strike_or_boycott rdfs:subClassOf :BoycottEmbargoSanctionsOrStrike .
# oeevent:Impose_embargo\,_boycott\,_or_sanctions rdfs:subClassOf :BoycottEmbargoSanctionsOrStrike .

:BoycottOrEmbargo a owl:Class ;
    rdfs:label "Boycott or embargo"@en ;
    rdfs:comment "Deals with the withdrawal or cessation of trade or relations with another entity. The Actor imposing the boycott/embargo is the active actor, while the other entity is the affected actor."@en ;
    rdfs:subClassOf :ReductionRestrictionOrRemoval .

:BusinessCeremony a owl:Class ;
    rdfs:label "Business ceremony"@en ;
    rdfs:comment "Examples of BusinessCeremony include a business opening or party celebrating a company's successful release of a product."@en ;
    rdfs:subClassOf :Ceremony .

:CapacityOrStorage a owl:Class ;
    rdfs:label "Capacity or storage"@en ;
    rdfs:comment "Instances of type, CapacityOrStorage (e.g., a pipeline with the capacity of x trillion cubic feet of natural gas, cargo handling capacity, food or water storage capacity or computer processing power), describes the ability to hold/store/deliver/... some artifact. The artifact whose capacity is described is identified using the event:has_instrument property. The artifact which is held/stored/delivered is defined using the general:involves_goods_or_property predicate. To define a particular capacity, use the TimeSeriesAndMeasurements ontology's ReportedValue and the meas:has_measurement_value property."@en ;
    rdfs:subClassOf :Factor .

:CargoTransportation a owl:Class ;
    rdfs:label "Cargo transportation"@en ;
    rdfs:comment "CargoTransportation describes moving goods by air, ground or naval vessels/vehicles. To define the type of goods transported (if that is relevant), use general:involves_goods_or_property. To specify the mode of transportion, use event:has_instrument. And, to identify the Actors sending/receiving the goods or the locations from/to which the goods are transported, use event:has_provider/recipient and event:has_origin/destination, respectively."@en ;
    rdfs:subClassOf :LocationChange .
#   owl:equivalentClass cco:ActOfCargoTransportation .

:CeasefireOrTruce a owl:Class ;
    rdfs:label "Ceasefire or truce"@en ;
    rdfs:comment "An agreement between Actors to stop fighting/a conflict. It may be for a certain period of time which is specified using the general:earliest/latest_possible_start/end_time properties."@en ;
    rdfs:subClassOf :FormalAgreement, :ReductionRestrictionOrRemoval .
#   owl:equivalentClass oeevent:Declare_truce\,_ceaseﬁre .

:Ceremony a owl:Class ;
    rdfs:label "Ceremony"@en ;
    rdfs:comment "A business, social, personal or military gathering in remembrance of a previous event (e.g., a birthday, anniversary, historical event, etc.) or to celebrate/highlight an occassion (such as the opening of a facility). The event being remembered or celebrated is defined using the event:has_topic property. Note that the sub-class, Commemoration, is specifically defined since many activities may be associated with historical commemorations."@en ;
    rdfs:subClassOf :Event .
#   owl:equivalentClass cco:ActOfCeremony .

:Change a owl:Class ;
    rdfs:label "Change"@en ;
    rdfs:comment "The class, Change, and its sub-classes (Increase and Decrease) are used to record a difference in the availability/amount of a thing/artifact (such as a change in the amount of food, water or schooling), a change in the number of people in certain roles (such as a change in the number of police or teachers), or changes related to 'general' Events (such as a change in the number of MurderOrHomicide occurrences in a specific location) or Factors (such as a change in the Anger level in a community). If the change is related to another Event/Factor, the Change individual uses the event:has_topic property to reference that other Event. To identify a change in the availability/amount of something, the Change individual is related to the artifact using general:involves_goods_or_property. To identify a change in the number of people in certain roles, those people are defined as an individual that is a GroupOfPersons with a general:position_or_role property, and that entity is related to Change via event:has_actor."@en ;
    rdfs:subClassOf :EventOrFactor .
#   owl:equivalentClass cco:Change .

:ChangeOfResidence a owl:Class ;
    rdfs:label "Change of residence"@en ;
    rdfs:comment "ChangeOfResidence is a sub-class of LocationChange highlighting that an individual or group is moving their home(s) to a new location. The reason for the move may be mandated by political, military or environmental conditions or voluntarily. When the change is 'caused' by other Actors or conditions, the ChangeOfResidence individual may be related to these using a causal:CausalAssertion or (at a minimum) by an event:preceded_by property relationship."@en ;
    rdfs:subClassOf :LocationChange .
#   owl:equivalentClass cco:ActOfChangeOfResidence .

:ChemicalHazard a owl:Class ;
    rdfs:label "Chemical hazard"@en ;
    rdfs:comment "A sub-class of EnvironmentalHazard defined by JP1-02 as 'any chemical manufactured, used, transported, or stored that can cause death or other harm through toxic properties of those materials, including chemical agents and chemical weapons prohibited under the Chemical Weapons Convention as well as toxic industrial chemicals.'."@en ;
    general:noun_exemplar "[[Chemical hazards]] and toxic substances pose a wide range of health hazards (such as irritation, sensitization, and carcinogenicity) and physical hazards (such as flammability, corrosion, and explosibility)."@en ;
    rdfs:subClassOf :EnvironmentalHazard .

:ChemicalUse a owl:Class ;   
    rdfs:label "Chemical use"@en ;
    rdfs:comment "ChemicalUse indicates that some event:ChemicalSubstance was used. The type of substance is indicated by the event:has_instrument, which could reference an event:Pesticide, event:CryogenicMaterial, etc."@en ;
    rdfs:subClassOf :Event .

:CivilCampaign a owl:Class ;
    rdfs:label "Civil campaign"@en ;
    rdfs:comment "A CivilCampaign is a sub-class of Operation. Examples of CiviCampaigns are neighborhood watches, or a group of citizens getting together to cleanup a neighborhood or to raise money for a family in need. An Operation occurs over time, has specific goals, and is composed of specific, coordinated acts/Events intended to achieve those goals. The component Events (if known) are associated using the general:has_member property. The goal is identified using the actor:has_objective property."@en ;
    rdfs:subClassOf :Operation .

:ClaimingOfResponsibility a owl:Class ;
    rdfs:label "Claiming of responsibility"@en ;
    rdfs:comment "Deals with an Actor (the active actor) indicating that they are responsible for some Event. The Event for which responsibility is taken is specified using event:has_topic. Note that claiming responsibility may not actually be a true statement."@en ;
    rdfs:subClassOf :DeclarativeCommunication .
#   owl:equivalentClass oeevent:Acknowledge_or_claim_responsibility .

:ColdTemperature a owl:Class ;
    rdfs:label "Cold temperature"@en ;
    rdfs:comment "Temperatures perceived as 'low', typically related to freezing temperatures, snow/ice, etc."@en ;
    rdfs:subClassOf :WeatherIssue .

:CollapsedStructure a owl:Class ;
    rdfs:label "Collapsed structure"@en ;
    rdfs:comment "StructuralDamage may be so severe that the structure actually fails/gives way and is no longer usable. Examples of collapsed structures include buildings, bridges, etc."@en ;
    rdfs:subClassOf :StructuralDamage .

:Collision a owl:Class ;
    rdfs:label "Collision"@en ;
    rdfs:comment "An Accident where a moving object impacts an Actor or Artifact. If the Collision was unintended, then the Modifier, event:UnintentionalAct, should also be used to classify the individual. If it was intended, however, then there should be an Actor defined using event:has_active_actor. The moving object which impacts another is identified using event:has_instrument, while the impacted Actor or Artifact (or both) are identified using event:has_affected_actor and general:involves_goods_or_property, respectively."@en ;
    rdfs:subClassOf :Accident .
#   owl:equivalentClass cco:ActOfCollision .

:Commanding a owl:Class ;
    rdfs:label "Commanding"@en ;
    rdfs:comment "Commanding involves issuing orders or instructions. When classifying individuals with this type, it is important to indicate who/what is commanded. This is accomplished using the event:has_affected_actor and event:has_topic object properties. In JP1-02, command is defined as '1. The authority that a commander in the armed forces lawfully exercises over subordinates by virtue of rank or assignment. 2. An order given by a commander; that is, the will of the commander expressed for the purpose of bringing about a particular action. 3. A unit or units, an organization, or an area under the command of one individual.'"@en ;
    rdfs:subClassOf :DirectiveCommunication .
#   owl:equivalentClass cco:ActOfCommanding .

:Commemoration a owl:Class ;
    rdfs:label "Commemoration"@en ;
    rdfs:comment "A Commemoration is a Ceremony held to remember an Event. The Event being remembered or celebrated (for example, a person's birthday or a historical event, such as the bombing of Pearl Harbor) is defined using the event:has_topic property."@en ;
    rdfs:subClassOf :Ceremony .

:CommercialOperation a owl:Class ;
    rdfs:label "Commercial or business operation"@en ;
    rdfs:comment "A CommercialOperation is about specific sets of activities that a business undertakes, such as a reorganization, a construction project, a software project, etc. An Operation occurs over time, has specific goals, and is composed of specific, coordinated acts/Events intended to achieve those goals. The component Events (if known) are associated using the general:has_member property. The goal is identified using the actor:has_objective property."@en ;
    rdfs:subClassOf :Operation .

:CommissiveCommunication a owl:Class ;
    rdfs:label "Commissive communication (committing an actor to future behaviors/actions)"@en ;
    rdfs:comment "Deals with any kind of commitment (in general), agreement, promise, contract, oath taking, etc. and/or expression of intent to do something. More specific types of commitment are defined as sub-classes. When using the CommissiveCommunication Event type (or one of its sub-classes), it is important to indicate what is being committed. This is accomplished using the event:has_topic object property."@en ;
    rdfs:subClassOf :Communication .
#   owl:equivalentClass cco:ActOfCommissiveCommunication .

:CommunicationConveyingEmotion a owl:Class ;
    rdfs:label "Communication conveying emotion"@en ;
    rdfs:comment "Deals with communications conveying empathy (such as apologizing or forgiving), optimism, pessimism, sympathy, thanks, threats, etc. More specific types are defined as sub-classes."@en ;
    rdfs:subClassOf :Communication .
#   owl:equivalentClass cco:ActOfExpressiveCommunication .

:CommunicationConveyingEmpathy a owl:Class ;
    rdfs:label "Communication conveying empathy"@en ;
    rdfs:comment "Deals with any communications that express that one Actor understands or shares the feelings of another."@en ;
    rdfs:subClassOf :CommunicationConveyingEmotion .
#   owl:equivalentClass oeevent:Make_empathetic_comment .

:CommunicationConveyingOptimism a owl:Class ;
    rdfs:label "Communication conveying optimism"@en ;
    rdfs:comment "Deals with any communications that express hope for the future,  or belief in the success of some endeavor/action (the specific 'action' is an Event associated using event:has_topic and which may have a tense of event:Future)."@en ;
    rdfs:subClassOf :CommunicationConveyingEmotion .
#   owl:equivalentClass oeevent:Make_optimistic_comment .

:CommunicationConveyingPessimism a owl:Class ;
    rdfs:label "Communication conveying pessimism"@en ;
    rdfs:comment "Deals with any communications that express dismay for the future,  or the belief that some endeavor/action will not succeed/will fail (the specific 'action' is an Event associated using event:has_topic and which may have a tense of event:Future)."@en ;
    rdfs:subClassOf :CommunicationConveyingEmotion .
#   owl:equivalentClass oeevent:Make_pessimistic_comment .

:CommunicationFactor a owl:Class ;
    rdfs:label "Communication factor"@en ;
    rdfs:comment "Describes the capabilities or availability of communication services. Examples include the availability or number of subscribers to land line/cellular/internet services, the coverage of cellular towers or satellites in an area, or other aspects of networks, transmission systems, relay stations, tributary stations and/or data terminal equipment (DTE)."@en ;
    rdfs:subClassOf :InfrastructureAndUtilities .

:CommunicationViaConferencing a owl:Class ;
    rdfs:label "Communication via conferencing technology"@en ;
    rdfs:comment "Indicates that an Actor (the active actor) used the medium of video/chat conferencing to contact another Actor or group. This Event does not define the content of/information in the communication (which is a type of event:Communication or one of its sub-classes), but the means of the communication."@en ;
    rdfs:subClassOf :PersonalCommunication .

:CommunicationViaInstantOrTextMessage a owl:Class ;
    rdfs:label "Communication via instant or text message"@en ;
    rdfs:comment "Indicates that an Actor (the active actor) used the medium of text/instant messaging to contact another Actor or group. This Event does not define the content of/information in the communication (which is a type of event:Communication or one of its sub-classes), but the means of the communication."@en ;
    rdfs:subClassOf :PersonalCommunication .

:CommunicationViaLetterOrPersonalMail a owl:Class ;
    rdfs:label "Communication via letter or personal mail"@en ;
    rdfs:comment "Indicates that an Actor (the active actor) used the medium of a message delivered by mail/a postal service or via email to contact another Actor or group. This Event does not define the content of/information in the communication (which is a type of event:Communication or one of its sub-classes), but the means of the communication."@en ;
    rdfs:subClassOf :PersonalCommunication .

:CommunicationViaPhone a owl:Class ;
    rdfs:label "Communication via phone (via land-line or cellular)"@en ;
    rdfs:comment "Indicates that an Actor (the active actor) used the medium of a cellular phone or land line to contact another Actor or group. This Event does not define the content of/information in the communication (which is a type of event:Communication or one of its sub-classes), but the means of the communication."@en ;
    rdfs:subClassOf :PersonalCommunication .
#   owl:equivalentClass oeevent:Discuss_by_telephone .

:CommunicationViaVideo a owl:Class ;
    rdfs:label "Communication via video (deprecated)"@en ;
    owl:deprecated "true"^^xsd:boolean ;
    rdfs:comment "Indicates that an Actor (the active actor) used the medium of video conferencing to contact another Actor or group. This Event does not define the content of/information in the communication (which is a type of event:Communication or one of its sub-classes), but the means of the communication."@en ;
    rdfs:comment "Note that CommunicationViaVideo is deprecated in lieu of using its super-class, event:CommunicationViaConferencing."@en ;
    rdfs:subClassOf :CommunicationViaConferencing .

:Compassion a owl:Class ;
    rdfs:label "Compassion"@en ;
    rdfs:comment "Compassion is an EmotionalResponse where an Actor is sympathically aware of or concerned about another Actor or a situation. If emotion concerns a situation, it can be associated using the event:has_topic property. The Actor who is compassionate is identified using the event:has_active_actor property. If the compassion is directed toward another Actor, that individual is identified using event:has_affected_actor."@en ;
    rdfs:subClassOf :EmotionalResponse .
#   owl:equivalentClass oeceo:Compassion .

:Competition a owl:Class ;
    rdfs:label "Competition"@en ;
    rdfs:comment "A Competition may be a sporting event between opposing teams (in which case it is also classified as an event:EntertainmentEvent) or it may describe a general Factor where two or more groups are attempting to establish superiority or control over each other, over a territory, etc. The latter should also be classified as a type of event:Factor. There are many examples of military, political and economic Competition which are defined by the Actors involved in it."@en ;
    rdfs:subClassOf :EventOrFactor .

:ConcentrationOfDisplacedPersons a owl:Class ;
    rdfs:label "Concentration of displaced persons"@en ;
    rdfs:comment "A Factor providing data (typically, an individual meas:ReportedValue or meas:TimeSeries) about displacements in/of a population or particular sub-groups within it. The population/group whose demographic is reported is identified using the event:has_actor property."@en ;
    rdfs:subClassOf :Demographic .

:Confession a owl:Class ;
    rdfs:label "Confession (deprecated)"@en ;
    owl:deprecated "true"^^xsd:boolean ;
    rdfs:comment "Deals with an Actor (the active actor) indicating that they are responsible for some Event. The Event for which responsibility is taken is specified using event:has_topic. Note that claiming responsibility may not actually be a true statement."@en ;
    rdfs:comment "Note that Confession is deprecated in lieu of using its super-class, ClaimingOfResponsibility."@en ;
    rdfs:subClassOf :ClaimingOfResponsibility .
#   owl:equivalentClass oeevent:Acknowledge_or_claim_responsibility .

:Confidence a owl:Class ;
    rdfs:label "Confidence"@en ;
    rdfs:comment "Confidence in the future is hope, while Confidence as belief in someone/something is trust. These semantics can be better conveyed by using the event:Hope or event:Trust classes, if the distinction is known. In general, Confidence is an EmotionalResponse where an Actor has positive feelings, desires or expectations that something will occur, or believes in the ability/capabilities of someone or something. The situation which inspires the confidence, if known, can be associated using the event:has_topic property (and could be defined with an event:has_tense of event:Future). When the confidence is directed toward another Actor, that individual is identified using event:has_affected_actor. If the confidence is about a thing (such as being confident that a lock on a door will hold), the artifact is identified using general:involves_goods_or_property. The Actor who has confidence is identified using the event:has_active_actor property."@en ;
    rdfs:subClassOf :EmotionalResponse ;
    owl:equivalentClass [ a owl:Class ;
                          owl:unionOf ( :Hope :Trust ) ] .

:Confirmation a owl:Class ;
    rdfs:label "Confirmation/validation of act/event"@en ;
    rdfs:comment "Confirmation is an Event where some Event/Factor is verified/validated or some Actor is formally placed in a role. When using the Confirmation Event type, it is important to indicate what has been validated/established to be 'true' or the Actor and role. The former is accomplished using the event:has_topic property (referencing the 'confirmed' act/event). The latter is accomplished using event:has_affected_actor and general:position_or_role property to define the position/role. An example of a Confirmation is validating that a crime occurred (where the crime is specified using event:has_topic)."@en ;
    rdfs:comment "From JP1-02, validation is '1. A process associated with the collection and production of intelligence that confirms that an intelligence collection or production requirement is sufficiently important to justify the dedication of intelligence resources, does not duplicate an existing requirement, and has not been previously satisfied. 2. A part of target development that ensures all candidate targets meet the objectives and criteria outlined in the commander’s guidance and ensures compliance with the law of war and rules of engagement. 3. In the context of time-phased force and deployment data validation, it is an execution procedure whereby all the information records in the timephased force and deployment data are confirmed error-free and accurately reflect the current status, attributes, and availability of units and requirements. 4. A global force management procedure for assessing combatant command requirements to determine viability, for sourcing, with respect to risk and prioritization between competing needs and the nature of the requirement.'"@en ;
    general:noun_exemplar "The Senate began a 15 minute roll call vote on [[confirmation]] of Executive Calendar #200 David Bernhardt, of Virginia, to be Secretary of the Interior."@en ;
    general:verb_exemplar "Nikkei, the Japanese media firm that owns the FT, has [[confirmed]] that it has acquired Singapore-based new media startup, Deal Street Asia."@en ;
    rdfs:subClassOf :Communication .

:Confiscation a owl:Class ;
    rdfs:label "Confiscation"@en ;
    rdfs:comment "Confiscation deals with taking an Actor's goods or property, based on some authority. The Actor whose goods/property are seized is defined by the event:has_affected_actor property."@en ;
    rdfs:subClassOf :ReductionRestrictionOrRemoval .
#   owl:equivalentClass oeevent:Confiscate_property .

:ConfiscationDamageOrDestruction a owl:Class ;
    rdfs:label "Confiscation, damage or destruction"@en ;
    rdfs:comment "Deals with either taking/seizure of, or the complete or partial loss of an Actor's goods or property. This class is used when the exact nature of the loss is unknown."@en ;
    rdfs:subClassOf :Event ;
    owl:equivalentClass [ a owl:Class ;
                          owl:unionOf ( :Confiscation :DamageOrDestruction ) ] .
# oeevent:Seize_or_damage_property rdfs:subClassOf :ConfiscationDamageOrDestuction .

:Confusion a owl:Class ;
    rdfs:label "Confusion"@en ;
    rdfs:comment "Confusion is an EmotionalResponse where an Actor is uncertain about a situation. If the situation is known, it can be associated using the event:has_topic property. The Actor is identified using the event:has_active_actor property."@en ;
    rdfs:subClassOf :EmotionalResponse .

:Congratulation a owl:Class ;
    rdfs:label "Congratulation"@en ;
    rdfs:comment "Congratulation is an acknoledgement from one Actor to another, that the latter has cause for celebration and/or that the former is pleased with the success of the latter."@en ;
    rdfs:subClassOf :CommunicationConveyingEmpathy .
#   owl:equivalentClass cco:ActOfCongratulating .

:ConservationLandUse a owl:Class ;
    rdfs:label "Conservation land use"@en ;
    rdfs:comment "ConservationLandUse describes how the land/environment is managed or modified in order to preserve its current state. It describes both specific acts, and general details/factors."@en ;
    rdfs:subClassOf :LandUse, :ProtectionOrPreservation .

:ConsiderationOrExploration a owl:Class ;
    rdfs:label "Consideration or exploration"@en ;
    rdfs:comment "ConsiderationOrExploration is an act of considering, exploring, studying, ... some idea or proposal, or set of ideas/proposals. The ideas/proposals are identified using the event:has_topic property."@en ;
    rdfs:subClassOf :Event .
#   owl:equivalentClass oeevent:Consider_policy_option .

:ConsumerSpending a owl:Class ;
    rdfs:label "Consumer spending (deprecated)"@en ;
    owl:deprecated "true"^^xsd:boolean ;
    rdfs:comment "An EconomicFactor providing data (typically, an individual meas:ReportedValue or meas:TimeSeries) on spending by a particular Actor, for a population or in a region. The Actor/population/group whose spending is reported is identified using the event:has_actor property, while the region is defined using general:located_at. The class may also be used to describe changes in spending (in which case, an individual is also typed as an event:Increase/Decrease/Stasis). Instances of type, Spending, may deal with specific artifacts that can be identified using the general:involves_goods_or_property predicate."@en ;
    rdfs:comment "Note that ConsumerSpending is deprecated in lieu of using its super-class, event:Spending."@en ;
    rdfs:subClassOf :Spending .

:Consumption a owl:Class ;
    rdfs:label "Consumption/consuming"@en ;
    rdfs:comment "Instances of type, Consumption, deal with specific artifacts (food, water, drugs, transportation, etc.) that should be identified using the general:involves_goods_or_property predicate."@en ;
    rdfs:subClassOf :Event .
#   owl:equivalentClass cco:ActOfConsumption .

:ContaminatedWater a owl:Class ;
    rdfs:label "Contaminated water"@en ;
    rdfs:comment "ContaminatedWater is both a type of EnvironmentalHazard as well as relevant to the general semantics of FoodWaterAndNutrition."@en ;
    rdfs:subClassOf :EnvironmentalHazard, :FoodWaterAndNutrition .

:Contempt a owl:Class ;
    rdfs:label "Contempt (deprecated)"@en ;
    owl:deprecated "true"^^xsd:boolean ;
    rdfs:comment "Contempt is an EmotionalResponse where an Actor is disrespectful toward, scorns, or is repulsed by another Actor, thing or situation. The Actor who is contemptful/disgusted is identified using the event:has_active_actor property. When the contempt/disgust is directed toward another Actor, that individual is identified using event:has_affected_actor. If the contempt/disgust is directed toward a thing (such as showing disrespect/contempt for a country's flag), the thing is identified using general:involves_goods_or_property. If the contempt/disgust is regarding a situation, that can be associated using the event:has_topic property."@en ;
    rdfs:comment "Note that Contempt is deprecated in lieu of using its super-class, event:ContemptOrDisgust."@en ;
    rdfs:subClassOf :ContemptOrDisgust .
# oeceo:Contempt rdfs:subClassOf :ContemptOrDisgust .

:ContemptOrDisgust a owl:Class ;
    rdfs:label "Contempt or disgust"@en ;
    rdfs:comment "ContemptOrDisgust is an EmotionalResponse where an Actor is disrespectful toward, scorns, or is repulsed by another Actor, thing or situation. The Actor who is contemptful/disgusted is identified using the event:has_active_actor property. When the contempt/disgust is directed toward another Actor, that individual is identified using event:has_affected_actor. If the contempt/disgust is directed toward a thing (such as showing disrespect/contempt for a country's flag), the thing is identified using general:involves_goods_or_property. If the contempt/disgust is regarding a situation, that can be associated using the event:has_topic property."@en ;
    rdfs:subClassOf :EmotionalResponse .
# oeceo:Contempt rdfs:subClassOf :ContemptOrDisgust .
# oeceo:Disgust rdfs:subClassOf :ContemptOrDisgust .

:Contentment a owl:Class ;
    rdfs:label "Contentment"@en ;
    rdfs:comment "Contentment is an EmotionalResponse where an Actor is (happy and) satisfied with their current situation. The Actor who is contented is identified using the event:has_active_actor property."@en ;
    rdfs:subClassOf :Happiness .
#   owl:equivalentClass oeceo:Contentment .

:ContractRelatedEvent a owl:Class ;
    rdfs:label "Contract-related event"@en ;
    rdfs:comment "Such as entering into or dissolving a legal contract"@en ;
    rdfs:subClassOf :FormalAgreement .

:Cooperation a owl:Class ;
    rdfs:label "Cooperation"@en ;
    rdfs:comment "Cooperation may describe either a specific event where two actors work together to achieve a goal, or a general environment of cooperation. The latter should also be classified as a type of event:Factor. Actors that cooperate are usually working together to achieve some objective. That objective/goal can be defined using the actor:has_objective property. The Actors that are cooperating are identified using the event:has_active_actor property."@en ;
    rdfs:subClassOf :EventOrFactor .

:Corruption a owl:Class ;
    rdfs:label "Corruption"@en ;
    rdfs:comment "Corruption is any act of dishonesty or lack of integrity, or a general environment that permits this. It can be a specific Event (such as a specific bribery event) or a state of affairs (such as government corruption). If the latter, then the individual can also be classified using event:Factor (or, for this example, more specifically, event:GovernmentalFactor)."@en ;
    rdfs:subClassOf :DefyingLawsNormsDirectives .

:Counteraction a owl:Class ;
    rdfs:label "Counteraction"@en ;
    rdfs:comment "An action taken in response. The original Event which promoted a response is defined using event:has_topic."@en ;
    general:noun_exemplar "Protesters planned a [[counteraction]] against the court injunctions intended to clear the streets."@en ;
    general:verb_exemplar "The administration deliberately intervened in the climate system to [[counteract]] global warming"@en ;
    rdfs:subClassOf :Event .

:CounterOperation a owl:Class ;
    rdfs:label "Counter-operation"@en ;
    rdfs:comment "A CounterOperation is a coordinated set of activities undertaken in response to another Actor's operation or to a threat. An Operation occurs over time, has specific goals/responds to specific threat(s), and is composed of specific, coordinated acts/Events intended to achieve those goals. The component Events (if known) are associated using the general:has_member property. The goal is identified using the actor:has_objective property."@en ;
    rdfs:subClassOf :Operation, :CounterAction .

:CounterTerrorismOperation a owl:Class ;
    rdfs:label "Counter terrorism operation"@en ;
    rdfs:comment "A coordinated set of activities undertaken in response to a terrorist threat. An Operation occurs over time, has specific goals/responds to specific threat(s), and is composed of specific, coordinated acts/Events intended to achieve those goals. The component Events (if known) are associated using the general:has_member property. The goal is identified using the actor:has_objective property. From JP1-02, counterterrorism is any 'activities and operations taken to neutralize terrorists and their organizations and networks in order to render them incapable of using violence to instill fear and coerce governments or societies to achieve their goals."@en ;
    rdfs:subClassOf :CounterOperation .

:CriminalAct a owl:Class ;
    rdfs:label "Criminal act"@en ;
    rdfs:comment "CriminalAct describes any act (or failure to perform an act) of evil or one which is punishable by law. Note that failure to perform an act is denoted using event:has_polarity and setting its value to event:Negative."@en ;
    rdfs:subClassOf :DefyingLawsNormsDirectives, event:Event .
#   owl:equivalentClass cco:CriminalAct .

:CriminalActOrCorruption a owl:Class ;
    rdfs:label "Criminal act or corruption"@en ;
    rdfs:comment "CriminalActOrCorruption describes any act (or failure to perform an act) of evil (which may or may not be punishable by law) or of dishonesty. Note that failure to perform an act is denoted using event:has_polarity and setting its value to event:Negative."@en ;
    rdfs:subClassOf :DefyingLawsNormsDirectives ;
    owl:equivalentClass [ a owl:Class ;
                          owl:unionOf ( :CriminalAct :Corruption ) ] .

:CropFailure a owl:Class ;
    rdfs:label "Crop failure"@en ;
    rdfs:comment "An EnvironmentalFactor related to insufficient crops to sustain persons/groups/a community or to provide a surplus to sell in order to acquire other necessities."@en ;
    general:noun_exemplar "The GEOGLAM Crop Monitor for Early Warning provides science-driven alerts for countries that may be in danger of [[low crop yields]]."@en ; 
    general:noun_exemplar "Farmers across northern and central Europe are facing [[crop failure]] and bankruptcy as one of the most intense regional droughts in recent memory strengthens its grip."@en ;
    general:verb_exemplar "Historically, when a [[crop failed]] in one of these breadbaskets, only nearby areas had to contend with shortages and rising prices."@en ;
    general:noun_exemplar "[[Harvest failures]], high food prices and hunger all shaped the course of the French Revolution, particularly for the working classes."@en ;
    rdfs:subClassOf :EnvironmentalFactor .

:CultureTransformationOrLoss a owl:Class ;
    rdfs:label "Culture transformation or loss"@en ;
    rdfs:comment "Cultures evolve for many reasons including immigration (the influx of new peoples and new cultural traits), because their traditions/language/... become unpopular or irrelevant, because the populations maintaining or practicing them die or move away, etc. This Factor describes the general condition of cultural evolution."@en ;
    rdfs:subClassOf :ArtsAndCulture .

:Curfew a owl:Class ;
    rdfs:label "Curfew"@en ;
    rdfs:comment "A Curfew is a regulation restricting the movement of people/requiring people to remain indoors between certain hours. The area or population that are under curfew are defined using the event:has_affected_actor and event:located_at properties."@en ;
    rdfs:subClassOf :ReductionRestrictionOrRemoval, :GoverningDirective .
#   owl:equivalentClass oeevent:Impose_curfew .

:Curiosity a owl:Class ;
    rdfs:label "Curiosity"@en ;
    rdfs:comment "Curiosity is an EmotionalResponse where an Actor desires to know something (or know more) about another Actor, a thing or a situation. If the curiosity is about a situation, that can be associated using the event:has_topic property. The Actor who is curious is identified using the event:has_active_actor property. If the curiosity is directed toward another Actor, that individual is identified using event:has_affected_actor. If the curiosity is about a thing, it is referenced using general:involves_goods_or_property."@en ;
    rdfs:subClassOf :EmotionalResponse .

:CyberAttack a owl:Class ;
    rdfs:label "Cyber attack"@en ;
    rdfs:comment "CyberAttack is defined as 'actions taken in cyberspace that create noticeable denial effects (i.e., degradation, disruption, or destruction) in cyberspace or manipulation that leads to denial that appears in a physical domain, and is considered a form of fires' (JP1-02). CyberAttacks are individual Events but may be part of an overall event:InformationOperation. This would be defined by including the attacks in the InformationOperation using the general:has_member property."@en ;
    rdfs:subClassOf :Attack, :InformationHandling .
#   owl:equivalentClass oeevent:Attack_cybernetically .

:CyberDefense a owl:Class ;
    rdfs:label "Cyber defense"@en ;
    rdfs:comment "CyberDefense is defined as 'actions taken within protected cyberspace to defeat specific threats that have breached or are threatening to breach cyberspace security measures and include actions to detect, characterize, counter, and mitigate threats, including malware or the unauthorized activities of users, and to restore the system to a secure configuration' (JP1-02). CyberDefense is typically a kind of, or a part of, an overall event:InformationOperation. The latter would be defined by including the defense operation in the overall InformationOperation using the general:has_member property."@en ;
    rdfs:subClassOf :InformationOperation .

:DamageOrDestruction a owl:Class ;
    rdfs:label "Damage or destruction"@en ;
    rdfs:comment "The type, DamageOrDestruction, is used to identify events that result in complete or partial loss in value of goods or property. This is distinct from a Factor such as StructuralDamage that describes an on-going condition in the environment. The thing that is destroyed is indicated using the general:involves_goods_or_property predicate."@en ;
    rdfs:subClassOf :Event .

:Death a owl:Class ;
    rdfs:label "Death"@en ;
    rdfs:comment "Death defines a specific life event. The individual that dies is best identified as the event:has_affected_actor, but in the case of multiple inheritance including event:Suicide, that individual is the active actor."@en ;
    rdfs:subClassOf :PersonalLifeEvent .
#   owl:equivalentClass cco:Death .

:Debt a owl:Class ;
    rdfs:label "Debt"@en ;
    rdfs:comment "An EconomicFactor providing data (typically, an individual meas:ReportedValue or meas:TimeSeries) on the debts incurred/carried by a GPE, for a population or in a region. The GPE/population/group whose debt is reported is identified using the event:has_actor property, while the region is defined using general:located_at."@en ;
    rdfs:subClassOf :EconomicFactor .

:Deception a owl:Class ;
    rdfs:label "Deception"@en ;
    rdfs:comment "An intentional action intended to deceive, cause harm or otherwise misrepresent something."@en ;
    rdfs:subClassOf :Event .
#   owl:equivalentClass cco:ActOfDeceptiveCommunication .

:DecisionOrRecommendation a owl:Class ;
    rdfs:label "Decision or recommendation"@en ;
    rdfs:comment "DecisionOrRecommendation is an act of concluding or resolving some issue or question. It may result from the debate and (eventual) agreement of multiple parties. This is distinct from the semantics of Advising which is a suggestion. The difference can also be seen in the super-classing of Advising versus DecisionOrRecommendation. The former sub-classes from DirectiveCommunication, while the this class sub-classes from DeclarativeCommunication."@en ;
    rdfs:subClassOf :DeclarativeCommunication .

:DeclarativeCommunication a owl:Class ;
    rdfs:label "Declarative communication"@en ;
    rdfs:comment "Deals with any type of 'declaration' such as accusations, claims/denials of responsibility, defending or supporting/disapproving or denouncing someone or something, vetoes, appraisals, reports, etc. (whether what is declared is 'true' or 'false' is not considered). When instantiating DeclarativeCommunication (or one of its sub-classes), it is important to indicate what are the topic(s) of the communication. This is accomplished using the event:has_affected_actor, event:has_topic or general:involves_goods_or_property object properties (referencing an Actor, an act/event or a thing, respectively). Examples of DeclarativeCommunication combined with using these properties include supporting a Person who might be accused of a crime (where the Person is related using event:has_affected_actor), denouncing an action/event that an Actor performed (where the event is defined using event:has_topic), or supporting something, such as supporting guns/firearms (where the 'thing' is specified using general:involves_goods_or_property). Note that releasing propaganda (an event:PropagandaActivity) is considered a type of event:DeclarativeCommunication and event:Deception."@en ;
    rdfs:subClassOf :Communication .
#   owl:equivalentClass cco:ActOfDeclarativeCommunication .
# cco:ActOfRepresentativeCommunication rdfs:subClassOf :DeclarativeCommunication .

:DeclineToComment a owl:Class ;
    rdfs:label "Decline to comment"@en ;
    rdfs:comment "A refusal to reply to a question typically asked by a journalist."@en ;
    rdfs:subClassOf :RefusalOrRejection .
#   owl:equivalentClass oeevent:Decline_comment .

:Decrease a owl:Class ;
    rdfs:label "Decrease"@en ;
    rdfs:comment "The class, Decrease, is used to record a decline/decrease in the availability/amount of a thing/artifact (such as a decrease in the amount of food, water or schooling), a decline/decrease in the number of people in certain roles (such as a decrease in the number of police or teachers), or decreases related to 'general' Events (such as a decrease in the number of MurderOrHomicide occurrences in a specific location) or Factors (such as a decrease in the Anger level in a community). If the decrease is related to another Event/Factor, the Decrease individual uses the event:has_topic property to reference that other Event. To identify a decrease in the availability/amount of something, the Decrease individual is related to the artifact using general:involves_goods_or_property. To identify a decrease in the number of people in certain roles, those people are defined as an individual that is a GroupOfPersons with a general:position_or_role property, and that entity is related to the Decrease via event:has_actor."@en ;
    rdfs:subClassOf :Change .

:Deescalation a owl:Class ;
    rdfs:label "De-escalation"@en ;
    rdfs:comment "Deescalation is a reduction in the intensity of a disagreement or conflict. If multiple Actors are involved in a Deescalation Event, all are identified as active actors."@en ;
    rdfs:subClassOf :ReductionRestrictionOrRemoval .

:DefenseOrSupport a owl:Class ;
    rdfs:label "Defense or support"@en ;
    rdfs:comment "DefenseOrSupport deals strictly with arguing in defense/support of a topic or Actor. When using this Event type, it is important to indicate who/what is being defended/supported. This is accomplished using the event:has_affected_actor, event:has_topic or general:involves_goods_or_property object properties (referencing a supported Actor, an act/event or a thing). Examples of DefenseOrSupport include supporting a Person who might be accused of a crime (where the Person is related using has_affected_actor), supporting an action/event that an Actor performed (where the event is defined using event:has_topic), or supporting a thing, such as supporting guns/firearms (where the thing is specified using general:involves_goods_or_property)."@en ;
    owl:disjointWith :LackOfSupport ;
    rdfs:subClassOf :DeclarativeCommunication .
# oeevent:Defend_verbally rdfs:subClassOf :DefenseOrSupport .

:DefensiveManeuver a owl:Class ;
    rdfs:label "Defensive maneuver"@en ;
    rdfs:comment "Any MilitaryAction taken to defend against or to deter aggression or attack."@en ;
    rdfs:subClassOf :MilitaryAction .

:DefyingLawsNormsDirectives a owl:Class ;
    rdfs:label "Defying laws, norms or directives"@en ;
    rdfs:comment "DefyingLawsNormsDirectives represents a range of activities (some of which may also be classified as CriminalActs) or general conditions. Therefore, it is sub-classed from event:EventOrFactor. When indicating a general condition/factor, an individual should also be classified as a type of event:Factor. Note that all acts of defiance are not necessarily criminal acts. For example, someone might burn their country's flag as a act of defiance - and it would be considered 'criminal' in some countries but not others. However, this semantic is about defiance more than criminality."@en ;
    rdfs:subClassOf :EventOrFactor .
#   owl:equivalentClass oeevent:Defy_norms\,_law .

:Demand a owl:Class ;
    rdfs:label "Demand"@en ;
    rdfs:comment "Demands are forcful requests. When using the Demand Event type, it is important to indicate what is being demanded and of whom. This is accomplished using the event:has_affected_actor, and event:has_topic object properties (referencing a supported Actor, and/or an act/event). Examples of Demand include demanding that a Person claim responsibility for an act/event (where the Person is the affected actor and the act/event is defined using event:has_topic), or demanding that an action/event be taken (where the event is defined using event:has_topic)."@en ;
    rdfs:subClassOf :RequestOrAppeal, :StrongOrIntense .
#   owl:equivalentClass oeevent:Demand .

:Demobilization a owl:Class ;
    rdfs:label "De-mobilization"@en ;
    rdfs:comment "From JP1-02, demobilization is '1. The process of transitioning a conflict or wartime military establishment and defense-based civilian economy to a peacetime configuration while maintaining national security and economic vitality. 2. The process necessary to release from active duty, or federal service, units and Reserve Component members who were ordered to active duty or called to federal service.' If multiple Actors are involved in a Demobilization Event, all are identified as active actors."@en ;
    rdfs:subClassOf :ReductionRestrictionOrRemoval .

:Democracy a owl:Class ;
    rdfs:label "Democracy"@en ;
    rdfs:comment "Democracy is a form of government where decision-making is by vote of the people, where the people vote directly on issues and/or vote for officials who make decisions on their behalf."@en ;
    rdfs:subClassOf :GovernmentalFactor .

:Demographic a owl:Class ;
    rdfs:label "Demographic"@en ;
    rdfs:comment "A Factor providing data (typically, an individual meas:ReportedValue or meas:TimeSeries) related to a population and/or particular groups within it. Sub-classes include semantics such as age or ethnicity demographics, information on births/fertility and mortality, etc. The population/group whose demographic is reported is identified using the event:has_actor property."@en ;
    rdfs:subClassOf :Factor .

:DemonstrationOrProtest a owl:Class ;
    rdfs:label "Demonstration or protest"@en ;
    rdfs:comment "A public gathering that is in support of or against some topic, thing or Actor. The topic, thing or Actor are identified using the event:has_topic, general:involves_goods_or_property or event:has_affected_actor properties, respectively."@en ;
    rdfs:subClassOf :MeetingOrEncounter .
#   rdfs:subClassOf oeevent:Demonstrate_or_rally .

:Denial a owl:Class ;
    rdfs:label "Denial"@en ;
    rdfs:comment "Deals with an Actor (the active actor) indicating that some Event or the existence of some Artifact is not true. Either an Event or an Artifact may be denied. These are specified using the event:has_topic and general:involves_goods_or_property, respectively."@en ;
    rdfs:subClassOf :DeclarativeCommunication .
#   owl:equivalentClass cco:ActOfDenying .

:DenialOfResponsibility a owl:Class ;
    rdfs:label "Denial of responsibility"@en ;
    rdfs:comment "Deals with an Actor (the active actor) indicating that they are NOT responsible for some Event. The Event for which responsibility is denied is specified using event:has_topic. Note that denying responsibility may not actually be a true statement."@en ;
    rdfs:subClassOf :Denial .
#   owl:equivalentClass oeevent:Reject_accusation\,_deny_responsibility .

:Departure a owl:Class ;
    rdfs:label "Departure"@en ;
    rdfs:comment "The act of leaving a destination. The destination is identified using the general:has_origin property."@en ;
    rdfs:subClassOf :LocationChange .
#   owl:equivalentClass cco:ActOfDeparture .

:Deployment a owl:Class ;
    rdfs:label "Deployment"@en ;
    rdfs:comment "Deployment is the act of bringing something or some Actor into use/into action. The thing or Actor that is deployed is defined using the event:involves_goods_or_property and event:has_affected_actor properties, respectively. Deployments can occur in business (releasing a new product or process), militarily (deploying troops or weapons), etc."@en ;
    rdfs:comment "From JP1-02, deployment is 'the movement of forces into and out of an operational area'."@en ;
    rdfs:subClassOf :Event .

:Deportation a owl:Class ;
    rdfs:label "Deportation"@en ;
    rdfs:comment "The act of expelling a person from a country. The country/GPE is typically defined as the active actor, while the deported person(s) are the affected actors. The persons' destination(s) may be specified using event:has_destination."@en ;
    rdfs:subClassOf :Expulsion .

:Desperation a owl:Class ;
    rdfs:label "Desperation"@en ;
    rdfs:comment "Desperation is an EmotionalResponse where an Actor has lost hope and may act recklessly. The Actor who is desperate is identified using the event:has_active_actor property."@en ;
    rdfs:subClassOf :EmotionalResponse .

:Deterrence a owl:Class ;
    rdfs:label "Deterrence/preventing"@en ;
    rdfs:comment "From JP1-02, Deterrence is 'the prevention of action by the existence of a credible threat of unacceptable counteraction and/or belief that the cost of action outweighs the perceived benefits'. Deterrence is a strategy that may be employed in business, military, social and other scenarios."@en ;
    general:noun_exemplar "[[Deterrence]] in the Gray Zone involves both preventing escalation to direct military conflict and assuaging an actor’s desire to violate international norms of behavior."@en ;
    general:verb_exemplar "A state seeking to [[deter]] should credibly threaten to impose negative consequences on a target if the same target does not comply with the action-avoidance request."@en ;
    rdfs:subClassOf :Event .

:DiplomaticCooperation a owl:Class ;
    rdfs:label "Diplomatic cooperation"@en ;
    rdfs:comment "DiplomaticCooperation may describe either a specific event where two actors work together to achieve a goal, or a general environment of diplomatic cooperation. The latter should also be classified as a type of event:Factor. A goal of the Cooperation can be defined using the actor:has_objective property. The Actors that are cooperating are identified using the event:has_active_actor property."@en ;
    rdfs:subClassOf :Cooperation .
#   owl:equivalentClass oeevent:Engage_in_diplomatic_cooperation .

:DiplomaticRecognition a owl:Class ;
    rdfs:label "Diplomatic recognition"@en ;
    rdfs:comment "DiplomaticRecognition is the acknowledgment of a country/GPE by another, or the acknowledgment/rejection of the actions of a country (such as the occupation of a territory outside of its boundaries)."@en ;
    rdfs:subClassOf :Event .
#   owl:equivalentClass oeevent:Grant_diplomatic_recognition .

:DiplomaticSanctions a owl:Class ;
    rdfs:label "Diplomatic sanctions"@en ;
    rdfs:comment "Diplomatic sanctions are the reduction or removal of diplomatic ties, such as by the closing of embassies or the recall of a diplomat."@en ;
    rdfs:subClassOf :Sanctions .

:DirectiveCommunication a owl:Class ;
    rdfs:label "Directive communication"@en ;
    rdfs:comment "Deals with advising, commanding, permitting/prohibiting or warning someone and/or about how to perform an action or reach a goal. The actor to which the communication is directed is the affected actor, while the action that is directed is another event (idenitified using event:has_topic property)."@en ;
    rdfs:subClassOf :Communication .
#   owl:equivalentClass cco:ActOfDirectiveCommunication .

:DisabilityDemographic a owl:Class ;
    rdfs:label "Disability demographic"@en ;
    rdfs:comment "A Factor providing data (typically, an individual meas:ReportedValue or meas:TimeSeries) about the disabilities observed in a population or its sub-groups. The population/group whose demographic is reported is identified using the event:has_actor property."@en ;
    rdfs:subClassOf :Demographic .

:DisagreementOrDispute a owl:Class ;
    rdfs:label "Disagreement or dispute"@en ;
    rdfs:comment "DisagreementOrDispute characterizes any act where two or more Actors do NOT share the same opinion or thoughts. When using the DisagreementOrDispute Event type, it is important to indicate what is the subject of the disagreement and who are the Actors involved. This is accomplished using the event:has_active_actor and event:has_topic object properties."@en ;
    rdfs:subClassOf :Event .

:DisapprovalOrDenunciation a owl:Class ;
    rdfs:label "Disapproval or denunciation"@en ;
    rdfs:comment "Examples of DisapprovalOrDenunciation include denouncing a Person who might be accused of a crime or of a certain ethnicity (where the Person is related using event:has_affected_actor), denouncing an action/event that an Actor performed (where the event is defined using event:has_topic), or denouncing a thing, such as denouncing guns/firearms (where the thing is specified using general:involves_goods_or_property). When using the DisapprovalOrDenunciation Event type, it is important to indicate what is being denounced. This is accomplished using the event:has_affected_actor, event:has_topic or general:involves_goods_or_property object properties (referencing an Actor, an act/event or a thing, respectively)."@en ;
    rdfs:subClassOf :DeclarativeCommunication .
#   owl:equivalentClass oeevent:Criticize_or_denounce .

:Disgust a owl:Class ;
    rdfs:label "Disgust (deprecated)"@en ;
    owl:deprecated "true"^^xsd:boolean ;
    rdfs:comment "Disgust is an EmotionalResponse where an Actor is disrespectful toward, scorns, or is repulsed by another Actor, thing or situation. The Actor who is contemptful/disgusted is identified using the event:has_active_actor property. When the contempt/disgust is directed toward another Actor, that individual is identified using event:has_affected_actor. If the contempt/disgust is directed toward a thing (such as showing disrespect/contempt for a country's flag), the thing is identified using general:involves_goods_or_property. If the contempt/disgust is regarding a situation, that can be associated using the event:has_topic property."@en ;
    rdfs:comment "Note that Disgust is deprecated in lieu of using its super-class, event:ContemptOrDisgust."@en ;
    rdfs:subClassOf :ContemptOrDisgust .
# oeceo:Disgust rdfs:subClassOf :ContemptOrDisgust .

:DisinformationOperation a owl:Class ;
    rdfs:label "Disinformation operation"@en ;
    rdfs:comment "A DisinformationOperation involves the release of false information with the intent of misleading or deceiving some Actors. An Operation occurs over time, has specific goals, and is composed of specific, coordinated acts/Events intended to achieve those goals. The component Events (if known) are associated using the general:has_member property. The goal is identified using the actor:has_objective property."@en; 
    rdfs:subClassOf :MisinformationOperation, :Deception, :Influence .

:Distrust a owl:Class ;
    rdfs:label "Distrust (deprecated)"@en ;
    owl:deprecated "true"^^xsd:boolean ;
    rdfs:comment "Distrust is an EmotionalResponse where an Actor has misgivings about someone or something. The Actor who is distrustful/suspicious is identified using the event:has_active_actor property. When the distrust/suspicion is directed toward another Actor, that individual is identified using event:has_affected_actor. If the distrust/suspicion is directed toward a thing (such as doubting a car's brakes/braking ability), the artifact is identified using general:involves_goods_or_property."@en ;
    rdfs:comment "Note that Distrust has been deprecated in lieu of using its super-class, DistrustOrSuspicion."@en ;
    rdfs:subClassOf :DistrustOrSuspicion .

:DistrustOrSuspicion a owl:Class ;
    rdfs:label "Distrust or suspicion"@en ;
    rdfs:comment "DistrustOrSuspicion is an EmotionalResponse where an Actor has misgivings about someone or something. The Actor who is distrustful/suspicious is identified using the event:has_active_actor property. When the distrust/suspicion is directed toward another Actor, that individual is identified using event:has_affected_actor. If the distrust/suspicion is directed toward a thing (such as doubting a car's brakes/braking ability), the artifact is identified using general:involves_goods_or_property."@en ;
    rdfs:subClassOf :EmotionalResponse .

:DomesticTrade a owl:Class ;
    rdfs:label "Domestic trade"@en ;
    rdfs:comment "An EconomicFactor providing data (typically, an individual meas:ReportedValue or meas:TimeSeries) on internal/domestic trade for a population or in a region. The population/group whose trade is reported is identified using the event:has_actor property, while the region is defined using general:located_at."@en ;
    rdfs:subClassOf :EconomicFactor .

:Donation a owl:Class ;
    rdfs:label "Donation"@en ;
    rdfs:comment "A Donation is a gift of goods, monies, services, etc. to some Actor (the affected actor)."@en ;
    rdfs:subClassOf :Event .

:Drought a owl:Class ;
    rdfs:label "Drought"@en ;
    rdfs:comment "A Drought is a (significant) period of time without rainfall, leading to a water shortage."@en ;
    rdfs:subClassOf :WeatherIssue, :WaterInsecurity, :NaturalDisaster .

:DrugTrade a owl:Class ;
    rdfs:label "Drug trade"@en ;
    rdfs:comment "DrugTrade or drug trafficking is a black market activity related to the growing/producing and distributing/selling/purchasing of controlled substances and/or medicines."@en ;
    rdfs:subClassOf :BlackMarketTrade .

:EarthquakeAndAftershock a owl:Class ;
    rdfs:label "Earthquake and/or aftershock(s)"@en ;
    rdfs:comment "A NaturalDisaster related to the movement of the earth's crust or due to volcanic activity."@en ;
    rdfs:subClassOf :NaturalDisaster .

:EconomicCondition a owl:Class ;
    rdfs:label "Economic condition"@en ;
    rdfs:comment "A super-class for a variety of characterizations of the economy of a population or in a region. Sub-classes of EconomicCondition are EconomicDepression/Recession/Growth/Equality/Inequality/Inflation and Poverty. The population/group whose economy is reported is identified using the event:has_actor property, while the region is defined using general:located_at. If this type is used to classify a statistics, then the meas:ReportedValue or meas:TimeSeries types should also be added."@en ;
    rdfs:subClassOf :EconomicFactor .

:EconomicCooperation a owl:Class ;
    rdfs:label "Economic cooperation"@en ;
    rdfs:comment "EconomicCooperation may describe either a specific event where two actors work together to achieve a goal, or a general environment of economic cooperation. The latter should also be classified as a type of event:EconomicFactor. A goal of the Cooperation can be defined using the actor:has_objective property. The Actors that are cooperating are identified using the event:has_active_actor property."@en ;
    rdfs:subClassOf :Cooperation .
#   owl:equivalentClass oeevent:Cooperate_economically .

:EconomicDepression a owl:Class ;
    rdfs:label "Depression (economic)"@en ;
    rdfs:comment "An EconomicCondition describing that the economy for a population or in a region is contracting/in a depression (as opposed to event:EconomicGrowth). The population/group whose economy is reported is identified using the event:has_actor property, while the region is defined using general:located_at."@en ;
    rdfs:subClassOf :EconomicCondition .

:EconomicDevelopment a owl:Class ;
    rdfs:label "Economic development"@en ;
    rdfs:comment "Any specific Events or EconomicFactors related to improving the economic and social environment of a population or in a region. The population/group whose economy is described is identified using the event:has_actor property, while the region is defined using general:located_at."@en ;
    rdfs:subClassOf :EconomicFactor, :ExpansionOrDevelopment .

:EconomicEquality a owl:Class ;
    rdfs:label "Economic equality"@en ;
    rdfs:comment "EconomicCondition describing equal distributions of incomes and opportunities in an area or for a population."@en ;
    owl:disjointWith :EconomicInequality ;
    rdfs:subClassOf :EconomicCondition .

:EconomicFactor a owl:Class ;
    rdfs:label "Economic factor"@en ;
    rdfs:comment "Deals with any aspect of the economic environment. Sub-classes address the specific semantics of consumer spending, trade (including trade on the black market), trade balance, conditions (such as debt, economic inequality, inflation, etc.), economic development, sanctions, economic secrecy or transparency, employment, import/expert, GDP/GNI, pricing, productivity, revenue, spending, wages and much more. These semantics may be related to a specific event, or to general conditions/factors/statistics. When defining general conditions or statistics, an individual should also be classified using event:Factor, meas:ReportedValue or meas:TimeSeries."@en ;
    rdfs:comment "(From the Army War College Command Post Exercise) EconomicFactors encompass individual and group behaviors related to producing, distributing, and consuming resources. In terms of DIME-FIL, it involves the creation and enforcement of trade, fiscal and monetary policies, the implementation of sanctions, embargoes or tariffs, provision of economic/financial assistance, etc."@en ;
    rdfs:subClassOf :EventOrFactor .

:EconomicGrowth a owl:Class ;
    rdfs:label "Economic growth"@en ;
    rdfs:comment "An EconomicFactor describing that the economy for a population or in a region is expanding (as opposed to event:EconomicRecession/Depression). The population/group whose economy is reported is identified using the event:has_actor property, while the region is defined using general:located_at."@en ;
    general:noun_exemplar "[[Economic growth]] occurs whenever people take resources and rearrange them in ways that are more valuable."@en ;
    general:noun_exemplar "A [[growing economy]] consumes natural resources and produces wastes."@en ;
    general:verb_exemplar "The U.S. [[economy grew]] at a faster pace than expected in the first quarter and posted its best growth to start a year in four years."@en ;
    rdfs:subClassOf :EconomicFactor, :ExpansionOrDevelopment .

:EconomicInequality a owl:Class ;
    rdfs:label "Economic inequality"@en ;
    rdfs:comment "EconomicCondition describing unequal distributions of incomes and opportunities in an area or for a population."@en ;
    rdfs:subClassOf :EconomicCondition .

:EconomicInflation a owl:Class ;
    rdfs:label "Inflation (economic)"@en ;
    rdfs:comment "In economics, inflation is related to a general increase in prices (usually due to a decrease in the purchasing power of a country's currency."@en ;
    rdfs:subClassOf :EconomicCondition .

:EconomicOpportunity a owl:Class ;
    rdfs:label "Economic opportunity"@en ;
    rdfs:comment "EconomicOpportunity may describe either a specific event where an Actor gains some advantage from selling/buying/leasing/... something, or a general environment of economic advantage. If the latter, then the individual should also be classified using event:Factor."@en ;
    rdfs:subClassOf :EconomicFactor .

:EconomicRecession a owl:Class ;
    rdfs:label "Recession (economic)"@en ;
    rdfs:comment "An EconomicCondition describing that the economy for a population or in a region is contracting/in a recession (as opposed to event:EconomicGrowth). The population/group whose economy is reported is identified using the event:has_actor property, while the region is defined using general:located_at."@en ;
    rdfs:subClassOf :EconomicCondition .

:EconomicSanctions a owl:Class ;
    rdfs:label "Economic sanctions"@en ;
    rdfs:comment "Economic sanctions are typically expressed as a ban on trade between countries, which may be limited to certain goods or apply to all goods (with certain exceptions)."@en ; 
    rdfs:subClassOf :Sanctions, :EconomicFactor .

:EconomicSecrecy a owl:Class ;
    rdfs:label "Economic secrecy"@en ;
    rdfs:comment "EconomicSecrecy is obfuscation, and lack of accountability and openness regarding economic activities and conditions."@en ;
    owl:disjointWith :EconomicTransparency ;
    rdfs:subClassOf :Secrecy, :EconomicFactor .

:EconomicTransparency a owl:Class ;
    rdfs:label "Economic transparency"@en ;
    rdfs:comment "EconomicTransparency is clarity, lack of obfuscation, accountability and openness regarding economic activities and conditions."@en ;
    rdfs:subClassOf :Transparency, :EconomicFactor .

:EducationAndTraining a owl:Class ;
    rdfs:label "Education and training"@en ;
    rdfs:comment "Semantics describing or affecting teaching and learning of a population or in a region. EducationAndTraining may describe specific events (such as the hiring of teachers or a new approach to testing students' knowledge), general conditions such as an increase/decrease in school attendance in a population/region (event:Increase/Decrease/Stasis), or statistics (an individual meas:ReportedValue or meas:TimeSeries) related to education and training. Because the semantics can address either events or conditions/factors, it is defined as a subclass of event:EventOrFactor."@en ;
    rdfs:subClassOf :EventOrFactor .

:Election a owl:Class ;
    rdfs:label "Election"@en ;
    rdfs:comment "Election is the process of choosing someone for a position (which may be a political office, but is not necessarily so - e.g., 'John was elected to be the jury foreman'). This is distinct from Voting, which is meant to address both voting for/against a candidate or on an issue. Although voting is a part of an election, it is defined to distinguish between an individual voting/going to vote, and (for example) Trump and Clinton running two ElectionCampaigns in the 2016 Presidential Election."@en ;
    rdfs:subClassOf :Event .
#   owl:equivalentClass cco:Election .

:ElectionCampaign a owl:Class ;
    rdfs:label "Election campaign"@en ;
    rdfs:comment "An organized effort by a candidate to influence the outcome of an Election. An Operation occurs over time, has specific goals (for a candidate to be elected or for a law/directive to be passed/rejected), and is composed of specific, coordinated acts/Events intended to achieve those goals. The component Events (if known) are associated using the general:has_member property. The goal is identified using the actor:has_objective property."@en ;
    rdfs:subClassOf :Operation .

:ElectromagneticActivity a owl:Class ;
    rdfs:label "Electromagnetic activity"@en ;
    rdfs:comment "Activity involving the use of electromagnetic theory and directed energy to control communications and the electromagnetic spectrum in general, and/or to disrupt the communications and infrastructure of an enemy. This includes jamming, hardening and signal detection activities."@en ;
    rdfs:subClassOf :InformationHandling .

:ElectromagneticRadiationHazard a owl:Class ;
    rdfs:label "Electromagnetic radiation hazard"@en ;
    rdfs:comment "A sub-class of EnvironmentalHazard defined by JP1-02 as 'transmitter or antenna installation that generates or increases electromagnetic radiation in the vicinity of ordnance, personnel, or fueling operations in excess of established safe levels'."@en ; 
    general:noun_exemplar "The US government standard, Federal Standard 1037C defines EMF caution as [[Electromagnetic Radiation Hazards]] (RADHAZ or EMR hazards)."@en ;
    general:noun_exemplar "[[EMR hazards]], sometimes referred to as [[RADHAZ]], exist whenever there is an electromagnetic field of sufficient intensity to cause personnel injury, ignition of explosives/fuels/material, or disruption of electronics."@en ;
    rdfs:subClassOf :EnvironmentalHazard .

:Employment a owl:Class ;
    rdfs:label "Employment"@en ;
    rdfs:comment "Employment generally describes specific events (such as the hiring of a new CXX officer or the hiring or lay off of personnel), a general condition/factor describing the increase/decrease of employment (event:Increase/Decrease/Stasis) for a population or in a region, or statistics (individual meas:ReportedValues or meas:TimeSeries) related to employment numbers. Because the semantics can address either events or conditions/factors, Employment is defined as a subclass of event:EventOrFactor."@en ;
    rdfs:subClassOf :EventOrFactor .

:EmploymentRelatedEvent a owl:Class ;
    rdfs:label "Employment-related event (deprecated)"@en ;
    owl:deprecated "true"^^xsd:boolean ;
    rdfs:comment "EmploymentRelatedEvents include events such as a company announcing the hiring of a new CXX officer, the hiring or lay off of personnel, the intention to raise/lower wages, etc."@en ;
    rdfs:comment "Note that EmploymentRelatedEvent is deprecated in lieu of using its super-class, Employment."@en ;
    rdfs:subClassOf :Employment .

:EnergyRelatedFactor a owl:Class ;
    rdfs:label "Energy related factor"@en ;
    rdfs:comment "Energy related factors deal with the various aspects of production/supply, consumption/demand, inventory, distribution and transport for electricity, fuels, solar or wind power, etc., where the latter are associated via general:involves_goods_or_property. EnergyRelatedFactor describes a general condition/factor indicating the increase/decrease of available energy/produced materials for a population or in a region (event:Increase/Decrease/Stasis), or statistics (an individual meas:ReportedValue or meas:TimeSeries) related to energy production/generation/..."@en ;
    rdfs:subClassOf :Factor .

:EntertainmentEvent a owl:Class ;
    rdfs:label "Entertainment event"@en ;
    rdfs:comment "Examples of EntertainmentEvent are a sporting events/competitions, performances, etc."@en ;
    rdfs:subClassOf :Event .

:EnvironmentalFactor a owl:Class ;
    rdfs:label "Environmental factor"@en ;
    rdfs:comment "EnvironmentalFactors address geography and man-made structures as well as the climate, weather and conditions in an area. Sub-classes of EnvironmentalFactor include EnvironmentalProtection, NaturalDisasters, NaturalResources and WeatherIssue, among others. Individuals can represent specific events or general conditions/factors/statistics. When defining general conditions or statistics, an individual should also be classified using event:Factor, meas:ReportedValue or meas:TimeSeries."@en ;
    rdfs:subClassOf :EventOrFactor .

:EnvironmentalHazard a owl:Class ;
    rdfs:label "Environmental hazard"@en ;
    rdfs:comment "EnvironmentalHazards are substances or conditions 'with the potential to cause injury, illness, or death of personnel; damage to or loss of equipment or property; or mission degradation'. The 'adverse effects [could be] due to an accidental or deliberate release and dissemination' (JP1-02). Sub-classes are defined reflecting key concepts in JP1-02 (Biological/Chemical/ElectromagneticRadiation/Explosive/Nuclear/RadiologicalHazard) as well as Pollution."@en ; 
    general:noun_exemplar "We are especially committed to protecting the health of those most vulnerable to certain [[environmental hazards]] — children, the elderly, and people with chronic health conditions."@en ;
    rdfs:subClassOf :EnvironmentalFactor .

:EnvironmentalProtection a owl:Class ;
    rdfs:label "Environmental protection"@en ;
    rdfs:comment "EnvironmentalProtection deals with activities where Actors conserve or repair an area, or address an issue such as pollution or deforestation."@en ;
    rdfs:subClassOf :Event, :EnvironmentalFactor, :ProtectionOrPreservation .

:Escape a owl:Class ;
    rdfs:label "Escape"@en ;
    rdfs:comment "Events dealing with an entity getting free, who has been physically captured/detained."@en ; 
    rdfs:subClassOf :Event .

:EspionageOperation a owl:Class ;
    rdfs:label "Espionage operation"@en ;
    rdfs:comment "An Operation occurs over time, has specific goals, and is composed of specific, coordinated acts/Events intended to achieve those goals. The component Events (if known) are associated using the general:has_member property. The goal is identified using the actor:has_objective property. An example of an EspionageOperation is a set of coordinated activities to infiltrate a terrorist cell. This is distinct from an EspionageOrTreason Event, which is an act perpetrated by someone. Note that an individual EspionageOrTreason Event may indeed be part of an EspionageOperation."@en ;
    rdfs:subClassOf :Operation .

:EspionageOrTreason a owl:Class ;
    rdfs:label "Espionage or treason"@en ;
    rdfs:comment "EspionageOrTreason addresses both the act of spying/illicitly obtaining information and formal acts of treason against one's country. According the US Constitution, Article 3, 'Treason against the United States, shall consist only in levying War against them [the States], or in adhering to their Enemies, giving them Aid and Comfort. No Person shall be convicted of Treason unless on the Testimony of two Witnesses to the same overt Act, or on Confession in open Court.'"@en ;
    rdfs:subClassOf :Event .
#   owl:equivalentClass cco:ActOfEspionage .

:EthnicCleansing a owl:Class ;
    rdfs:label "Ethnic cleansing"@en ;
    rdfs:comment "A United Nations Commission of Experts (mandated to look into violations of international humanitarian law committed in the territory of the former Yugoslavia) defined ethnic cleansing in its interim report S/25274 and final report S/1994/674. It is described as 'a purposeful policy designed by one ethnic or religious group to remove by violent and terror-inspiring means the civilian population of another ethnic or religious group from certain geographic areas.' EthnicCleansing crosses the semantics of MurderOrHomicide, ForcedMove and Imprisonment."@en ;
    rdfs:subClassOf :Event ;
    owl:equivalentClass [ a owl:Class; 
                          owl:unionOf ( :MurderOrHomicide :ForcedMove :Imprisonment ) ] .
#   owl:equivalentClass oeevent:Engage_in_ethnic_cleansing .

:EthnicityDemographic a owl:Class ;
    rdfs:label "Ethnicity demographic"@en ;
    rdfs:comment "A Factor providing data (typically, an individual meas:ReportedValue or meas:TimeSeries) about the ethnic characteristics of/ethnicities observed in a population or its sub-groups. The population/group whose demographic is reported is identified using the event:has_actor property."@en ;
    rdfs:subClassOf :Demographic .

:Evacuation a owl:Class ;
    rdfs:label "Evacuation"@en ;
    rdfs:comment "From JP1-02, Evacuation is '1. Removal of a patient by any of a variety of transport means from a [location]/theater of military operation, or between health services capabilities, for the purpose of preventing further illness or injury, providing additional care, or providing disposition of patients from the ... health care system. 2. The clearance of personnel, animals, or materiel from a given locality. 3. The controlled process of collecting, classifying, and shipping unserviceable or abandoned materiel, United States or foreign, to appropriate reclamation, maintenance, technical intelligence, or disposal facilities. 4. The ordered or authorized departure of ... evacuees from a specific area to another in the same or different countries.'"@en ;
    rdfs:subClassOf :ForcedMove .

:EvaluationOrAppraisal a owl:Class ;
    rdfs:label "Evaluation or appraisal"@en ;
    rdfs:comment "Examples of EvaluationOrAppraisal include evaluating a Person in a position (where the Person is the affected actor and their general:position_or_role property is evaluated), evaluating the performance of the active actor in an action/event (where the event is defined using event:has_topic), or evaluating a thing, such as appraising a building/facility (where the thing is specified using general:involves_goods_or_property). When using the EvaluationOrAppraisal Event type, it is important to indicate who/what is being evaluated. This is accomplished using the event:has_affected_actor, event:has_topic or general:involves_goods_or_property object properties (referencing an Actor, an act/event or a thing, respectively)."@en ;
    rdfs:subClassOf :DeclarativeCommunication .
#   owl:equivalentClass cco:ActOfAppraisal .

:Excess a owl:Class ;
    rdfs:label "Excess/abundance of supply"@en ;
    rdfs:comment "There can be excesses of things/artifacts (such as an excess of food or fuel), excesses of services or people in certain roles (such as an excess of teachers or homeless), or excesses related to different Factors (such as an excess of violence). The details of the first (excesses of things) are described by an Excess individual that references the thing/artifact (for example, food in general or a particular type of food such as potatoes, fuel, water, etc.) using the general:involves_goods_or_property object property. The details of the second (excesses of people in roles) are described by an Excess individual that references a GroupOfPersons using the event:has_actor property with their role defined using the general:position_or_role property. The details of the third (excesses of Factors) are described by an Excess event that references the Factor using the event:has_topic property."@en ;
    rdfs:subClassOf :Factor .

:Execution a owl:Class ;
    rdfs:label "Execution"@en ;
    rdfs:comment "Carrying out a death sentence against a person (the affected actor). A 'death sentence' is a form of legal sentencing/penalty."@en ;
    rdfs:subClassOf :Death, :LegalSentence .

:ExecutiveGovernmentActivity a owl:Class ;
    rdfs:label "Executive government activity"@en ;
    rdfs:comment "ExecutiveGovernmentActivities deal with the operation of the executive/ruling branch of a government and activities undertaken by the government leaders. These activities include veteos, nominations, issuance of orders, directives and reports, etc. They may also be characterized by other classes, such as event:IntimidationAndCoercion or event:Corruption."@en ;
    rdfs:subClassOf :GovernmentActivity .

:ExhibitionOfPower a owl:Class ;
    rdfs:label "Exhibition of power"@en ;
    rdfs:comment "An ExhibitionOfPower is any act that demonstrates the authority and/or capabilities of a group, but that does not include the use of force. Examples include military build-ups near disputed territories, military or police maneuvers to demonstrate preparedness, openly carrying weapons, etc. Note that the actor involved in the Event defines whether this is an exhibition of military or police power, or of the capabilities of a terrorist organization, for example."@en ;
    rdfs:subClassOf :IntimidationAndCoercion .
# oeevent:Exhibit_military_or_police_power rdfs:subClassOf :ExhibitionOfPower .

:ExpansionOrDevelopment a owl:Class ;
    rdfs:label "Expansion or development"@en ;
    rdfs:comment "ExpansionOrDevelopment is concerned with activites/new developments designed to increase (something) in size/quantity/quality/volume/scope/etc. The thing that is 'increased' is identified using either the event:has_affected_actor, general:involves_goods_or_property or event:has_topic properties. For example, expanding the size of a military force uses has_affected_actor, increasing the storage capacity of a facility uses involves_goods_or_property, and increasing the scope of an investigation uses has_topic."@en ;
    owl:disjointWith :ReductionRestrictionOrWithdrawal ;
    rdfs:subClassOf :Event .

:ExperimentOrTest a owl:Class ;
    rdfs:label "Experiment or test"@en ;
    rdfs:comment "An ExperimentOrTest involves trying something in order to learn about it. Examples include missile tests, drug experiments or trials, etc. Note that the 'thing' that is tried is indicated using the event:has_instrument or event:has_topic properties - conveying that either an Artifact (such as a new missile or drug) is tested, or that a process/emotion/action is tested. An example of the latter would be performing a small demonstration of power (an event:ExhibitionOfPower) to gauge reaction."@en ;
    general:verb_exemplar "North Korea said on Thursday that it [[tested]] a new type of 'tactical guided weapon,' in what appeared to be a warning from Kim Jong-un to President Trump."@en ;
    general:noun_exemplar "The missile [[test]] was the North’s first since 2017."@en ;
    general:noun_exemplar "A clinical [[trial]] to evaluate long-acting antiretroviral therapy for maintaining HIV suppression has begun at research sites across the United States."@en ;
    general:noun_exemplar "Nuclear weapons [[tests]] are [[experiments]] carried out to determine the effectiveness, yield, and explosive capability of nuclear weapons."@en ;
    general:noun_exemplar "Farm animals used in agricultural [[experimentation]] are explicitly excluded from the law's definition of 'animal'."@en ;
    general:verb_exemplar "More than 100,000 monkeys are [[experimented]] on in the United States."@en ;
    rdfs:subClassOf :Event .

:ExploitationOfNaturalResources a owl:Class ;
    rdfs:label "Exploitation of natural resoures"@en ;
    rdfs:comment "The ExploitationOfNaturalResources class deals with any acts that involve obtaining, processing or using the materials in the natural environment. This includes drilling, mining, harvesting forests, irrigation projects, refining fuels, etc."@en ;
    rdfs:subClassOf :Event, :NaturalResources .

:ExploratoryCommunication a owl:Class ;
    rdfs:label "Exploratory communication (such as negotiations and interviews)"@en ;
    rdfs:comment "Deals with communicating to better understand someone or something (for example via an interview), questioning or investigating (including investigating alternatives such as in a negotiation). When instantiating ExploratoryCommunication (or one of its sub-classes), it is important to indicate who is involved in the communication and what is being negotiated/questioned/explored. This is accomplished using the event:has_active_actor and event:has_topic object properties, respectively."@en ;
    rdfs:subClassOf :Communication .

:ExplosiveHazard a owl:Class ;
    rdfs:label "Explosive hazard"@en ;
    rdfs:comment "A sub-class of EnvironmentalHazard defined by JP1-02 as '1. Any material posing a potential threat that contains an explosive component such as unexploded explosive ordnance, booby traps, improvised explosive devices, captured enemy ammunition, and bulk explosives. 2. In explosive ordnance disposal, a condition where danger exists because explosives are present that may react in a mishap with potential unacceptable effects to people, property, operational capability, or the environment.'"@en ; 
    general:noun_exemplar "U.S.-Funded [[explosive hazard]] risk education programs improve safety and human security across Iraq."@en ;
    general:noun_exemplar "Workers must be protected from combustible dust flash fire and [[explosion hazards]]."@en ;
    rdfs:subClassOf :EnvironmentalHazard .

:Export a owl:Class ;
    rdfs:label "Export"@en ;
    rdfs:comment "Export deals with any conditions favorable/disfavorable to sending goods or services to another country, or various statistics (an individual meas:ReportedValue or meas:TimeSeries) related to exports. Factors which influence export include their availability, trade policies, exchange rates and demand, among others."@en ;
    rdfs:subClassOf :EconomicFactor .

:ExpressionOfCondolenceOrSympathy a owl:Class ;
    rdfs:label "Expression of condolence or sympathy"@en ;
    rdfs:comment "ExpressionOfCondolenceOrSympathy is empathy with another's grief. The Actor expressing the emotion is defined as the active actor, while the one with whom they empathize is the affected actor. If the emotion concerns an event/factor, that can be referenced using the event:has_topic property."@en ;
    rdfs:subClassOf :CommunicationConveyingEmpathy .
#   owl:equivalentClass cco:ActOfCondoling .

:ExpressionOfIntent a owl:Class ;
    rdfs:label "Expression of intent"@en ;
    rdfs:comment "ExpressionOfIntent is a type of CommissiveCommunication indicating how an Actor plans to do/accomplish something. When using the ExpressionOfIntent Event type, it is important to indicate what is being stated as intended and to whom (if known/applicable). This is accomplished using the event:has_topic and event:has_affected_actor object properties."@en ;
    rdfs:subClassOf :CommissiveCommunication .

:Expulsion a owl:Class ;
    rdfs:label "Expulsion"@en ;
    rdfs:comment "Expulsion deals with forcing an individual to leave a place or organization. Note that specific sub-classes are not defined (for example, expulsion of peacekeepers or aid agencies). Instead, this semantic can be expressed as an Expulsion Event, where the Event's affected actor conveys the details concerning the Person(s), Group(s) or Organization(s) expelled. The details of the Actor's type could define it as an actor:AidOrReliefOrganization, and the Actor's general:position_or_role property could indicate their function or role (e.g., 'https://en.wikipedia.org/wiki/Peacekeeping', 'https://en.wikipedia.org/wiki/Inspection', 'https://en.wikipedia.org/wiki/Observer', 'https://en.wikipedia.org/wiki/President_(corporate_title)', etc.)."@en ;
    rdfs:subClassOf :ForcedMove, :Withdrawal .

:ExpulsionDeportationOrWithdrawal a owl:Class ;
    rdfs:label "Expulsion, deportation or withdrawal (deprecated)"@en ;
    owl:deprecated "true"^^xsd:boolean ;
    rdfs:comment "Deals with either the expulsion (or more specific deportation) or the forced or voluntary withdrawal of Actors from a country or organization. It is recommended that this class NOT be used (it is deprecated). The more general class, event:Withdrawal, should be used if the reason for the move is unknown. Otherwise, the more specific classes, Expulsion or Deportation, should be used. Note that Deportation is a sub-class of Expulsion (hence, Expulsion is more general and can be used if it is unknown if an expulsion or deportation occurred)."@en ;
    rdfs:subClassOf :ReductionRestrictionOrRemoval ;
    owl:equivalentClass [ a owl:Class ;
                          owl:unionOf ( :Deportation :Expulsion :Withdrawal ) ] .
# oeevent:Expel_or_withdraw rdfs:subClassOf :ExpulsionDeportationOrWithdrawal .
# oeevent:Expel_or_deport_individuals rdfs:subClassOf :ExpulsionDeportationOrWithdrawal .

:Extradition a owl:Class ;
    rdfs:label "Extradition"@en ;
    rdfs:comment "Extradition is 'an act where one jurisdiction delivers a person accused or convicted of committing a crime in another jurisdiction, over to their law enforcement. It is a cooperative law enforcement process between the two jurisdictions and depends on the arrangements made between them.' (https://en.wikipedia.org/wiki/Extradition)"@en ;
    rdfs:subClassOf :ForcedMove, :JudicialGovernmentActivity, :JudicialCooperation .

:ExtraJudicialExecution a owl:Class ;
    rdfs:label "Extra-judicial execution"@en ;
    rdfs:comment "The 'killing of a person [or persons] by governmental authorities or individuals without the sanction of any judicial proceeding or legal process' (https://en.wikipedia.org/wiki/Extrajudicial_killing)."@en ;
    rdfs:subClassOf :MurderOrHomicide .

:Famine a owl:Class ;
    rdfs:label "Famine"@en ;
    rdfs:comment "Famine is the condition characterized by a severe shortage of food that results in starvation and death."@en ;
    rdfs:subClassOf :Shortage, :StrongOrIntense, :FoodInsecurity .

:Fear a owl:Class ;
    rdfs:label "Fear (deprecated)"@en ;
    owl:deprecated "true"^^xsd:boolean ;
    rdfs:comment "Fear is an EmotionalResponse where an Actor is troubled by, has misgivings about, or anticipates pain or danger due to a situation or another Actor or thing. The Actor is identified using the event:has_active_actor property. If the response is directed toward another Actor, that individual is identified using the event:has_affected_actor property. If the response concerns a thing, that individual is identified using general:involves_goods_or_property. To associate a situation, the event:has_topic property is used."@en ;
    rdfs:comment "Note that Fear is deprecated in lieu of using its super-class, event:ApprehensionAnxietyFearOrWorry."@en ;
    rdfs:subClassOf :ApprehensionAnxietyFearOrWorry .

:FeelingSafeOrSecure a owl:Class ;
    rdfs:label "Feeling safe or secure"@en ;
    rdfs:comment "FeelingSafeOrSecure is an EmotionalResponse where an Actor believes that they are free from danger, harm or risk. The Actor is identified using the event:has_active_actor property."@en ;
    rdfs:subClassOf :EmotionalResponse .

:FeelingUnsafeOrInsecure a owl:Class ;
    rdfs:label "Feeling unsafe or insecure"@en ;
    rdfs:comment "FeelingUnsafeOrInsecure is an EmotionalResponse where an Actor believes that they are in danger, or at risk. The Actor is identified using the event:has_active_actor property."@en ;
    rdfs:subClassOf :EmotionalResponse .
  
:FilingOfLawsuit a owl:Class ;
    rdfs:label "Filing of lawsuit"@en ;
    rdfs:comment "Deals with registering a legal document which claims loss(es) due to the actions (or lack of action) by another, and remedies to be imposed by a court/the judicial system. The Actor registering the document/filing the lawsuit is known as the 'plaintiff' and is the active actor. The other Actor is the 'defendant' and is the affected actor."@en ;
    rdfs:subClassOf :LegalEvent . 
#   owl:equivalentClass oeevent:Bring_lawsuit_against .

:FinancialDeposit a owl:Class ;
    rdfs:label "Financial deposit"@en ;
    rdfs:comment "Concerns actions/events related to putting money into a bank or similar institution, a partial payment made at the time of purchase of something, a payment that acts as security and is made at the time of acquiring/taking something for temporary use, or any payment indicating that an obligation will be met."@en ;
    rdfs:subClassOf :FinancialEvent .
#   owl:equivalentClass cco:ActOfFinancialDeposit .

:FinancialEvent a owl:Class ;
    rdfs:label "Financial (finance-related) event"@en ;
    rdfs:comment "FinancialEvents involve monies/currency, such as a transfer of funds."@en ;
    rdfs:subClassOf :Event .
#   owl:equivalentClass cco:ActOfFinancialInstrumentUse .

:FinancialWithdrawal a owl:Class ;
    rdfs:label "Financial withdrawal"@en ;
    rdfs:comment "Concerns actions/events related to removing money or other securities/capital."@en ;
    rdfs:subClassOf :FinancialEvent, :Withdrawal .
#   owl:equivalentClass cco:ActOfFinancialWithdrawal .

:FindingOfGuilty a owl:Class ;
    rdfs:label "Finding of guilty"@en ;
    rdfs:comment "FindingOfIGuilty covers any legal judgment/verdict where the defendant is found 'guilty'. A synonymous term is 'convicted'."@en ;
    general:noun_exemplar "The jury reached a [[guilty verdict]]."@en ;
    general:noun_exemplar "The jurors deliberated for 6.5 hours before coming back with their [[verdict of guilty]] of first-degree murder."@en ;
    general:verb_exemplar "A Georgia woman was [[found guilty]] of starving her stepdaughter to death."@en ;
    general:verb_exemplar "Rudy Francis was [[convicted]] Sept. 17, 2010, of killing his business partner in a car in Gentilly."@en ;
    rdfs:subClassOf :LegalFinding .
#   owl:equivalentClass oeevent:Find_guilty_or_liable_(legally) .

:FindingOfInnocent a owl:Class ;
    rdfs:label "Finding of innocent (deprecated)"@en ;
    owl:deprecated "true"^^xsd:boolean ;
    rdfs:comment "FindingOfInnocent covers any legal judgment where the defendant is found 'not guilty'. A synonymous term is 'acquittal'. This term has been deprecated in lieu of using event:FindingOfNotGuilty."@en ;
    rdfs:subClassOf :LegalFinding ;
    owl:equivalentClass :FindingOfNotGuilty .

:FindingOfNotGuilty a owl:Class ;
    rdfs:label "Finding of not guilty"@en ;
    rdfs:comment "FindingOfNotGuilty covers any legal judgment where the defendant is found 'not guilty'. A synonymous term is 'acquittal'."@en ;
    general:noun_exemplar "The jury reached a [[verdict of not guilty]]."@en ;
    general:verb_exemplar "The Montgomery County sheriff’s deputy who was arrested in November was [[found not guilty]] on a second-degree criminal trespass charge."@en ;
    general:verb_exemplar "A jury [[acquitted]] a Naval Academy midshipman on all charges Friday, the culmination of a five-day trial for charges of sexual assault."@en ;
    general:noun_exemplar "In a rare move, a U.S. judge ordered the [[acquittal]] of Barclays' currency trader."@en ;
    rdfs:subClassOf :LegalFinding .

:Fire a owl:Class ;
    rdfs:label "Fire"@en ;
    rdfs:comment "A Fire can be a specific Event (such as a house fire) or an environmental concern/factor (such as a wildfire). The latter is indicated by using the sub-class, event:WildFire."@en ;
    rdfs:subClassOf :EventOrFactor .

:Flood a owl:Class ;
    rdfs:label "Flood"@en ;
    rdfs:comment "Floods involve a body of water overflowing onto normally dry lands. It may be the result of heavy rains or due to another reasons (such as the failure of a dam). In case of the former, the Event individual could also be classified using event:WeatherIssue."@en ;
    rdfs:subClassOf :NaturalDisaster .

:FoodWaterAndNutrition a owl:Class ;
    rdfs:label "Food, water and nutrition"@en ;
    rdfs:comment "FoodWaterAndNutrition is used to describe any events or conditions/factors/statistics related to food stuffs, their nutritional information and their availability, water quality and its availability, or the nutrition of a people/region. More specific sub-classes are defined and should be used whenever possible. These sub-classes include Food or WaterSecurity/Insecurity, Malnutrition, ContaminatedWater, WaterManagement or PromotionOfWaterSanitationAndHygiene (also a type of event:CivilCampaign). Because the semantics can address either events or conditions/factors, FoodWaterAndNutrition is defined as a subclass of event:EventOrFactor (specifically, a sub-class of event:HealthAndDisease). When defining general conditions or statistics, an individual should also be classified using event:LivingCondition, meas:ReportedValue or meas:TimeSeries."@en ;
    rdfs:subClassOf :HealthAndDisease, :LivingCondition .

:FoodInsecurity a owl:Class ;
    rdfs:label "Food insecurity"@en ;
    rdfs:comment "Food insecurity indicates a state/condition where people do not have access to 'sufficient, safe and nutritious food to meet their dietary needs and food preferences' (taken from the 1996 World Food Summit definition)."@en ;
    owl:disjointWith :FoodSecurity ;
    rdfs:subClassOf :FoodWaterAndNutrition .

:FoodSecurity a owl:Class ;
    rdfs:label "Food security"@en ;
    rdfs:comment "According to the 1996 World Food Summit, food security 'exists when all people, at all times, have physical and economic access to sufficient, safe and nutritious food to meet their dietary needs and food preferences for an active and healthy life'."@en ;
    rdfs:subClassOf :FoodWaterAndNutrition .

:ForcedMove a owl:Class ;
    rdfs:label "Forced/involuntary move/change of location"@en ;
    rdfs:comment "A ForcedMove is an involuntary change of location which could be for humanitarian, political or military reasons. Various sub-classes of ForcedMove are defined such as Expulsion, Extradition and Evacuation."@en ;
    rdfs:subClassOf :LocationChange, :ReductionRestrictionOrRemoval .

:Forgiving a owl:Class ;
    rdfs:label "Forgiving"@en ;
    rdfs:comment "Forgiving is a type of Communication where one Actor accepts the apology of another (where this Event is preceded_by an Apology Event), or decides to stop being upset or resentful toward another. The Actor who does the forgiving is the active actor, while the one who is forgiven is the affected actor. If the forgiveness is for a previous act/offense, that can be indicated using the event:has_topic property."@en ;
    rdfs:subClassOf :CommunicationConveyingEmpathy .
#   owl:equivalentClass oeevent:Forgive .

:FormalAgreement a owl:Class ;
    rdfs:label "Formal agreement"@en ;
    rdfs:comment "A FormalAgreement is a documented agreement/commitment between governments or legal entities/Actors. It is subclassed from AgreementOrPromise to add the semantic of a legally binding and/or formally signed agreement."@en ;
    rdfs:subClassOf :AgreementOrPromise .

:Frustration a owl:Class ;
    rdfs:label "Frustration"@en ;
    rdfs:comment "Frustration is an EmotionalResponse where an Actor has negative feelings due to being unable to change or achieve a situation. The situation which is desired, if known, can be associated using the event:has_topic property (and is defined with an event:has_tense of event:Future). The Actor who is frustrated is identified using the event:has_active_actor property."@en ;
    rdfs:subClassOf :EmotionalResponse .

:Funeral a owl:Class ;
    rdfs:label "Funeral"@en ;
    rdfs:comment "A Funeral is a type of Ceremony to honor a Person after their death. It may involve visitation and a formal ceremony and may include burial/cremation."@en ;
    rdfs:subClassOf :Ceremony .
#   owl:equivalentClass cco:Funeral .

:Goodwill a owl:Class ;
    rdfs:label "Goodwill"@en ;
    rdfs:comment "Goodwill is an EmotionalResponse where an Actor has a friendly, helpful or cooperative attitude (in general or toward another). The Actor who experiences the emotion is identified using the event:has_active_actor property. If the emotion is directed toward another Actor, that individual is identified using the event:has_affected_actor property."@en ;
    rdfs:subClassOf :EmotionalResponse .

:GoverningDirective a owl:Class ;
    rdfs:label "Governing law, policy or other directive"@en ;
    rdfs:comment "GoverningDirective is any law, policy or other formal declaration/instruction which is issued by a governmental authority/GPE and defines/restricts actions and behavior for a populace or a region. Note that the time that the law/policy/directive goes/went into effect (or will be/was terminated) can be defined using the InitiationOrStart and TerminationOrEnd Events, along with the GeneralConcepts' ontology's time properties."@en ;
    rdfs:subClassOf :PoliticalFactor .

:GovernmentActivity a owl:Class ;
    rdfs:label "Government activity"@en ;
    rdfs:comment "GovernmentActivities deal with the operation of a government and are sub-classed to executive, legislative and judicial activites."@en ;
    rdfs:subClassOf :Event .

:GovernmentalFactor a owl:Class ;
    rdfs:label "Governmental factor"@en ;
    rdfs:comment "Governmental factors deal with forms of government or general details regarding the functioning of the government."@en ;
    rdfs:subClassOf :PoliticalFactor .

:GovernmentCeremony a owl:Class ;
    rdfs:label "Government ceremony"@en ;
    rdfs:comment "An example of a GovernmentCeremony is an inauguration of a newly elected official."@en ;
    rdfs:subClassOf :Ceremony, :GovernmentActivity .

:Graduation a owl:Class ;
    rdfs:label "Graduation"@en ;
    rdfs:comment "Graduation is a Ceremony in which a person or person(s) are given diplomas and/or granted academic degrees. A synonym is 'commencement'."@en ;
    rdfs:subClassOf :PersonalLifeEvent, :Ceremony .

:GrantingOfAsylum a owl:Class ;
    rdfs:label "Granting of asylum"@en ;
    rdfs:comment "GrantingOfAsylum is a sub-class of ProvisionOfAid. It indicates that a GPE allows a foreign citizen to remain on its territory, at its embassies, on its vessels, etc. because they cannot return to their home country. This may be because of persecution or a fear of persecution due to ethnicity, religion, nationality, affiliations, etc. The UNHCR Refugee Agency describes various distinctions of the term, asylum. 'The term 'diplomatic asylum' in the broad sense is used to denote asylum granted by a State outside its territory, particularly in its diplomatic missions (diplomatic asylum in the strict sense), in its consulates, on board its ships in the territorial waters of another State (naval asylum), and also on board its aircraft and of its military or para-military installations in foreign territory. The other form of asylum granted to individuals, namely, that which is granted by the State within its borders, is generally given the name 'territorial asylum'. The terminology employed in this entire field lacks uniformity. The terms 'internal asylum', 'external asylum' and 'political asylum' are used by some to denote diplomatic asylum and by others to refer to territorial asylum. The State in whose territory diplomatic asylum is sought is know as the 'local' or 'territorial' State ... while the person granted asylum may be called either a 'refugee' or an 'asylee'.' (https://www.unhcr.org/protection/historical/3ae68bf10/question-diplomatic-asylum-report-secretary-general.html)"@en ;
    rdfs:subClassOf :ProvisionOfAid .
#   owl:equivalentClass oeevent:Grant_asylum .

:Grief a owl:Class ;
    rdfs:label "Grief"@en ;
    rdfs:comment "Grief is an EmotionalResponse where an Actor has feelings of intense sorrow due to the loss of someone or something. The Actor who is grief-stricken is identified using the event:has_active_actor property."@en ;
    rdfs:subClassOf :Sadness, :StrongOrIntense .
#   owl:equivalentClass oeceo:Grief .

:GrossDomesticProduct a owl:Class ;
    rdfs:label "Gross domestic product"@en ;
    rdfs:comment "GrossDomesticProduct indicates a GPE's economic health and is defined as the total value of goods and services produced/provided within the GPE, in a specific time period (usually a year). Instances of the class may describe general conditions such as its increase/decrease (event:Increase/Decrease/Stasis), or various statistics (an individual meas:ReportedValue or meas:TimeSeries) related to GDP."@en ;
    rdfs:subClassOf :EconomicFactor .

:GrossNationalIncome a owl:Class ;
    rdfs:label "Gross national income"@en ;
    rdfs:comment "GrossNationalIncome indicates a GPE's economic health and is similar to GrossDomesticProduct. GNI is defined as the sum of a GPE's gross domestic product, plus monies coming into a country (such as salaries paid by foreign companies or income from foreign properties). In many cases, GDP and GNI are similar. However, this will not be case for countries receiving significant monies as foreign aid. Instances of this class may describe general conditions such as GNI's increase/decrease (event:Increase/Decrease/Stasis), or various statistics (an individual meas:ReportedValue or meas:TimeSeries) related to GNI."@en ;
    rdfs:subClassOf :EconomicFactor .

:GroundCollapse a owl:Class ;
    rdfs:label "Ground collapse"@en ;
    rdfs:comment "A NaturalDisaster that occurs when the ground is too weak to support the structures built on it (due to erosion, excavation, earthquake, etc.) and collapses. Sinkholes are a type of ground collapse."@en ;
    rdfs:subClassOf :NaturalDisaster .

:GuardingOrPatrolling a owl:Class ;
    rdfs:label "Guarding and/or patrolling"@en ;
    rdfs:comment "GuardingOrPatrolling is the act of watching over someone or something in order to protect them or prevent harm. The action could involve a 'patrol' which periodically navigates around/through an area for security purposes."@en ;
    rdfs:subClassOf :ProtectionOrPreservation .

:Happiness a owl:Class ;
    rdfs:label "Happiness"@en ;
    rdfs:comment "Happiness is a range of EmotionalResponses from contentment to intense joy. The Actor who is happy is identified using the event:has_active_actor property. If the happiness concerns a situation, that can be associated using the event:has_topic property."@en ;
    rdfs:subClassOf :EmotionalResponse .
#   owl:equivalentClass oeceo:Happiness .

:Hatred a owl:Class ;
    rdfs:label "Hatred"@en ;
    rdfs:comment "Hatred is an EmotionalResponse where an Actor experiences intense dislike for another Actor, thing or situation. The Actor who is hateful is identified using the event:has_active_actor property. When the hate is directed toward another Actor, that individual is identified using event:has_affected_actor. If the hate is directed toward a thing (such as despising broccoli), the thing is identified using general:involves_goods_or_property. If the hate is regarding a situation, that can be associated using the event:has_topic property."@en ;
    rdfs:subClassOf :EmotionalResponse .

:HeadquartersOrBaseEstablished a owl:Class ;
    rdfs:label "Headquarters or base established"@en ;
    rdfs:comment "HeadquartersOrBaseEstablished describes an occurrence of note involving the opening/establishment of an office that serves as the administrative center of an enterprise, or the opening/establishment of a military installation from which operations are initiated or commanded."@en ;
    rdfs:subClassOf :Affiliation .

:HealthAndDisease a owl:Class ;
    rdfs:label "Health and disease"@en ;
    rdfs:comment "HealthAndDisease generally describes specific events (such as an event:Illness), general conditions such as disease outbreak in a region or malnutrition in a population/region (event:InfectiousHumanDisease or event:Malnutrition), increase/decrease trends (event:Increase/Decrease/Stasis) or statistics (an individual meas:ReportedValue or meas:TimeSeries) related to health and disease. Because the semantics can address either events or conditions/factors, it is defined as a subclass of event:EventOrFactor."@en ;
    rdfs:subClassOf :EventOrFactor .

:HighTemperature a owl:Class ;
    rdfs:label "High temperature"@en ;
    rdfs:comment "Temperatures perceived as 'high', typically nearing or above human body temperatures."@en ;
    rdfs:subClassOf :WeatherIssue .

:HighUnemployment a owl:Class ;
    rdfs:label "High unemployment"@en ;
    rdfs:comment "An EconomicCondition describing that many people in a region or segment of the population are without work/are unemployed."@en ;
    owl:disjointWith :LowUnemployment ;
    rdfs:subClassOf :Employment, :EconomicCondition .

:HighWind a owl:Class ;
    rdfs:label "High wind"@en ;
    rdfs:comment "A WeatherIssue describing strong gusts of air. Synonyms include the terms, 'squall', 'breeze', 'gale'. High winds may damage property, affect the spread of fire or enable the dispersal of plant seeds."@en ;
    rdfs:subClassOf :WeatherIssue .

:Hope a owl:Class ;
    rdfs:label "Hope"@en ;
    rdfs:comment "Hope is an EmotionalResponse where an Actor has positive feelings, desires or expectations that something will occur. The situation which is desired, if known, can be associated using the event:has_topic property (and is defined with an event:has_tense of event:Future). The Actor who is hopeful is identified using the event:has_active_actor property."@en ;
    rdfs:subClassOf :EmotionalResponse .
#   owl:equivalentClass oeceo:Hope .

:HumanitarianCrisis a owl:Class ;
    rdfs:label "Humanitarian crisis"@en ;
    rdfs:comment "A Factor that threatens the health, safety or well being of an area and its populace. It can be a natural or man-made disaster or a complex emergency (e.g., an individual is classified as an event:NaturalDisaster or one of its sub-classes, or as an event:CollectionOfEventsOrFactors with more specific member events)."@en ;
    rdfs:subClassOf :EnvironmentalFactor .

:HumanRightsAbuse a owl:Class ;
    rdfs:label "Human rights abuse"@en ;
    rdfs:comment "HumanRightsAbuses address a range of events from unfair trials and restriction of freedoms of expression, all the way to torture, murder, etc. An individual should be classified using multiple types when a murder (for example, of dissenters) occurs. That would be both event:MurderOrHomicide and event:HumanRightsAbuses. Note that not all murders are human rights abuses, and not all abuses are murders. These are separate concepts, but when they occur together, both classifications should be used."@en ;
    rdfs:subClassOf :Event .

:HungerStrike a owl:Class ;
    rdfs:label "Hunger strike"@en ;
    rdfs:comment "A voluntary refusal to eat, over a prolonged period of time, intended as an act of protest. The person, action or thing that is the subject of the protest is defined using the properties, event:has_affected_actor, event:has_topic or general:involves_goods_or_property, respectively."@en ;
    rdfs:subClassOf :Strike, :SymbolicAct .
#   owl:equivalentClass oeevent:Conduct_hunger_strike .

:HurricaneOrTyphoon a owl:Class ;
    rdfs:label "Hurricane or typhoon"@en ;
    rdfs:comment "HurricaneOrTyphoon describes a type of TropicalStorm with sustained winds of 74mph or higher. Hurricanes occur in the Atlantic Ocean and northeastern and north central Pacific Ocean. and a typhoon occurs in the Indian and northwestern Pacific Ocean."@en ;
    rdfs:subClassOf :TropicalStorm .

:Identification a owl:Class ;
    rdfs:label "Identification"@en ;
    rdfs:comment "Identification involves asserting who or what someone or something is (for example, identifying an assailant or murder weapon), or who/what/how a situation came to be. When using the Identification Event type, it is important to define who or what is being identified. This is accomplished using the event:has_affected_actor, event:has_topic and general:involves_goods_or_property object properties (referencing an Actor, an act/event or thing, respectively)."@en ;
    rdfs:subClassOf :DeclarativeCommunication .
#   owl:equivalentClass cco:ActOfIdentifying .

:Illness a owl:Class ;
    rdfs:label "Illness"@en ;
    rdfs:comment "Used when a person or population/group is sick due to a contagion, mental condition or disease. The semantics can describe a specific event, a general condition/factor of increased/decreased illness by a set of people or in a region (event:Increase/Decrease/Stasis), or statistics (an individual meas:ReportedValue or meas:TimeSeries) related to illness in a population/region."@en ;
    rdfs:subClassOf :HealthAndDisease .

:IllnessOrInjury a owl:Class ;
    rdfs:label "Illness or inury"@en ;
    rdfs:comment "When a person is ill or injured in some way, but the exact nature of the condition is unknown, then this class should be used. However, if the condition is known to be a disease, mental condition or sickness due to a contagion, then the more specific class of Illness should be used. If the condition is due to an injury, then that class (or its event:Wounding sub-class) should be used."@en ;
    rdfs:subClassOf :HealthAndDisease ;
    owl:equivalentClass [ a owl:Class;
                          owl:unionOf ( :Illness :Injury ) ] .

:Immigration a owl:Class ;
    rdfs:label "Immigration"@en ;
    rdfs:comment "Movement to a new location, usually to a country where the Actor is not a citizen, in order to settle there. Note that immigration versus emigration is only a difference of perspective. To emigrate is to leave a location to reside permanently in another, while immigration is to come to a new location to reside. It is defined as a sub-class of ChangeOfResidence, and the origin and destination locations can be specified using the event:has_origin/destination properties."@en ;
    rdfs:subClassOf :ChangeOfResidence .

:Import a owl:Class ;
    rdfs:label "Import"@en ;
    rdfs:comment "Import deals with any conditions favorable/disfavorable to bringing goods or services into a country, or various statistics (an individual meas:ReportedValue or meas:TimeSeries) related to imports. Factors which influence import include their availability, trade policies, exchange rates and demand, among others."@en ;
    rdfs:subClassOf :EconomicFactor .

:ImportAndExport a owl:Class ;
    rdfs:label "Import and export"@en ;
    rdfs:comment "ImportAndExport deals with any conditions favorable/disfavorable to bringing goods or services into/out of a country, or various statistics (an individual meas:ReportedValue or meas:TimeSeries) related to import/export. Factors which influence import/export include their availability, trade policies, exchange rates and demand, among others."@en ;
    rdfs:subClassOf :EconomicFactor ;
    owl:equivalentClass [ a owl:Class ;
                          owl:unionOf ( :Import :Export ) ] .

:Imprisonment a owl:Class ;
    rdfs:label "Imprisonment"@en ;
    rdfs:comment "Imprisonment is a legal/military ('official') action related to being held in jail for just or unjust cause. It is distinguished from the AbductionHostageTakingOrHijacking Event type (~kidnapping)."@en ;
    rdfs:subClassOf :LegalEvent .

:IncomeAndExpense a owl:Class ;
    rdfs:label "Income and expense"@en ;
    rdfs:comment "IncomeAndExpense deals an individual Actor's reported incomes/revenue/expenses, overall trends and changes (event:Increase/Decrease/Stasis), or statistics (individual meas:ReportedValues or meas:TimeSeries) for a population or region. The Actor is identified using event:has_actor and the location is defined using general:located_at."@en ;
    rdfs:subClassOf :EconomicFactor .

:Incompetency a owl:Class ;
    rdfs:label "Incompetency"@en ;
    rdfs:comment "Describes that a specific Actor (Person, GroupOfPersons/Organization, GeopoliticalEntity, ...) is incompetent or that a situation of incompetency exists in some location/organization/etc. Note that the 'incompentent' Actor is related to the Factor using event:has_actor."@en ;
    rdfs:subClassOf :Factor .

:Increase a owl:Class ;
    rdfs:label "Increase"@en ;
    rdfs:comment "The class, Increase, is used to record a growth/increase in the availability/amount of a thing/artifact (such as an increase in the amount of food, water or schooling), a growth/increase in the number of people in certain roles (such as an increase in the number of police or teachers), or increases related to 'general' Events (such as an increase in the number of MurderOrHomicide occurrences in a specific location) or Factors (such as an increase in the Anger level in a community). If the increase is related to another Event/Factor, the Increase individual uses the event:has_topic property to reference that other Event. To identify an increase in the availability/amount of something, the Increase individual is related to the artifact using general:involves_goods_or_property. To identify an increase in the number of people in certain roles, those people are defined as an individual that is a GroupOfPersons with a general:position_or_role property, and that entity is related to the Increase via event:has_actor."@en ;
    rdfs:subClassOf :Change .

:Indictment a owl:Class ;
    rdfs:label "Indictment"@en ;
    rdfs:comment "A formal charge/LegalEvent accusing an Actor of wrongdoing. The Actor that is charged/accused is the affected actor and the wrongdoing is associated using the event:has_topic property."@en ;
    rdfs:subClassOf :AccusationOrAssigningOfResponsibility, :LegalEvent .

:InfectiousHumanDisease a owl:Class ;
    rdfs:label "Infectious human disease"@en ;
    rdfs:comment "InfectiousHumanDisease may describe either a specific illness/sickness, the presence of a disease/outbreak in a population/region, overall trends and changes (e.g., event:Increase/Decrease/Stasis) or statistics (individual meas:ReportedValues or meas:TimeSeries)."@en ;
    rdfs:subClassOf :HealthAndDisease .

:Influence a owl:Class ;
    rdfs:label "Indictment"@en ;
    rdfs:comment "Action intended to have an effect on the character, development, or behavior of someone or something. Influence includes interference, manipulation and similar concepts."@en ;
    rdfs:subClassOf :Event .

:InformationHandling a owl:Class ;
    rdfs:label "Information handling"@en ;
    rdfs:comment "Information handling deals with any activities to collect (for example by observation), process (store, transmit, protect, disrupt), or act on information."@en ;
    rdfs:subClassOf :Event .

:InformationOperation a owl:Class ;
    rdfs:label "Information operation"@en ;
    rdfs:comment "An InformationOperation deals with actions taken to affect an adversary's beliefs, positions and information systems, while defending one's own positions and systems. It may involve ElectromagneticActivities to affect enemy communications, ProgandaActivities to influence civilian populations, Deceptions to camouflage troop movements, etc. An Operation occurs over time, has specific goals, and is composed of specific, coordinated acts/Events intended to achieve those goals. The component Events (if known) are associated using the general:has_member property. The goal is identified using the actor:has_objective property."@en ;
    rdfs:comment "From JP1-02, information operations are 'the integrated employment, during military operations, of information-related capabilities in concert with other lines of operation to influence, disrupt, corrupt, or usurp the decision-making of adversaries and potential adversaries while protecting our own."@en ;
    rdfs:subClassOf :Operation, :InformationHandling .

:InfrastructureAndUtilities a owl:Class ;
    rdfs:label "Infrastructure and utilities"@en ;
    rdfs:comment "InfrastructureAndUtilities deal with the basic facilities, services/utilities, and installations needed for the functioning of a community or society. Individuals may describe specific events concerning structures and services, their general conditions (event:Factor and/or event:Increase/Decrease/Stasis), or various statistics (meas:ReportedValues and meas:TimeSeries) about them. As examples of specific events, consider the building of a new power generation plant or damage to a road or bridge. These individuals would be classified as both event:InfrastructureAndUtilities and event:ManufacturingCreatingOrBuilding or event:DamageOrDestruction, and would use general:involves_goods_or_property to indicate the power plant facility or structure."@en ;
    rdfs:subClassOf :EventOrFactor .

:Injury a owl:Class ;
    rdfs:label "Injury"@en ;
    rdfs:comment "Used when a person is harmed in some specific event, to provide statistics (an individual meas:ReportedValue or meas:TimeSeries), or to describe a general condition/factor of increased/decreased injury (event:Increase/Decrease/Stasis). Note that event:Wounding is a sub-class indicating that an injury was the result of some violence."@en ;
    rdfs:subClassOf :HealthAndDisease .

:Innovation a owl:Class ;
    rdfs:label "Innovation"@en ;
    rdfs:comment "Deals with factors affecting (driving or suppressing) innovation in a population or region, such as funding, governmental policy, openness to new ideas, business outcomes of innovation, etc."@en ;
    rdfs:subClassOf :Factor .

:InsectInfestation a owl:Class ;
    rdfs:label "Insect infestation"@en ;
    rdfs:comment "The condition of being invaded or overrun by insects that feed on humans, animals, plants, wooden structures, etc. Individuals may describe specific infestation events, the general conditions or overall trends and changes (event:Increase/Decrease/Stasis) related to infestations, or statistics (individual meas:ReportedValues and meas:TimeSeries)."@en ;
    general:noun_exemplar "Left unchecked, pest and [[insect infestations]] can really get the better of your home."@en ;
    general:noun_exemplar "Countries could then prepare to reduce the impact of [[insect invasions]]."@en ;
    general:noun_exemplar "[[Crop losses to pests]] may grow."@en ;
    general:verb_exemplar "Rising temperatures can encourage, or discourage, [[insects invading]] new territories."@en ;
    rdfs:subClassOf :EnvironmentalFactor .

:InspectionOrObservation a owl:Class ;
    rdfs:label "Inspection and/or observation"@en ;
    rdfs:comment "InspectionOrObservation involves both formal and informal review/paying attention to someone or something and (likely) producing a report/analysis. Who or what is inspected/observed is defined by either the event:has_affected_actor, event:involves_goods_or_property or event:has_topic properties."@en ;
    rdfs:subClassOf :Event .

:Inspiration a owl:Class ;
    rdfs:label "Inspiration"@en ;
    rdfs:comment "Inspiration is an EmotionalResponse where an Actor is motivated to do something/be creative. The Actor who is inspired is identified using the event:has_active_actor property. The situation/act which is desired, if known, can be associated using the event:has_topic property (and is defined with an event:has_tense of event:Future)."@en ;
    rdfs:subClassOf :EmotionalResponse .
#   owl:equivalentClass oeceo:Inspiration .

:IntelligenceGathering a owl:Class ;
    rdfs:label "Intelligence gathering"@en ;
    rdfs:comment "IntelligenceGathering deals with activities to collect, collate, evaluate, analyze, integrate and interprete collected military, economic, … information. From JP1-02, intelligence is '1. The product resulting from the collection, processing, integration, evaluation, analysis, and interpretation of available information concerning foreign nations, hostile or potentially hostile forces or elements, or areas of actual or potential operations. 2. The activities that result in the product. 3. The organizations engaged in such activities.'"@en ;
    rdfs:subClassOf :InformationHandling .

:IntelligenceOperation a owl:Class ;
    rdfs:label "Intelligence operation"@en ;
    rdfs:comment "An example of an IntelligenceOperation is an ongoing wiretap monitoring a Person. An Operation occurs over time, has specific goals, and is composed of specific, coordinated acts/Events intended to achieve those goals. The component Events (such as Espionage or ReconnaissanceOperation, EspionageOrTreason or ReconnaissanceActivity) are associated using the general:has_member property. The goal is identified using the actor:has_objective property."@en ;
    rdfs:comment "From JP1-02, intelligence is '1. The product resulting from the collection, processing, integration, evaluation, analysis, and interpretation of available information concerning foreign nations, hostile or potentially hostile forces or elements, or areas of actual or potential operations. 2. The activities that result in the product. 3. The organizations engaged in such activites.'"@en ;
    rdfs:subClassOf :InformationOperation .

:Interview a owl:Class ;
    rdfs:label "Interview"@en ;
    rdfs:comment "An Interview involves questioning a Person to gather information, especially regarding information to be hired, for the purpose of doing an evaluation, etc. When using the Interview Event type, it is important to indicate who is being interviewed and why (for what purpose). This is accomplished using the event:has_affected_actor and event:has_topic object properties. The latter may be a 'Future' event (such as being hired)."@en ;
    rdfs:subClassOf :ExploratoryCommunication .

:IntimidationAndCoercion a owl:Class ;
    rdfs:label "Intimidation and coercion"@en ;
    rdfs:comment "Event dealing with the use of force or authority to compel or dissuade action, or to induce fear. IntimidationAndCoercion crosses political, economic, diplomatic, military and other categories as indicated by the specific actors involved."@en ;
    rdfs:subClassOf :Influence .
#   owl:equivalentClass oeevent:Coerce .

:Investigation a owl:Class ;
    rdfs:label "Investigation"@en ;
    rdfs:comment "Investigation can be either a formal or informal search for someone, something, some place (e.g., a facility) or some information. The object of the search can be described using the general:involves_goods_or_property predicate."@en ;
    rdfs:subClassOf :Event .
#   owl:equivalentClass oeevent:Investigate .

:Investment a owl:Class ;
    rdfs:label "Investment"@en ;
    rdfs:comment "The different types of investments are stocks, bonds, funds (such as mutual funds), bank products (such as savings accounts), options, annuities, retirement investments (such as a 401K or IRA), and futures (both commodity and security). These are indicated by using the event:has_instrument property to reference a subclass of cco:Artifact. A purchase or receipt of investment funds is distinguished by adding either the event:Purchasing or event:Receipt classification."@en ;
    rdfs:comment "Investment may describe specific events (such as a Person investing their lottery winnings in a business), general conditions such as an increase/decrease in investments in a population/region/location (event:Increase/Decrease/Stasis), or statistics (an individual meas:ReportedValue or meas:TimeSeries) related to investment. Because the semantics can address either events or conditions/factors, it is defined as a subclass of event:EventOrFactor."@en ;
    rdfs:subClassOf :FinancialEvent, :EventOrFactor .

:Invitation a owl:Class ;
    rdfs:label "Invitation"@en ;
    rdfs:comment "An Invitation is a request/communication (either verbal or written) to participate or be present in some event. The Event is indicated using event:has_topic and may be a 'Future' event. The Actor who is invited is defined by event:has_affected_actor."@en ;
    rdfs:subClassOf :RequestOrAppeal .
#   owl:equivalentClass cco:ActOfInviting .

:IssuingPublishingOrReleasing a owl:Class ;
    rdfs:label "Issuing, publishing or releasing"@en ;
    rdfs:comment "IssuingPublishingOrReleasing involves activities related to providing something new, potentially in return for payment. Examples include providing visual, audio or written materials (such as issuing a press release), or releasing a new product or software. The goal is to make something known, or to announce, provide or disseminate something to some Actor(s). The vehicle for IssuingPublishingOrReleasing (such as a cco:Report or event:BlogPost) is identified using event:has_instrument, while information on what the item concerns (e.g., an Event, Artifact or Actor) is identified using the event:has_topic, event:involves_goods_or_property or event:has_affected_actor properties, respectively."@en ;
    rdfs:subClassOf :Event .

:JailsAndPrisoners a owl:Class ;
    rdfs:label "Jails and prisoners"@en ;
    rdfs:comment "JailsAndPrisoners is concerned with general information related to increases/decreases of jail facilities or Persons who are incarcerated (event:Increase/Decrease/Stasis), or specific statistics (an individual meas:ReportedValue or meas:TimeSeries) related to jails and prisoners. Note that if the information describes the demographics of the prisoner population, then the class event:Demographic should also be used to classify the individual."@en ;
    rdfs:subClassOf :Factor .

:Jealousy a owl:Class ;
    rdfs:label "Jealousy"@en ;
    rdfs:comment "Jealousy is an EmotionalResponse where an Actor envies another and their situation or possessions. The Actor who is jealous is identified using the event:has_active_actor property. If the jealousy is directed toward another Actor, that individual is identified using the event:has_affected_actor property."@en ;
    rdfs:subClassOf :EmotionalResponse .
#   owl:equivalentClass oeceo:Jealousy .

:JointOperation a owl:Class ;
    rdfs:label "Joint operation such as conducted by a 'joint' task force"@en ;
    rdfs:comment "A JointOperation 'connotes activities [and] operations ... in which elements of two or more Military Departments participate' (from JP1-02). An Operation occurs over time, has specific goals, and is composed of specific, coordinated acts/Events intended to achieve those goals. The component Events (if known) are associated using the general:has_member property. The goal is identified using the actor:has_objective property."@en ;
    rdfs:subClassOf :Operation .

:JudicialCooperation a owl:Class ;
    rdfs:label "Judicial cooperation"@en ;
    rdfs:comment "JudicialCooperation may describe either a specific event where two actors work together to achieve a goal, or a general environment of cooperation. The former should also be defined as a type of event:JudicialGovernmentActivity, while the latter is a type of event:Factor. A goal of the Cooperation can be defined using the actor:has_objective property. The Actors that are cooperating are identified using the event:has_active_actor property."@en ;
    rdfs:subClassOf :Cooperation .
#   owl:equivalentClass oeevent:Engage_in_judicial_cooperation .

:JudicialGovernmentActivity a owl:Class ;   
    rdfs:label "Judicial government activity"@en ;
    rdfs:comment "JudicialGovernmentActivities deal with the operation of the judicial branch of government - for example, appointment and removal of judges, the definition of policies, etc."@en ;
    rdfs:subClassOf :GovernmentActivity .

:JuryDeliberation a owl:Class ;
    rdfs:label "Jury deliberation"@en ;
    rdfs:comment "JuryDeliberation is an activity of a trial's jury, where the members of the jury discuss the trial and legal arguments (in private) to decide on a verdict (guilty or not guilty, or deciding in favor of the case's plaintiff or defendant). The jury is the active actor, and its members (if known) can be identified using general:has_member."@en ;
    rdfs:subClassOf :LegalEvent .

:LackOfOrNegativeSupport a owl:Class ;
    rdfs:label "Lack of support, or negative sentiment (deprecated)"@en ;
    owl:deprecated "true"^^xsd:boolean ;
    rdfs:comment "LackOfOrNegativeSupport deals either with a general Factor/condition indicating dissatisfaction or a communication arguing against a topic or Actor. This class is deprecated in lieu of using event:DisapprovalOrDenunciation for the latter, or event:LackOfSupportOrDissatisfaction for the former. When using this Event type, it is important to indicate what is being opposed/not supported. This is accomplished using the event:has_affected_actor, event:has_topic or general:involves_goods_or_property object properties (referencing an Actor, an act/event or a thing). Examples of LackOfSupport include protesting against a Person who might be accused of a crime (where the Person is related using has_affected_actor), denigrating an action/event that an Actor performed (where the event is defined using event:has_topic), or opposing a thing, such as guns/firearms (where the thing is specified using general:involves_goods_or_property)."@en ;
    rdfs:subClassOf :EventOrFactor ;
    owl:equivalentClass [ a owl:Class; 
                          owl:unionOf ( :DisapprovalOrDenunciation :LackOfSupportOrDissatisfaction ) ] .

:LackOfRespectForRightsFreedoms a owl:Class ;
    rdfs:label "Lack of respect for human rights and political freedoms"@en ;
    rdfs:comment "Fundamental rights (as defined by the United Nations) include the right to self-determination, liberty, due process and peaceful assembly/freedom of association, as well as freedom of thought, religion, movement and expression. This class deals with restrictions or refusal to permit individual freedoms by the government, military, law enforcement or social groups. It includes passing laws, ignoring abuses, or actively suppressing rights and freedoms. LackOfRespectForRightsFreedoms may describe either a specific event, or a general environment of lack of respect. When defining general conditions or statistics, an individual should also be classified using event:LivingCondition, meas:ReportedValue or meas:TimeSeries."@en ;
    rdfs:subClassOf :EventOrFactor .

:LackOfSupportOrDissatisfaction a owl:Class ;
    rdfs:label "Lack of support or dissatisfaction"@en ;
    rdfs:comment "LackOfSupport deals with dissatisfaction with someone or something. It is important to indicate what is being opposed/not supported or the subject of the dissatisfaction. This is accomplished using the event:has_affected_actor, event:has_topic or general:involves_goods_or_property object properties (referencing an Actor, an act/event or a thing). An example of LackOfSupportOrDissatisfaction is general opposition to a thing, such as a law or guns/firearms (where the thing is specified using general:involves_goods_or_property)."@en ;
    rdfs:subClassOf :Factor .

:LandslideOrMudslide a owl:Class ;
    rdfs:label "Landslide or mudslide"@en ;
    rdfs:comment "A slide of a large mass of dirt, rock or mud down a mountain or cliff. It is a form of event:NaturalDisaster."@en ;
    rdfs:subClassOf :NaturalDisaster .

:LandUse a owl:Class ;
    rdfs:label "Land use"@en ;
    rdfs:comment "A sub-class of event:NaturalResources, providing information about how the land/environment is managed and/or modified for various uses."@en ;
    rdfs:subClassOf :NaturalResources .

:Lawlessness a owl:Class ;
    rdfs:label "Lawlessness"@en ;
    rdfs:comment "A Factor dealing with disorder and/or disrespect for the law in a region or for a population. "@en ;
    rdfs:subClassOf :LivingCondition, :DefyingLawsNormsDirectives .

:LegalEvent a owl:Class ;
    rdfs:label "Legal (law-related) event"@en ;
    rdfs:comment "Any activity/event based on law, official or accepted rules, or related to or allowed by laws or the legal system."@en ;
    rdfs:subClassOf :JudicialGovernmentActivity .
#   owl:equivalentClass cco:ActOfLegalInstrumentUse .

:LegalFinding a owl:Class ;
    rdfs:label "Legal finding by judge/jury"@en ;
    rdfs:comment "A legal finding is either 'guilty' or 'not guilty' for a criminal case, or a finding in favor of the plaintiff or defendant in a civil case. The active actor is the judge or jury which issues the finding, and the affected actor is the defendant in the criminal case, or the (losing) plaintiff or defendant in the civil case."@en ;
    rdfs:subClassOf :LegalEvent .

:LegalFine a owl:Class ;
    rdfs:label "Legal fine"@en ;
    rdfs:comment "A LegalFine is the amount of money or penalty that a court, jury or other authority decides has to be paid as punishment for a crime or other offence. The affected actor is the Actor which has to make the payment or satisfy the penalty."@en ;
    rdfs:subClassOf :LegalFinding .

:LegalProceedingsOrTrial a owl:Class ;
    rdfs:label "Legal proceedings/trial"@en ;
    rdfs:comment "A type of LegalEvent, such as a trial or binding arbitration. 'Although the term may be defined more broadly or more narrowly as circumstances require, it has been noted that [t]he term legal proceedings includes proceedings brought by or at the instigation of a public authority, [or] an appeal against the decision of a court or tribunal. Legal proceedings are generally characterized by an orderly process in which participants or their representatives are able to present evidence in support of their claims, and to argue in favor of particular interpretations of the law, after which a judge, jury, or other factfinder makes a determination of the factual and legal issues.' Activities include 'conduct of a trial, whether a lawsuit or civil trial, or a criminal trial; issuance and enforcement of court orders, including those imposing foreclosure or receivership; hearings, particularly administrative hearings; [or] arbitration'. (https://en.wikipedia.org/wiki/Legal_proceeding)"@en ;
    rdfs:subClassOf :Ceremony, :LegalEvent .

:LegalSentence a owl:Class ;
    rdfs:label "Legal sentence"@en ;
    rdfs:comment "A LegalSentence is 'the post-conviction stage of the criminal justice process, in which the defendant is brought before the court for the imposition of a penalty ... A sentence is the penalty ordered by the court. Generally, the primary goals of sentencing are punishment, deterrence, incapacitation, and rehabilitation. In some states, juries may be entitled to pronounce sentence, but in most states, and in federal court, sentencing is performed by a judge."@en ;
    rdfs:subClassOf :LegalFinding .

:LegislativeGovernmentActivity a owl:Class ;
    rdfs:label "Legistlative government activity"@en ;
    rdfs:comment "LegislativeGovernmentActivities deal with the operation of the legistlative branch of the government - for example, the election of officials, voting on laws/legislation, etc. The Activity individual may be further classified by other Event types, such as event:Election."@en ;
    rdfs:subClassOf :GovernmentActivity .

:LifeExpenctancy a owl:Class ;
    rdfs:label "Life expenctancy"@en ;
    rdfs:comment "A Factor providing data (typically, an individual meas:ReportedValue or meas:TimeSeries) about the life expectancies of a population or particular sub-groups within it. The population/group whose demographic is reported is identified using the event:has_actor property."@en ;
    rdfs:subClassOf :Demographic .

:LimnicEruption a owl:Class ;
    rdfs:label "Limnic eruption"@en ;
    rdfs:comment "Occurs when a gas (such as CO2) erupts from a deep lake water and could potentially suffocate animal life and humans. A tsunami may also result from a LimnicEruption."@en ; 
    rdfs:subClassOf :NaturalDisaster .

:LivingCondition a owl:Class ;
    rdfs:label "Living condition (in an area)"@en ;
    rdfs:comment "Deals with a variety of factors that reflect (improve or worsen) access to shelter, food, clothing, safety, clean water, etc. Sub-classes include event:Lawlessness, event:SanitaryConditions and event:UnsanitaryConditions, as well as event:FoodWaterAndNutrition."@en ;
    rdfs:subClassOf :SocialCondition .

:Loan a owl:Class ;
    rdfs:label "Loan"@en ;
    rdfs:comment "Something that is lent/borrowed. If money is lent, then a Loan individual would also be a FinancialEvent."@en ;
    rdfs:comment "Loan may describe specific events (such as an bank loaning money to a business), general conditions such as an increase/decrease in loans in a population/region/location (event:Increase/Decrease/Stasis), or statistics (an individual meas:ReportedValue or meas:TimeSeries) related to loans. Because the semantics can address either events or conditions/factors, it is defined as a subclass of event:EventOrFactor."@en ;
    rdfs:subClassOf :EventOrFactor .

:LocatingOrTargeting a owl:Class ;
    rdfs:label "Locating or targeting"@en ;
    rdfs:comment "LocatingOrTargeting involves determining/indicating an entity or location, especially related to aiming a weapon or for attack. The entity or location that is targeted is defined using the properties, event:has_affected_actor, general:involves_goods_or_property or event:has_destination (if the entity is an Actor, Artifact or Location, respectively). From JP1-02, a target is 'an entity or object that performs a function for the threat considered for possible engagement or other action'."@en ;
    general:verb_exemplar "The telescope enables us to [[locate]] objects in space."@en ; 
    general:verb_exemplar "A web application can be [[targeted]] by Cyber Criminals with different attacks."@en ; 
    general:noun_exemplar "The Department of Defense defined its strategic nuclear weapons [[targeting]] policy."@en ;
    rdfs:subClassOf :Identification .

:LocationChange a owl:Class ;
    rdfs:label "Location change"@en ;
    rdfs:comment "LocationChange involves the movement of people or goods. If the origin/destination are known, these can be specified using the event:has_origin/destination properties. If the Actor or goods are known, these can be defined using event:has_affected_actor or event:involves_goods_or_property. If the manner of transportation is known, that can be defined using the event:has_instrument property."@en ;
    rdfs:subClassOf :Event .
#   owl:equivalentClass cco:ActOfLocationChange .

:Looting a owl:Class ;
    rdfs:label "Looting"@en ;
    rdfs:comment "Stealing/plundering during riots or in wartime."@en ;
    rdfs:subClassOf :TheftOrRobbery , :Violence .

:LowUnemployment a owl:Class ;
    rdfs:label "Low unemployment"@en ;
    rdfs:comment "An EconomicCondition describing that many people in a region or segment of the population have work/are employed."@en ;
    rdfs:subClassOf :Employment, :EconomicCondition .

:Maintenance a owl:Class ;
    rdfs:label "Maintenance"@en ;
    rdfs:comment "Maintenance is any kind of functional checking, servicing, repairing or replacing of devices, equipment, machinery, building infrastructure, utilities, software, hardware, ... The individual that is maintained is identified using event:involves_goods_or_property."@en ;
    rdfs:subClassOf :Event .

:Malnutrition a owl:Class ;
    rdfs:label "Malnutrition"@en ;
    rdfs:comment "Malnutrition may describe either a specific case of malnutrition, or a general conditions/statistics in a region. The latter is indicated by also classifying the individual as a type of event:Factor, meas:ReportingValue or meas:TimeSeries."@en ;
    rdfs:subClassOf :FoodWaterAndNutrition .

:ManufacturingCreatingOrBuilding a owl:Class ;
    rdfs:label "Manufacturing, creating or building"@en ;
    rdfs:comment "ManufacturingCreatingOrBuilding deals with defining, supervising, engaging in or financing the construction of something, creating a plan for something (such as a blueprint), or developing, founding, strengthening or building something up. The entity that is manufactured/created/built is typically defined by event:involves_goods_or_property, but may be defined by event:has_affected_actor when describing creating/building a new organization."@en ;
    rdfs:subClassOf :Event .
#   owl:equivalentClass cco:ActOfManufacturing .

:ManufacturingOrBuilding a owl:Class ;
    rdfs:label "Manufacturing or building (deprecated)"@en ;
    owl:deprecated "true"^^xsd:boolean ;
    rdfs:comment "ManufacturingCreatingOrBuilding deals with defining, supervising, engaging in or financing the construction of something, creating a plan for something (such as a blueprint), or developing, founding, strengthening or building something up. The entity that is manufactured/created/built is typically defined by event:involves_goods_or_property, but may be defined by event:has_affected_actor when describing creating/building a new organization."@en ;
    rdfs:comment "Note that ManufacturingOrBuilding has been deprecated in lieu of using its super-class, ManufacturingCreatingOrBuilding."@en ;
    rdfs:subClassOf :ManufacturingCreatingOrBuilding .
#   owl:equivalentClass cco:ActOfManufacturing .

:MaritimeDomainAwareness a owl:Class ;
    rdfs:label "Maritime domain awareness (MDA)"@en ;
    rdfs:comment "From JP1-02, MDA is 'the effective understanding of anything associated with the maritime domain that could impact the security, safety, economy, or environment of a nation.' Maritime domain is defined as 'the oceans, seas, bays, estuaries, islands, coastal areas, and the airspace above these, including the littorals'."@en ;
    rdfs:subClassOf :AwarenessOrUnderstanding .

:MassKilling a owl:Class ;
    rdfs:label "Mass killing"@en ;
    rdfs:comment "According to the Congressional Research Service report (https://fas.org/sgp/crs/misc/R44126.pdf) and FBI, 'mass [killing]' is defined as a multiple homicide incident in which four or more victims are [killed] ..., within one event, and in one or more locations in close proximity'."@en ;
    rdfs:subClassOf :MurderOrHomicide .
#   owl:equivalentClass oeevent:Engage_in_mass_killings .

:Mediation a owl:Class ;
    rdfs:label "Mediation"@en ;
    rdfs:comment "Mediation is a type of event:Negotiation to resolve differences or bring about a settlement that is conducted by some impartial party. The latter is identified as the active actor, while the groups who are mediated are the affected actors. When using the Mediation Event type, it may be important to indicate what is being mediated. This is accomplished using the event:has_topic object property."@en ; 
    rdfs:subClassOf :Negotiation .
#   owl:equivalentClass oeevent:Engage_in_mediation .

:MedicalEmergency a owl:Class ;
    rdfs:label "Medical emergency"@en ;
    rdfs:comment "MedicalEmergency is a specific event, requiring immediate medical attention/assistance, where an individual's life or organ/body function may be lost or severely impaired. The Actor/Person requiring attention is identified as the affected actor."@en ;
    rdfs:subClassOf :PersonalLifeEvent .

:MeetingEncounterOrNegotiation  a owl:Class ;
    rdfs:label "Meeting, encounter or negotiation (deprecated)"@en ;
    owl:deprecated "true"^^xsd:boolean ;
    rdfs:comment "MeetingEncounterOrNegotiation is defined as a mapping aid, based on the combining of the semantics of meeting and negotiation in the CAMEO event codes. It is recommended that this class NOT be used (it is deprecated). The more general class, event:MeetingOrEncounter, should be used if the reason for the gathering is unknown. If the purpose is negotiation, then an instance of the event:Negotiation class should be created."@en ;
    rdfs:subClassOf :Event ;
    owl:equivalentClass [ a owl:Class ;
                          owl:unionOf ( :MeetingOrEncounter :Negotiation ) ] .

:MeetingOrEncounter  a owl:Class ;
    rdfs:label "Meeting or encounter"@en ;
    rdfs:comment "A formal, informal or coincidental gathering or assembly of people."@en ;
    general:noun_exemplar "Bolton also mentioned that, at the [[meeting]] with Russian President Vladimir Putin in Finland on July 16, U. S. President Donald Trump had underlined that America does not recognize the illegal annexation of Crimea‚ and denounces Russia's war in Ukraine."@en ;
    general:verb_exemplar "Putin praised Russia's increasingly close ties with China as he [[met]] with Xi at the economic forum in Vladivostok on Tuesday."@en ;
    rdfs:subClassOf :Event .
#   owl:equivalentClass [ a owl:Class ;
#                         owl:unionOf ( cco:ActOfEncounter, cco:ActOfMeeting ) ] .

:Merger a owl:Class ;
    rdfs:label "Merger"@en ;
    rdfs:comment "A Merger is an event:FormalAgreement and event:LegalEvent that defines the combination of two or more entities. All entities are defined as the active actors."@en ;
    rdfs:subClassOf :FormalAgreement, :LegalEvent .

:MilitaryAction a owl:Class ;
    rdfs:label "Military action"@en ;
    rdfs:comment "MilitaryAction is a general semantic for any type of military activity or action, etc."@en ;
    rdfs:subClassOf :MilitaryFactor .

:MilitaryCampaignOrOperation a owl:Class ;
    rdfs:label "Military campaign/operation"@en ;
    rdfs:comment "From JP1-02, a military operation is '1. A sequence of tactical actions with a common purpose or unifying theme. 2. A military action or the carrying out of a strategic, operational, tactical, service, training, or administrative military mission.' An Operation occurs over time, has specific goals, and is composed of specific, coordinated acts/Events intended to achieve those goals. The component Events (if known) are associated using the general:has_member property. The goal is identified using the actor:has_objective property. Note that individual MilitaryActions may be part of a MilitaryOperation. If so, then they are associated with the Operation using the general:has_member property."@en ;
    rdfs:subClassOf :Operation, :MilitaryFactor .

:MilitaryCapability a owl:Class ;
    rdfs:label "Military capability"@en ;
    rdfs:comment "MilitaryCapability involves the capacity, ability, or skills/prerequisites/qualifications to accomplish/do something. The thing to be accomplished is defined using event:has_topic and likely is defined as a 'Future' Event. The Actor who is capable is identified using the event:has_active_actor property."@en ;
    general:noun_exemplar "Pursuant to a congressional request, GAO evaluated current measures used by the Department of Defense (DOD) to report [[military capabilities]], focusing on: (1) formal and informal measures of force structure, modernization, readiness, and sustainability; and (2) merits and limitations of those measures."@en ;
    general:noun_exemplar "Recent debates regarding the United Kingdom's defence ambition have highlighted the important question of how to assess [[military capability]]."@en ;
    general:noun_exemplar "The Defense Intelligence Agency (DIA) today released China [[Military Power]], a product that examines the core capabilities of China’s military."@en ;
    rdfs:subClassOf :PreparednessOrCapability, :MilitaryFactor .

:MilitaryCooperation a owl:Class ;
    rdfs:label "Military cooperation"@en ;
    rdfs:comment "MilitaryCooperation may describe either a specific event where two actors work together to achieve a goal, or a general environment of cooperation. A specific Event is defined by also classifying the individual as a type of event:MilitaryAction, while a condition/statistics are also typed as event:Factor, meas:ReportedValue or meas:TimeSeries. A goal of the Cooperation can be defined using the actor:has_objective property.  The Actors that are cooperating are identified using the event:has_active_actor property."@en ;
    rdfs:subClassOf :Cooperation, :MilitaryFactor .
#   owl:equivalentClass oeevent:Cooperate_militarily .

:MilitaryDeescalation a owl:Class ;
    rdfs:label "Military de-escalation"@en ;
    rdfs:comment "MilitaryDeescalation is a reduction in the intensity of a military conflict. If multiple Actors are involved in a Deescalation Event, all are identified as active actors."@en ;
    rdfs:subClassOf :Deescalation, :MilitaryFactor .

:MilitaryExercise a owl:Class ;
    rdfs:label "Military exercise"@en ;
    rdfs:comment "From JP1-02, a MilitaryExercise is 'a military maneuver or simulated wartime operation involving planning, preparation, and execution that is carried out for the purpose of training and evaluation'."@en ;
    rdfs:subClassOf :MilitaryAction .

:MilitaryFactor a owl:Class ;
    rdfs:label "Military factor"@en ;
    rdfs:comment "MilitaryFactor describes the military and/or paramilitary capabilities and activities of all relevant Actors (enemy, friendly, and neutral) in a given operational environment. It is the super-class of specific activities (MilitaryActions), operations (MilitaryCampaignOrOperation), technologies (such as weapons), capabilities (MilitaryCapability), etc. Since the semantics address both Events and Factors, MilitaryFactor is sub-classed from event:EventOrFactor. To describe a general condition related to the military, also classify an individual using event:Factor. If the semantics deal with individual statistics or time series, then the individual is also classified using meas:ReportedValue or meas:TimeSeries."@en ;
    rdfs:subClassOf :EventOrFactor .

:MilitaryOccupation a owl:Class ;
    rdfs:label "Military occupation"@en ;
    rdfs:comment "MilitaryOccupation is a MilitaryFactor/'condition in which territory is under the effective control of a foreign armed force' (JP1-02)."@en ;
    general:noun_exemplar "Georgian President Salome Zourabishvili says Russia's decadelong [[military occupation]] of South Ossetia and Abkhazia has failed to break the national will to maintain sovereignty and achieve European Union and NATO accession."@en ;
    rdfs:subClassOf :MilitaryFactor .

:MisinformationOperation a owl:Class ;
    rdfs:label "Misinformation operation"@en ;
    rdfs:comment "MisinformationOperations deal with the production, distribution and consumption of inaccurate information. The inaccuracies may be produced intentionally or not (if not, the Operation may also be classified as event:UnintentionalAct). An Operation occurs over time, has specific goals, and is composed of specific, coordinated acts/Events intended to achieve those goals. The component Events (if known) are associated using the general:has_member property. The goal is identified using the actor:has_objective property."@en ;
    rdfs:subClassOf :InformationOperation .

:MissingPersons a owl:Class ;
    rdfs:label "Missing persons"@en ;
    rdfs:comment "MissingPersons are individuals who have disappeared and whose fate/condition are not known. The Actor(s) may have voluntarily chosen to disappear or may be the victim of crimes. The 'missing' Persons are identified as the active actor."@en ;
    general:noun_exemplar "Deputies in Nash County responded to a call of a [[missing person]] report Saturday and saw her car was still at the residence."@en ;
    rdfs:subClassOf :Event .

:Mobilization a owl:Class ;
    rdfs:label "Mobilization"@en ;
    rdfs:comment "From JP1-02, mobilization is '1. The process of assembling and organizing national resources to support national objectives in time of war or other emergencies.' If multiple Actors are involved in a Mobilization Event, all are identified as active actors."@en ;
    rdfs:subClassOf :Event .

:Mortality a owl:Class ;
    rdfs:label "Mortality"@en ;
    rdfs:comment "A Factor providing data (typically, an individual meas:ReportedValue or meas:TimeSeries) about the mortality rates/characteristics of a population or particular sub-groups within it. The population/group whose demographic is reported is identified using the event:has_actor property."@en ;
    rdfs:subClassOf :Demographic .

:MurderOrHomicide a owl:Class ;
    rdfs:label "Murder/homicide"@en ;
    rdfs:comment "MurderOrHomicide deals with the premeditated or unintentional killing of an individual by another. The Actor who performed/caused the killing is the active actor, while the individual who was killed is the affected actor. If the method of death is known (for example, a knife or gun), that can be described using the event:has_instrument property. If the act was unintentional, that can be described by adding the event:UnintentionalAct class."@en ;
    rdfs:subClassOf :Violence , :Death .
#   owl:equivalentClass cco:ActOfHomicide .

:NaturalDisaster a owl:Class ;
    rdfs:label "Natural disaster"@en ;
    rdfs:comment "Any natural phenomenon that has a serious, negative effect on humans or the environment. Examples include earthquakes, landslides, tsunamis, etc."@en ;
    rdfs:subClassOf :EnvironmentalFactor .

:NaturalResources a owl:Class ;
    rdfs:label "Natural resources"@en ;
    rdfs:comment "Deals with the need for or availability of materials or substances such as minerals, forests, water and land."@en ;
    rdfs:subClassOf :EnvironmentalFactor .

:NeedOrRequirement a owl:Class ;
    rdfs:label "Need or requirement (deprecated)"@en ;
    owl:deprecated "true"^^xsd:boolean ;
    rdfs:comment "When using the NeedOrRequirement Event type, it is important to indicate what is needed/required/demanded. This is accomplished using the event:is_about_artifact property to define what is needed (such as a requirement/demand for oil, a Fuel)."@en ;
    rdfs:comment "Note that NeedOrRequirement is deprecated in lieu of using the reification, event:Dependence."@en ;
    rdfs:subClassOf :Factor .

:Negotiation a owl:Class ;
    rdfs:label "Negotiation"@en ;
    rdfs:comment "Negotiation is an ExploratoryCommunication intended to produce an agreement, resolve differences or bring about a settlement between several Actors. The Actors who are negotiating are defined as the active actors. However, if an intermediary is used (such as in an arbitration or mediation), then the arbitrator or mediator is identified as the active actor, while the groups who are arbitrated/mediated are the affected actors. When using the Negotiation Event type, it may be important to indicate what is being negotiated. This is accomplished using the event:has_topic object property."@en ;
    rdfs:subClassOf :ExploratoryCommunication, :MeetingOrEncounter .
#   owl:equivalentClass oeevent:Engage_in_negotiation .

:Neutralization  a owl:Class ;
    rdfs:label "Neutralization"@en ;
    rdfs:comment "Neutralization involves rendering someone or something ineffective or harmless. From JP1-02, to neutralize is to '1. As pertains to military operations, to render ineffective or unusable. 2. To render enemy personnel or materiel incapable of interfering with a particular operation. 3. To render safe mines, bombs, missiles, and booby traps. 4. To make harmless anything contaminated with a chemical agent.'"@en ;
    general:noun_exemplar "The Army has already eradicated much of its stockpile by incineration, which is cheaper per weapon than [[neutralization]]."@en ;
    general:verb_exemplar "Iran said on Saturday it had many options to [[neutralize]] the reimposition of U.S. sanctions on its oil exports."@en ;
    rdfs:subClassOf :ReductionRestrictionOrRemoval .

:NuclearHazard a owl:Class ;
    rdfs:label "Nuclear hazard"@en ;
    rdfs:comment "A sub-class of EnvironmentalHazard defined by JP1-02 as 'dangers associated with the blast, thermal, and radiation effects from nuclear explosion'."@en ;
    general:noun_exemplar "[[Nuclear hazard]] effects can be either initial or residual."@en ;
    rdfs:subClassOf :EnvironmentalHazard .

:OathTaking a owl:Class ;
    rdfs:label "Oath taking"@en ;
    rdfs:comment "An oath is a form of promise regarding future actions or behavior. A synonym is to 'swear'. A statement or text including the words, 'with God as my witness' or 'so help me God' (where 'God' is something sacred to the individual taking the oath), is usually considered an oath."@en ; 
    rdfs:subClassOf :AgreementOrPromise .
#   owl:equivalentClass cco:ActOfOathTaking .

:OccupationOfTerritory a owl:Class ;
    rdfs:label "Occupation of territory"@en ;
    rdfs:comment "OccupationOfTerritory or 'occupied territory' describes that a region is under the authority and control of another GeopoliticalEntitye and (typically, with the support of) their armed (military or para-military) force. Examples of occupied territories are the Golan Heights (occupied and annexed by Israel, from Syria) and Crimea (occupied and annexed by Russia, from Ukraine)."@en ;
    rdfs:subClassOf :Factor .
#   owl:equivalentClass oeevent:Occupy_territory .

:Oligarchy a owl:Class ;
    rdfs:label "Oligarchy"@en ;
    rdfs:comment "Oligarchy is a form of government where a few rulers control the government. These rulers gain their power and maintain their authority as a result of their wealth, family ties, education, military control or another form of influence . Aristocracy is one example of oligarchy."@en; 
    rdfs:subClassOf :GovernmentalFactor .

:Operation a owl:Class ;
    rdfs:label "Operation/coordinated set of activities"@en ;
    rdfs:comment "An Operation occurs over time, has specific goals, and is composed of specific, coordinated acts/Events intended to achieve those goals. The component Events (if known) are associated using the general:has_member property. The goal is identified using the actor:has_objective property."@en ;
    rdfs:comment "From JP1-02, an operation is '1. A sequence of tactical actions with a common purpose or unifying theme. 2. A military action or the carrying out of a strategic, operational, tactical, service, training, or administrative military mission.'"@en ;
    rdfs:subClassOf :CollectionOfEventsOrFactors .

:Ownership a owl:Class ;
    rdfs:label "Ownership, regardless of possession"@en ;
    rdfs:comment "Conveys the semantic of possessing or having the right to possess some goods or property. Although ownership sometimes implies possession, that is not guaranteed. Problems often occur when ownership is disputed, or the Actor possessing an entity is not the same as the Actor that owns it."@en ;
    rdfs:subClassOf :Factor .
#   owl:equivalentClass cco:ActOfOwnership .

:Pardon a owl:Class ;
    rdfs:label "Pardon"@en ;
    rdfs:comment "A Pardon is the act of formally excusing/forgiving a mistake or offense. The Actor granting the pardon is the active actor, while the individual who is pardoned is the affected actor."@en ;
    rdfs:subClassOf :Forgiving, :ReleaseOrParole .

:Parole a owl:Class ;
    rdfs:label "Parole"@en ;
    rdfs:comment "A Parole is a release from prison that entitles the individual to live outside the prison as long as they comply with the terms of the release. The Actor granting the parole is the active actor, while the individual who is paroled is the affected actor."@en ;
    rdfs:subClassOf :ReleaseOrParole .

:PaymentOrRepayment a owl:Class ;
    rdfs:label "Payment or repayment"@en ;
    rdfs:comment "PaymentOrRepayment is an act of reimbursing an Actor for a services, goods or monies. The payer is the active actor, while the Actor who is paid is the affected actor. If the payment/repayment is for services (a previous or future Event), that Event is indicated using the event:has_topic property. If for goods, then the Artifact is specified using general:involves_goods_or_property."@en ;
    rdfs:subClassOf :Event .

:Peace a owl:Class ;
    rdfs:label "Peace"@en ;
    rdfs:comment "Describes a lack of conflict or aggression. It is usually defined for a GeopoliticalEntity (such as a country or city) or location. Both are types of locations and are identified using the general:located_at property."@en ;
    rdfs:subClassOf :LivingCondition .

:Peacekeeping a owl:Class ;
    rdfs:label "Peacekeeping activity"@en ;
    rdfs:comment "From JP1-02, peacekeeping involves 'military operations undertaken, with the consent of all major parties to a dispute, designed to monitor and facilitate implementation of an agreement (ceasefire, truce, or other such agreement) and support diplomatic efforts to reach a long-term political settlement.' Note that the concept of PeacekeepingOperation is distinct from a PeacekeepingActivity. Note that an individual PeacekeepingActivity may indeed be part of an PeacekeepingOperation."@en ;
    rdfs:subClassOf :MilitaryAction .

:PeacekeepingOperation a owl:Class ;
    rdfs:label "Peacekeeping operation"@en ;
    rdfs:comment "A PeacekeepingOperation is a coordinated set of activities undertaken to maintain peace in a region. An Operation occurs over time, has specific goals, and is composed of specific, coordinated acts/Events intended to achieve those goals. The component PeacekeepingActivities and related events (if known) are associated using the general:has_member property. The goal is identified using the actor:has_objective property. From JP1-02, peacekeeping involves 'military operations undertaken, with the consent of all major parties to a dispute, designed to monitor and facilitate implementation of an agreement (ceasefire, truce, or other such agreement) and support diplomatic efforts to reach a long-term political settlement.' Note that the concept of PeacekeepingOperation is distinct from a Peacekeeping activity. Note that an individual PeacekeepingActivity may indeed be part of an PeacekeepingOperation."@en ;
    rdfs:subClassOf :MilitaryCampaignOrOperation, :ProtectionOrPreservation .
#   owl:equivalentClass oeevent:Provide_military_protection_or_peacekeeping .

:Performance a owl:Class ;
    rdfs:label "Performance"@en ;
    rdfs:comment "A sub-class of an EntertainmentEvent related to setting up for and presenting a live musical, acting, dance or vocal show/concert/enactment/..."@en ;
    rdfs:subClassOf :EntertainmentEvent .

:Permission a owl:Class ;
    rdfs:label "Permission"@en ;
    rdfs:comment "Permission is a kind of Communication giving approval to do something. When using the Permission Event type, it is important to indicate who/what is being permitted. This is accomplished using the event:has_affected_actor and event:has_topic object properties."@en ;
    rdfs:subClassOf :DirectiveCommunication .

:PersonalCommunication a owl:Class ;
    rdfs:label "Personal communication"@en ;
    rdfs:comment "PersonalCommunication deals with the means that an Actor uses to communicate with others. Its sub-classes describe communicating via conferencing technology (such as Skype), via written materials (such as a letter, email or instant message), or via phone."@en ;
    rdfs:subClassOf :Event .

:PersonalLifeEvent a owl:Class ;
    rdfs:label "Personal life event"@en ;
    rdfs:comment "Examples of PersonalLifeEvents include birth, marriage, graduation and death."@en ;
    rdfs:subClassOf :Event .

:PersonalOrPassengerTransportation a owl:Class ;
    rdfs:label "Travel and transportation of one or more persons"@en ;
    rdfs:comment "PersonalOrPassengerTransportation describes moving people by air, ground or naval vessels/vehicles. To specify the mode of transportion, use event:has_instrument. To identify the Actors doing the transportation and being transported, use event:has_active_actor and event:has_affected_actor, respectively. To define the origin and destination, use the event:has_origin/destination properties. Examples of PersonalOrPassengerTransportation are walking, or using a plane, bus, train, car, etc."@en ;
    rdfs:subClassOf :LocationChange .
#   owl:equivalentClass cco:ActOfTravel .

:Pilgrimage a owl:Class ;
    rdfs:label "Pilgrimage"@en ;
    rdfs:comment "A journey/travel to a special or sacred place."@en ;
    rdfs:subClassOf :PersonalOrPassengerTransportation .
#   owl:equivalentClass cco:ActOfPilgrimage .

:PlacementAsHumanShield a owl:Class ;
    rdfs:label "Placement as human shield"@en ;
    rdfs:comment "PlacementAsHumanShield describes 'the deliberate placement of non-combatants in or around combat targets to deter the enemy from attacking these combat targets. It may also refer to the use of persons to literally shield combatants during attacks, by forcing them to march in front of the combatants.' (https://en.wikipedia.org/wiki/Human_shield)"@en ;
    rdfs:subClassOf :WarCrime .
#   owl:equivalentClass oeevent:Use_as_human_shield .

:PhysicalAssault a owl:Class ;
    rdfs:label "Physical assault"@en ;
    rdfs:comment "An offensive act intended to physically harm an Actor or damage a location. The Actor taking the offensive/doing the attacking is the active actor, while the Actor that is attaked is the affected actor. If the attack is directed at a location, that is identified using the general:located_at property."@en ;
    rdfs:subClassOf :Attack .

:PhysicalMeasurement a owl:Class ;
    rdfs:label "Physical measurement"@en ;
    rdfs:comment "A Factor that is a PhysicalMeasurement reporting on properties such as temperature, pressure, speed, etc. (physical properties). It defines the measurement/reading from a sensor or as noted in a document. The measurement is a kind of TimeSeriesAndMeasurements ontology's ReportedValue class and is related using the has_topic property."@en ;
    rdfs:subClassOf :Factor .

:PhysicalSecurity a owl:Class ;
    rdfs:label "Physical security"@en ;
    rdfs:comment "PhysicalSecurity is about providing access control and/or protecting people and property, and includes camera surveillance, protective barriers, locks, access control protocols, ... (indicated using the event:has_instrument property), or security guards (indicated using the event:has_active_actor property referencing a GroupOfPersons with the general:position_or_role of wiki/Security_guard). The location whose security is described is indicated using the general:located_at property."@en ;
    rdfs:comment "From JP1-02, PhysicalSecurity is '1. That part of security concerned with physical measures designed to safeguard personnel; to prevent unauthorized access to equipment, installations, material, and documents; and to safeguard them against espionage, sabotage, damage, and theft. 2. In communications security, the component that results from all physical measures necessary to safeguard classified equipment, material, and documents from access thereto or observation thereof by unauthorized persons.'"@en ;
    rdfs:subClassOf :Factor .

:PhysicalSeparation a owl:Class ;
    rdfs:label "Physical separation"@en ;
    rdfs:comment "Indicates that there is some distance between Actors (such as GeopoliticalEntities) or Artifacts. Examples are the existence of a buffer zone between two countries or distance between facilities. The locations are indicated using the general:located_at property."@en ;
    rdfs:subClassOf :Factor .

:Planning a owl:Class ;
    rdfs:label "Planning"@en ;
    rdfs:comment "Planning describes any acts of defining a program or course of action, laying out of how a program/project will proceed, or what to do if/when an Event occurs. From JP1-02, Planning is performed to 'to solve problems related to a specific task or requirement'."@en ;
    rdfs:subClassOf :Event .
#   owl:equivalentClass cco:ActOfPlanning .

:PolicyChange a owl:Class ;
    rdfs:label "Policy change"@en ;
    rdfs:comment "A reversal or change in attitude, principle or point of view."@en ;
    rdfs:subClassOf :Event .

:PoliticalDissent a owl:Class ;
    rdfs:label "Political dissent"@en ;
    rdfs:comment "PoliticalDissent can be a specific Event (such as a protest indicating dissent) or a general state of affairs. If the latter, then the Event individual can also be classified using event:Factor."@en ;
    rdfs:subClassOf :PoliticalFactor .

:PoliticalFactor a owl:Class ;
    rdfs:label "Political factor"@en ;
    rdfs:comment "PoliticalFactor describes both specific activities and general conditions regarding governance in a region (including describing the distribution of responsibility and power at all levels of governance). It includes Actors who are formally constituted authorities, as well as informal or covert political parties. Since the semantics address both Events and Factors, PoliticalFactor is sub-classed from event:EventOrFactor. To describe a general condition, also classify an individual using event:Factor. If the semantics deal with individual statistics or time series, then the individual is also classified using meas:ReportedValue or meas:TimeSeries."@en ;
    rdfs:subClassOf :EventOrFactor .

:PoliticalInstability a owl:Class ;
    rdfs:label "Political instability"@en ;
    rdfs:comment "PoliticalInstability is a Factor describing overall conditions in a region/GeopoliticalEntity. It 'can be defined in at least three ways. A first approach is to define it as the propensity for regime or government change. A second is to focus on the incidence of political upheaval or violence in a society, such as assassinations, demonstrations, and so forth. A third approach focuses on instability in policies rather than instability in regimes (i.e., the degree to which fundamental policies of, for instance, property rights are subject to frequent changes).' (https://www.encyclopedia.com/social-sciences/applied-and-social-sciences-magazines/political-instability-indices)"@en ;
    owl:disjointWith :PoliticalStability ;
    rdfs:subClassOf :PoliticalFactor .

:PoliticalReform a owl:Class ;
    rdfs:label "Political reform"@en ;
    rdfs:comment "PoliticalReform can be a specific Event (such as a specific change of a law) or a general environment fostering reform. If the latter, then the Event individual should also be classified using event:Factor."@en ;
    rdfs:subClassOf :PoliticalFactor .

:PoliticalRevolution a owl:Class ;
    rdfs:label "Political revolution"@en ;
    rdfs:comment "A PoliticalRevolution is the overthrow of a government. It describes the specific events of an overthrow or the general environment where a revolution is imminent or has recently occurred (with its associated period of transition)."@en ;
    rdfs:subClassOf :PoliticalFactor .

:PoliticalSecrecy a owl:Class ;
    rdfs:label "Political secrecy"@en ;
    rdfs:comment "PoliticalSecrecy is obfuscation, and lack of accountability and openness regarding governmental and political activities and conditions."@en ;
    owl:disjointWith :PoliticalTransparency ;
    rdfs:subClassOf :Secrecy, :PoliticalFactor .

:PoliticalStability a owl:Class ;
    rdfs:label "Political stability"@en ;
    rdfs:comment "PoliticalStability is a Factor describing overall conditions in a region/GeopoliticalEntity. It is related to predictability of governance, but can be further clarified since a totalitarian government is stable but unjust. PoliticalStability can be further clarified 'in the context of growth ... [as] the rule of law, strong institutions rather than powerful individuals, a responsive and efficient bureaucracy, low corruption and a business climate that is conducive to investment' (can be defined in at least three ways. A first approach is to define it as the propensity for regime or government change. A second is to focus on the incidence of political upheaval or violence in a society, such as assassinations, demonstrations, and so forth. A third approach focuses on instability in policies rather than instability in regimes (i.e., the degree to which fundamental policies of, for instance, property rights are subject to frequent changes).' (http://www.lse.ac.uk/internationalRelations/dinamfellow/docs/dinamshepherdpoliticalstability.pdf)"@en ;
    rdfs:subClassOf :PoliticalFactor .

:PoliticalTransparency a owl:Class ;
    rdfs:label "Political transparency"@en ;
    rdfs:comment "PoliticalTransparency is clarity, lack of obfuscation, accountability and openness regarding governmental and political activities and conditions."@en ;
    rdfs:subClassOf :Transparency, :PoliticalFactor .

:Pollution a owl:Class ;
    rdfs:label "Pollution"@en ;
    rdfs:comment "Pollution addresses both the act of contaminating the environment and the condition of the environment being contaminated by harmful substances. Individuals can represent specific events or general conditions/factors/statistics. When defining general conditions or statistics, an individual should also be classified using event:Factor, meas:ReportedValue or meas:TimeSeries."@en ;
    rdfs:subClassOf :EnvironmentalHazard .

:Possession a owl:Class ;
    rdfs:label "Possession, regardless of ownership."@en ;
    rdfs:comment "Conveys the semantic of possessing some goods or property. Although ownership sometimes implies possession, that is not guaranteed. Problems often occur when the Actor possessing an entity is not the same as the Actor that owns it."@en ;
    rdfs:subClassOf :Factor .
#   owl:equivalentClass cco:ActOfPossession .

:Poverty a owl:Class ;
    rdfs:label "Poverty"@en ;
    rdfs:comment "An EconomicCondition describing that a region or population has little or no money and few or no possessions."@en ;
    rdfs:subClassOf :EconomicCondition .

:PowerBalance a owl:Class ;
    rdfs:label "Power balance"@en ;
    rdfs:comment "Indicates whether the Actors (referenced using the event:has_actor property) have roughly equivalent influence/power"@en ;
    rdfs:subClassOf :Factor .

:PraisingOrEndorsing a owl:Class ;
    rdfs:label "Praising or endorsing"@en ;
    rdfs:comment "PraisingOrEndorsing deals with any expressions of approval or commendation. When using this Event type, it is important to indicate who/what is being praised or endorsed. This is accomplished using the event:has_affected_actor, event:has_topic or general:involves_goods_or_property object properties (referencing an Actor, an act/event or a thing)."@en ;
    rdfs:subClassOf :DefenseOrSupport .
#   owl:equivalentClass oeevent:Praise_or_endorse .

:PreparednessOrCapability a owl:Class ;
    rdfs:label "Preparedness or capability"@en ;
    rdfs:comment "Describes that an Actor (such as a GeopoliticalEntity) has the capacity, ability, or skills/prerequisites/qualifications to accomplish/do something. The thing to be accomplished is defined using event:has_topic and likely is defined as a 'Future' Event. The Actor who is capable is identified using the event:has_active_actor property."@en ;
    rdfs:subClassOf :Factor .

:PriceGouging a owl:Class ;
    rdfs:label "Price gouging"@en ;
    rdfs:comment "PriceGouging is either a specific act of inflating prices or the general condition of inflated prices for commodities and basic necessities, such as could occur due to a shortage after a natural disaster. To describe that price gouging is related to specific goods, associate these using general:involves_goods_or_property (and the Artifact would be defined with the general:generic property set to 'true')."@en ;
    rdfs:subClassOf :Pricing .

:Pricing a owl:Class ;
    rdfs:label "Pricing/prices"@en ;
    rdfs:comment "An EconomicFactor describing the costs of goods or services and/or changes in these costs. The former is typically also classified as a meas:ReportedValue or meas:TimeSeries, and the latter is also typed as an event:Increase/Decrease/Stasis."@en ;
    rdfs:subClassOf :EconomicFactor .

:Pride a owl:Class ;
    rdfs:label "Pride"@en ;
    rdfs:comment "Pride is an EmotionalResponse where an Actor feels self-worth and value (in general) or feels satisfaction with an accomplishment or regarding some situation. The Actor who is proud is identified using the event:has_active_actor property. If the pride is related to a situation or accomplishment, that is identified using the event:has_topic property."@en ;
    rdfs:subClassOf :EmotionalResponse .
#   owl:equivalentClass oeceo:Pride .

:Productivity a owl:Class ;
    rdfs:label "Productivity"@en ;
    rdfs:comment "Productivity is an economic measure describing the ratio of the quality and quantity of outputs to inputs (which include capital, labor and materials) for an organization, GPE or other entity. For example, labor productivity is the ratio of the output of goods and services to the labor hours invested to generate that output. This class describes both increases/decreases in productivity (event:Increase/Decrease/Stasis) as well as specific measurements (meas:ReportedValues and meas:TimeSeries)."@en ;
    rdfs:subClassOf :EconomicFactor .

:ProfitAndLoss a owl:Class ;
    rdfs:label "Profit and loss"@en ;
    rdfs:comment "ProfitAndLoss is an economic measure summarizing the revenues, costs and expenses of an Actor, over a specified period (usually, a fiscal year). This class describes both increases/decreases in profits/losses (event:Increase/Decrease/Stasis) as well as specific measurements (meas:ReportedValues and meas:TimeSeries)."@en ;
    rdfs:subClassOf :EconomicFactor .

:PromotionOfWaterSanitationAndHygiene  a owl:Class ;
    rdfs:label "Promotion of water, sanitation and hygiene improvements"@en ;
    rdfs:comment "Describes a campaign to educate people, helping them to understand and develop the value of water sanitation and good hygience practices. The goal is to prevent disease and death. 'Several community development activities can be used to achieve this goal, including education and learning programmes, encouraging community management of environmental health facilities, and social mobilization and organization. [Water sanitation and] hygiene promotion is not simply a matter of providing information. It is more a dialogue with communities about [sanitation,] hygiene and related health problems, to encourage improved ... practices.' (https://www.who.int/water_sanitation_health/hygiene/settings/hvchap9.pdf)"@en ;
    rdfs:subClassOf :CivilCampaign, :FoodWaterAndNutrition .

:PropagandaActivity a owl:Class ;
    rdfs:label "Propaganda activity"@en ;
    rdfs:comment "Activity dealing with the creation, distribution or consumption of propaganda."@en ;
    rdfs:subClassOf :Deception, :DeclarativeCommunication, :Influence .
#   owl:equivalentClass cco:ActOfPropaganda .

:ProtectionOrPreservation a owl:Class ;
    rdfs:label "Protection or preservation"@en ;
    rdfs:comment "ProtectionOrPreservation is any activity or condition/factor dealing with keeping someone or something free from danger, harm, damage, etc. The Actor doing the protecting is the active actor, while another Actor, Location or Artifact is the entity that is protected. The latter are indicated using the properties, event:has_affected_actor or general:involves_goods_or_property. Note that an entity can protect/preserve itself (i.e., self-preservation) in which case the Actor is both active and affected. Note that ProtectionOrPreservation may describe specific events (such as characterized by its sub-class, event:GuardingOrPatrolling), general conditions such as an increase/decrease in preservation activities in a region (event:Increase/Decrease/Stasis), or statistics (an individual meas:ReportedValue or meas:TimeSeries) related to protection or preservation."@en ;
    general:noun_exemplar "Mines were hidden in the field as [[protection]] against the invading army."@en ;
    general:noun_exemplar "A sense of [[self-preservation]] cautioned her not to stick around."@en ;
    general:verb_exemplar "While serving as director general of GCHQ from 2014 to 2017, Robert Hannigan was at the heart of [[protecting]] the UK from a variety of threats."@en ;
    general:verb_exemplar "[[Protecting]] and [[preserving]] wildlife habitats will also [[protect]] the future of humanity."@en ;
    rdfs:subClassOf :EventOrFactor . 

:ProvisionOfAid a owl:Class ;
    rdfs:label "Provision of aid"@en ;
    rdfs:comment "ProvisionOfAid is any type of transfer of resources between Actors (typically, GeopoliticalEntities or Organizations). The resouce(s) that are transferred can be monetary (loans, grants or contributions), goods, skills or personnel (such as providing health-care or military skills), training, etc. The affected actor is the one receiving the aid. If the goal/objective of providing aid is known, that can be specified using the actor:has_objective property."@en ;
    rdfs:subClassOf :Event . 
#   owl:equivalentClass oeevent:Provide_aid .
# :ProvisionOfAid rdfs:subClassOf cco:EssentialServiceProvision .

:ProvisionOfEconomicAid a owl:Class ;
    rdfs:label "Provision of economic aid"@en ;
    rdfs:comment "ProvisionOfEconomicAid is any type of transfer of economic-related resources between Actors (typically, GeopoliticalEntities or Organizations). The resouce(s) that are transferred can be moneties (loans, grants or contributions), goods, skills or personnel, training, etc. The affected actor is the one receiving the aid. If the goal/objective of providing aid is known, that can be specified using the actor:has_objective property."@en ;
    rdfs:subClassOf :ProvisionOfAid .
#   owl:equivalentClass oeevent:Provide_economic_aid .

:ProvisionOfHumanitarianAid a owl:Class ;
    rdfs:label "Provision of humanitarian aid"@en ;
    rdfs:comment "ProvisionOfHumanitarinAid is any type of transfer of resources between Actors (typically, GeopoliticalEntities or Organizations) for humanitarian reasons and to promote the well-being of a populace. The resouce(s) that are transferred can be monetary (loans, grants or contributions), goods, skills or personnel (such as providing health-care or military skills), training, etc. The affected actor is the one receiving the aid. If the goal/objective of providing aid is known, that can be specified using the actor:has_objective property."@en ;
    rdfs:subClassOf :ProvisionOfAid .
#   owl:equivalentClass oeevent:Provide_humanitarian_aid .

:ProvisionOfInspectorsOrObservers a owl:Class ;
    rdfs:label "Provision of inspectors or observers"@en ;
    rdfs:comment "ProvisionOfInspectorsOrObservers describes providing a Person or GroupOfPersons to record and report on the processes, institutions, laws, etc. related to some Event/Factor (such as an event:Election or event:JailsAndPrisoners). The Event/Factor that is monitored is defined using the event:has_topic property."@en ;
    rdfs:subClassOf :ProvisionOfAid .

:ProvisionOfMilitaryAid a owl:Class ;
    rdfs:label "Provision of military aid"@en ;
    rdfs:comment "ProvisionOfMilitaryAid is any type of transfer of military-related resources between Actors (typically, GeopoliticalEntities  or Organizations). The resouce(s) that are transferred can be monetary (loans, grants or contributions), goods/armaments/..., skills or personnel, training, etc. The affected actor is the one receiving the aid. If the goal/objective of providing aid is known, that can be specified using the actor:has_objective property."@en ;
    rdfs:subClassOf :ProvisionOfAid, :MilitaryFactor .
#   owl:equivalentClass oeevent:Provide_military_aid .

:ProvisionOfMilitaryTrainingSchooling a owl:Class ;
    rdfs:label "Provision of military training or schooling"@en ;
    rdfs:comment "A specific type of military aid related to developing and/or improving the ability of military personnel to perform their duties/roles. Note that the affected actor is the one receiving the aid."@en ;
    rdfs:subClassOf :ProvisionOfTrainingSchooling, :ProvisionOfMilitaryAid .
#   owl:equivalentClass cco:ActOfMilitaryTrainingInstruction .

:ProvisionOfProtectionOrPeacekeepers a owl:Class ;
    rdfs:label "Provision of protection or peacekeepers"@en ;
    rdfs:comment "ProvisionOfProtectionOrPeacekeepers describes providing a Person or GroupOfPersons to maintain peace and security in a region."@en ;
    rdfs:subClassOf :ProvisionOfAid .

:ProvisionOfReligiousTrainingSchooling a owl:Class ;
    rdfs:label "Provision of religious training or schooling"@en ;
    rdfs:comment "Training in the practices and beliefs of a specific religion. The religion is defined by relating an oereligion:Religion sub-class with the active Actor(s), using the actor:has_affiliation property."@en ;
    rdfs:subClassOf :ProvisionOfTrainingSchooling .
#   owl:equivalentClass cco:ActOfReligiousTrainingInstruction .

:ProvisionOfTerroristTrainingSchooling a owl:Class ;
    rdfs:label "Provision of terrorist training or schooling"@en ;
    rdfs:comment "Training in skills to carry out terrorist activities. The terrorist organization is defined as the active actor."@en ;
    rdfs:subClassOf :ProvisionOfTrainingSchooling .
#   owl:equivalentClass cco:ActOfTerroristTrainingInstruction .

:ProvisionOfTrainingSchooling a owl:Class ;
    rdfs:label "Provision of training or schooling"@en ;
    rdfs:comment "ProvisionOfTrainingSchooling is any type of transfer of education-related resources between Actors (typically, GeopoliticalEntities or Organizations). The resouce(s) that are transferred can be monetary (loans, grants or contributions), skills or personnel, etc. The affected actor is the one receiving the aid."@en ;
    rdfs:subClassOf :ProvisionOfAid, :EducationAndTraining .
#   owl:equivalentClass cco:ActOfTrainingInstruction .

:ProvisionOfVocationalTrainingSchooling a owl:Class ;
    rdfs:label "Provision of vocational training or schooling"@en ;
    rdfs:comment "A specific type of training to acquire the skills of a trade (such as being an electrical or auto repair technician, dental/medical assistant, etc.). The various types of training can be defined using the general:position_or_role property."@en ;
    rdfs:subClassOf :ProvisionOfTrainingSchooling .
#   owl:equivalentClass cco:ActOfVocationalTrainingInstruction .

:PsychologicalAttack a owl:Class ;
    rdfs:label "Psychological attack"@en ;
    rdfs:comment "A PsychologicalAttack is intended to cause emotional harm/damage. Note that an individual PsychologicalAttack may be a component of an InformationOperation. In this case, it would be a sub-event of that Operation."@en ;
    rdfs:subClassOf :Attack .

:PublicTransportation a owl:Class ;
    rdfs:label "Public transportation availability/access, issues, etc."@en ;
    rdfs:comment "PublicTransportation '(also known as public [transport], public transit, or mass transit) is transport of passengers by group travel systems available for use by the general public, typically managed on a schedule, operated on established routes, and that charge a posted fee for each trip. Examples of public transport include city buses, trolleybuses, trams (or light rail) and passenger trains, rapid transit (metro/subway/underground, etc.) and ferries. Public transport between cities is dominated by airlines, coaches, and intercity rail.' (https://en.wikipedia.org/wiki/Public_transport) Individuals may describe specific events concerning transporation facilities, infrastructure and services, their general conditions (event:Factor and/or event:Increase/Decrease/Stasis), or various statistics (meas:ReportedValues and meas:TimeSeries)."@en ;
    rdfs:subClassOf :InfrastructureAndUtilities .

:Purchasing a owl:Class ;
    rdfs:label "Purchasing"@en ;
    rdfs:comment "Purchasing describes specific events (such as a paramilitary organization buying ammunitions), general conditions describing increases/decreases in purchasing in a region or for a populace  (event:Increase/Decrease/Stasis) or statistics (an individual meas:ReportedValue or meas:TimeSeries) related to purchases/buying. Because the semantics can address either events or conditions/factors, it is defined as a subclass of event:EventOrFactor."@en ;
    rdfs:subClassOf :EventOrFactor .
#   owl:equivalentClass cco:ActOfPurchasing .

:RadiologicalHazard a owl:Class ;
    rdfs:label "Radiological hazard"@en ;
    rdfs:comment "A sub-class of EnvironmentalHazard defined by JP1-02 as 'ionizing radiation that can cause damage, injury, or destruction from either external irradiation or due to radiation from radioactive materials within the body'."@en ;
    general:noun_exemplar "The World Health Organization (2011) says [[radiological hazards]] in food would have to be consumed over a period of time to present a risk."@en ;
    rdfs:subClassOf :EnvironmentalHazard .

:Raid a owl:Class ;
    rdfs:label "Raid"@en ;
    rdfs:comment "Raid characterizes any activities related to surprise attacks on an Actor or Location, search without warning, and/or the taking of goods related to such an attack. From JP1-02, a Raid is 'an operation to temporarily seize an area to secure information, confuse an enemy, capture personnel or equipment, or to destroy a capability culminating with a planned withdrawal'."@en ;
    rdfs:subClassOf :Attack .

:RainfallAndRunoff a owl:Class ;
    rdfs:label "Rainfall and runoff"@en ;
    rdfs:comment "A WeatherIssue providing data (typically, an individual meas:ReportedValue or meas:TimeSeries) on the amount or surplus/overflow of rain in a GPE or region. The Location is identified using the general:located_at property."@en ;
    rdfs:subClassOf :WeatherIssue .

:RallyingOpposition a owl:Class ;
    rdfs:label "Rallying opposition"@en ;
    rdfs:comment "Any activity involved with generating opposition to something, someone or some (likely, 'Future') Event. It can be specified (for example) as the objective (actor:has_objective) of an event:IssuingPublishingOrReleasing individual or an event:DemonstrationOrProtest entity. The something/someone/Event can be identified by associating an Artifact, Actor or Event using event:involves_goods_or_property, event:has_affected_actor or event:has_topic properties."@en ;
    owl:disjointWith :RallyingSupport ;
    rdfs:subClassOf :DisapprovalOrDenunciation .

:RallyingSupport a owl:Class ;
    rdfs:label "Rallying support"@en ;
    rdfs:comment "Any activity involved with generating opposition for something, someone or some (likely, 'Future') Event. It can be specified (for example) as the objective (actor:has_objective) of an event:IssuingPublishingOrReleasing individual or an event:DemonstrationOrProtest entity. The something/someone/Event can be identified by associating an Artifact, Actor or Event using event:involves_goods_or_property, event:has_affected_actor or event:has_topic properties."@en ;
    rdfs:subClassOf :DefenseOrSupport .

:Receipt a owl:Class ;
    rdfs:label "Receipt"@en ;
    rdfs:comment "Just as there are ProvisionOfXxx Event classes, there is a Receipt Event. This is for cases where something is received over the course of time, or when it is necessary to record a concept such as 'receipt of the prisoners'."@en ;
    rdfs:subClassOf :Event .

:ReceiptOfAid a owl:Class ;
    rdfs:label "Receipt of aid"@en ;
    rdfs:comment "ReceiptOfAid is any receipt of resources from another Actor (typically, GeopoliticalEntities or Organizations). The resouce(s) that are received can be monetary (loans, grants or contributions), goods, skills or personnel (such as providing health-care or military skills), training, etc. The active actor is the one receiving the aid. If the goal/objective of providing aid is known, that can be specified using the actor:has_objective property."@en ;
    rdfs:subClassOf :Receipt .

:Reconnaissance a owl:Class ;
    rdfs:label "Reconnaissance activity"@en ;
    rdfs:comment "From JP1-02, reconnaissance is 'a mission undertaken to obtain, by visual observation or other detection methods, information about the activities and resources of an enemy or adversary, or to secure data concerning the meteorological, hydrographic, or geographic characteristics of a particular area'. Note that the concept of ReconnaissanceOperation is distinct from a Reconnaissance activity. Note that an individual ReconnaissanceActivity may indeed be part of an ReconnaissanceOperation."@en ;
    rdfs:subClassOf :MilitaryAction, :InformationHandling .

:ReconnaissanceOperation a owl:Class ;
    rdfs:label "Reconnaissance operation"@en ;
    rdfs:comment "A ReconnaissanceOperation is a sub-class of Operation dealing any type of information gathering about an Actor or region. An Operation occurs over time, has specific goals, and is composed of specific, coordinated acts/Events intended to achieve those goals. The component ReconnaissanceActivities and related events (if known) are associated using the general:has_member property. The goal is identified using the actor:has_objective property. From JP1-02, reconnaissance is 'a mission undertaken to obtain, by visual observation or other detection methods, information about the activities and resources of an enemy or adversary, or to secure data concerning the meteorological, hydrographic, or geographic characteristics of a particular area'. Note that the concept of ReconnaissanceOperation is distinct from a ReconnaissanceActivity. Note that an individual ReconnaissanceActivity may indeed be part of an ReconnaissanceOperation."@en ;
    rdfs:subClassOf :InformationHandling, :MilitaryCampaignOrOperation .

:RecoveryOrRescue a owl:Class ;
    rdfs:label "Recovery or rescue"@en ;
    rdfs:comment "Note that RecoveryOrRescue of material goods can be described by an associated Artifact, using the property, general:involves_goods_or_property, while the rescue of people is described by associating a GroupOfPersons as the affected actor. From JP1-02, recovery is '1. In air (aviation) operations, that phase of a mission that involves the return of an aircraft to a land base or platform afloat. 2. The retrieval of a mine from the location where emplaced. 3. In personnel recovery, actions taken to physically gain custody of isolated personnel and return them to friendly control. 4. Actions taken to extricate damaged or disabled equipment for return to friendly control or repair at another location.'"@en ;
    rdfs:subClassOf :Event .

:RecruitmentActivity a owl:Class ;
    rdfs:label "Recruitment activity"@en ;
    rdfs:comment "A RecruitmentActivity is any action intended to enlist new individuals in a GroupOfActors."@en ;
    rdfs:subClassOf :RallyingSupport .

:RecruitmentOperation a owl:Class ;
    rdfs:label "Recruitment operation"@en ;
    rdfs:comment "A RecruitmentOperation is about specific sets of activities to garner new members in a Group, such as a militant/military, religious and/or political group. Note that an Operation occurs over time, has specific goals, and is composed of specific, coordinated acts/Events intended to achieve those goals. The component Events (if known) are associated using the general:has_member property. The goal is identified using the actor:has_objective property. Also, an individual RecruitmentActivity may be a component of a RecruitmentOperation. In this case, it would be associated using general:has_member."@en ;
    rdfs:subClassOf :Operation, :RallyingSupport .

:ReductionRestrictionOrRemoval a owl:Class ;
    rdfs:label "Reduction, restriction or removal"@en ;
    rdfs:comment "ReductionRestrictionOrRemoval characterizes any act intended to decrease, reduce, take away, dispose of or discard something or the quantity/quality of some Actor. The entity doing the reduction/removal is the active actor, while the thing or Actor that is decreased/reduced/... is defined using the general:involves_goods_or_property or event:has_affected_actor properties. To indicate that various locations were involved in the reduction/removal/restriction, use the general:located_at property, or its more specific event:has_origin/destination sub-properties."@en ;
    rdfs:subClassOf :Event .

:ReforestationLandUse a owl:Class ;
    rdfs:label "Reforestation land use"@en ;
    rdfs:comment "ReforestationLandUse describes how land is replanted (with trees) after a fire, cutting or other destructive event. It describes both specific acts, and general details/factors."@en ;
    rdfs:subClassOf :LandUse .

:RefusalOrRejection a owl:Class ;
    rdfs:label "Refusal or rejection"@en ;
    rdfs:comment "RefusalOrRejection characterizes any act where an Actor does not accept or acknowledge something, some offer or someone. When using the RefusalOrRejection Event type, it is important to indicate who/what is being/was rejected. This is accomplished using the event:has_affected_actor and event:has_topic object properties."@en ;
    rdfs:subClassOf :DeclarativeCommunication .
#   owl:equivalentClass cco:ActOfDenying, oeevent:Reject .

:ReleaseOrParole a owl:Class ;
    rdfs:label "Release or parole"@en ;
    rdfs:comment "ReleaseOrParole is any act of freeing someone or something (from confinement). This class would be used (for example) if an individual's release from prison was not known to be related to their completing their sentence, a parole or a pardon. If the more explicit semantics of event:Pardon or event:Parole are known, then one of those classes should be used instead. The individual who is released is the affected actor."@en ;
    rdfs:subClassOf :ReturnOrRelease .

:RelevanceOrImportance a owl:Class ;
    rdfs:label "Relevance or importance"@en ;
    rdfs:comment "Identifies the relevance/importance of some Event/Factor, Actor or Artifact, (optionally) based on the perspective of some Actor. The Actor whose perspective is considered is identified using event:has_actor, while the thing that is important is identified using event:has_topic, event:has_affected_actor or general:involves_goods_or_property (for Events/Factors, Actors or Artifacts, respectively)."@en ;
    rdfs:subClassOf :Factor .

:ReligiousCeremonyOrWorship a owl:Class ;
    rdfs:label "Religious ceremony or worship"@en ;
    rdfs:comment "Describes a religious event or act of public worship (or a portion of that event) that follows prescribed formats/rules."@en ;
    rdfs:subClassOf :Ceremony .
#   owl:equivalentClass cco:ActOfReligiousWorship .

:ReligiousOrPoliticalBeliefs a owl:Class ;
    rdfs:label "Religious or political beliefs"@en ;
    rdfs:comment "Indicates the presence of various religious or political beliefs in an area or the beliefs held by a population/group of people. The area is defined using the general:located_at property, while the population/group is defined using event:has_actor. The belief(s) are defined for the Location or Actor using actor:has_affiliation/ethnicity/political_orientation."@en ;
    rdfs:subClassOf :Factor .

:ReportAsMissing a owl:Class ;
    rdfs:label "Report as missing"@en ;
    rdfs:comment "ReportAsMissing is a Communication conveying that someone or something has disappeared and whose fate/condition not known. The Actor doing the reporting is the active actor. The entity that is reported as missing may be identified using either general:involves_goods_or_property or event:has_affected_actor."@en ;
    rdfs:subClassOf :Reporting .

:Reporting a owl:Class ;
    rdfs:label "Reporting"@en ;
    rdfs:comment "Reporting characterizes any act of informing, describing, accounting for or representing something or someone. When using the Reporting Event type (or one of its sub-classes), it is important to indicate who/what is being reported. This is accomplished using the event:has_affected_actor, general:involves_goods_or_property and event:has_topic object properties."@en ;
    rdfs:subClassOf :DeclarativeCommunication .
#   owl:equivalentClass cco:ActOfReporting .

:RepresentativeCommunication a owl:Class ;
    rdfs:label "Representative communication (deprecated)"@en ;
    owl:deprecated "true"^^xsd:boolean ;
    rdfs:comment "Deals with any communication which represents the Actors' opinions - accusations, claims/denials of responsibility, defending or supporting/disapproving or denouncing someone or something, vetoes, appraisals, reports, etc. (whether what is declared is 'true' or 'false' is not considered). This class is deprecated in lieu of using the similar event:DeclarativeCommunication class. When instantiating RepresentativeCommunication, it is important to indicate what are the topic(s) of the communication. This is accomplished using the event:has_affected_actor, event:has_topic or general:involves_goods_or_property object properties (referencing an Actor, an act/event or a thing, respectively)."@en ;
    owl:equivalentClass :DeclarativeCommunication ;
    rdfs:subClassOf :Communication .

:Repression a owl:Class ;
    rdfs:label "Repression"@en ;
    rdfs:comment "Repression can be a specific Event (such as repression of a riot) or a general state of affairs. If the latter, then the Event individual should also be classified using event:Factor."@en ;
    rdfs:subClassOf :EventOrFactor .

:RequestAppealOrDemand a owl:Class ;
    rdfs:label "Request, appeal or demand"@en ;
    rdfs:comment "Deals with either a request or a demand, when it is not known which was communicated. When using the RequestAppealOrDemand Event type, it is important to indicate who/what is being requested/demanded. This is accomplished using the event:has_affected_actor and event:has_topic object properties."@en ;
    rdfs:subClassOf :Communication ;
    owl:equivalentClass [ a owl:Class ;
                          owl:unionOf ( :RequestOrAppeal :Demand ) ] .

:RequestOrAppeal a owl:Class ;
    rdfs:label "Request or appeal"@en ;
    rdfs:comment "RequestOrAppeal characterizes any Communication that expresses a need or desire for something (including information), someone or that some Event occur. When using the RequestOrAppeal Event type, it is important to indicate who/what is being requested. This is accomplished using the general:involves_goods_or_property, event:has_affected_actor or event:has_topic object properties."@en ;
    rdfs:subClassOf :Communication .
#   owl:equivalentClass cco:ActOfRequesting, oeevent:Appeal .

:RequestOrAppealForAsylum a owl:Class ;
    rdfs:label "Request or appeal for asylum"@en ;
    rdfs:comment "RequestOrAppealForAsylum is a sub-class of RequestOrAppeal. It indicates that an Actor has asked (or intends to ask) a GPE to allow them to remain on its territory, at its embassies, on its vessels, or in a similar location because they cannot return to their home country. This may be because of persecution or a fear of persecution due to ethnicity, religion, nationality, affiliations, etc. The UNHCR Refugee Agency describes various distinctions of the term, asylum. 'The term 'diplomatic asylum' in the broad sense is used to denote asylum granted by a State outside its territory, particularly in its diplomatic missions (diplomatic asylum in the strict sense), in its consulates, on board its ships in the territorial waters of another State (naval asylum), and also on board its aircraft and of its military or para-military installations in foreign territory. The other form of asylum granted to individuals, namely, that which is granted by the State within its borders, is generally given the name 'territorial asylum'. The terminology employed in this entire field lacks uniformity. The terms 'internal asylum', 'external asylum' and 'political asylum' are used by some to denote diplomatic asylum and by others to refer to territorial asylum. The State in whose territory diplomatic asylum is sought is know as the 'local' or 'territorial' State ... while the person granted asylum may be called either a 'refugee' or an 'asylee'.' (https://www.unhcr.org/protection/historical/3ae68bf10/question-diplomatic-asylum-report-secretary-general.html)"@en ;
    rdfs:subClassOf :RequestOrAppeal .

:ResistanceRebellionOrUprising a owl:Class ;
    rdfs:label "Resistance, rebellion, revolt or uprising"@en ;
    rdfs:comment "ResistanceRebellionOrUprising defines organized opposition to a government/GeopoliticalEntity or some authority. It may involve the taking of control from the authority. ResistanceRebellionOrUprising may or may not be violent. If it is, also add the :Violence classification to the Event individual."@en ;
    rdfs:subClassOf :Event .

:RespectForRightsFreedoms a owl:Class ;
    rdfs:label "Respect for human rights and political freedoms"@en ;
    rdfs:comment "Fundamental rights (as defined by the United Nations) include the right to self-determination, liberty, due process and peaceful assembly/freedom of association, as well as freedom of thought, religion, movement and expression. This class deals with events/conditions that permit, encourage or strengthen individual freedoms by the government, military, law enforcement or social groups. It includes passing laws, prosecuting abuses, and actively supporting rights and freedoms. RespectForRightsFreedoms may describe either a specific event, or a general environment of respect. When defining general conditions or statistics, an individual should also be classified using event:LivingCondition, meas:ReportedValue or meas:TimeSeries."@en ;
    rdfs:subClassOf :EventOrFactor .

:Restoration a owl:Class ;
    rdfs:label "Restoration"@en ;
    rdfs:comment "Restoration deals with the return of something to a previous owner, to a previous location or to a previous condition. For a previous owner, the owner is defined as the affected actor, and the 'thing' is defined using the general:involves_goods_or_property predicate. For a previous location, the Restoration event is also a LocationChange where the 'restored' location is identified using the event:has_destination property, the origin (if known) is defined using the event:has_origin property, and the 'thing' is either an active or affected Actor (if restoring people to their homes) or an Artifact identified using general:involves_goods_or_property. For a previous condition, the Restoration event could reference another event that defines the loss/change of the condition, using the event:preceded_by property."@en ;
    rdfs:subClassOf :ReturnOrRelease .

:Retreat a owl:Class ;
    rdfs:label "Retreat"@en ;
    rdfs:comment "Retreat mostly describes military acts of withdrawing/moving troops to a different location to escape an enemy's forces or after a defeat, or to initial signal given to begin a retreat. However, the class can also be used to characterize any act of removing oneself or another Actor to escape something dangerous or unpleasant, or to be alone/to mediate/to study/..."@en ;
    rdfs:subClassOf :ReductionRestrictionOrRemoval .
#   rdfs:subClassOf oeevent:Retreat_or_surrender_militarily .

:RetreatSurrenderOrYielding a owl:Class ;
    rdfs:label "Retreat, surrender or yielding"@en ;
    rdfs:comment "This class is used when the exact nature or reason for cessation of fighting is unknown. The class is a union of event:Retreat and event:SurrenderOrYielding."@en ;
    rdfs:subClassOf :Event ;
    owl:equivalentClass [ a owl:Class ;
                          owl:unionOf ( :Retreat :SurrenderOrYielding ) ] .
# oeevent:Retreat_or_surrender_militarily rdfs:subClassOf :RetreatSurrenderOrYielding .

:ReturnOrRelease a owl:Class ;
    rdfs:label "Return or release"@en ;
    rdfs:comment "ReturnOrRelease deals with any action to restore something to its original owner or location, to grant freedom to someone or something or to let fall/spill/drop from something. Note that ReturnOrRelease of material goods or property can be described by an associated Artifact, using the predicate, general:involves_goods_or_property, while the return/release of people is described by associating a GroupOfPersons as the affected actor. Sub-classes of ReturnOrRelease include event:ReleaseOrParole and event:Restoration."@en ;
    rdfs:subClassOf :Event .
#   owl:equivalentClass oeevent:Return\,_release .

:Revenue a owl:Class ;
    rdfs:label "Revenue"@en ;
    rdfs:comment "An EconomicFactor describing the income from conducting business, usually from the sale of goods or services (where the instance is also classified as a meas:ReportedValue or meas:TimeSeries), or changes in revenue (where entities are also classified as event:Increase/Decrease/Stasis). Instances of type, Revenue, may deal with specific artifacts that can be identified using the general:involves_goods_or_property predicate."@en ;
    rdfs:subClassOf :EconomicFactor .

:Riot a owl:Class ;
    rdfs:label "Riot/violent protest"@en ;
    rdfs:comment "A Riot is an act of violence by an unruly mob or a state of disorder involving group violence."@en ;
    rdfs:subClassOf :DemonstrationOrProtest, :Violence .
#   owl:equivalentClass oeevent:Protest_violently\,_riot .

:Risk a owl:Class ;
    rdfs:label "Risk"@en ;
    rdfs:comment "A source of danger with the possibility of incurring damage/injury, loss or misfortune. When using the Risk Event type, it is important to indicate what is at risk. This is accomplished using the event:has_topic property to define the possible event (such as a risk of cholera/an InfectiousHumanDisease or a risk of conflict/a DisagreementOrDispute)."@en ;
    rdfs:subClassOf :Factor .

:RoadBlocked a owl:Class ;
    rdfs:label "Road blocked"@en ;
    rdfs:comment "A road rendered impassable due to obstructions."@en ;
    rdfs:subClassOf :BlockadeOrRestrictionOfMovement, :EnvironmentalFactor .

:RoadsideBombing a owl:Class ;
    rdfs:label "Roadside bombing"@en ;
    rdfs:comment "A sub-class of Bombing describing that an explosive device was placed in or alongside of a road and detonated when a target approached."@en ;
    rdfs:subClassOf :Bombing .
#   owl:equivalentClass oeevent:Carry_out_roadside_bombing .

:RuralDevelopment a owl:Class ;
    rdfs:label "Rural development"@en ;
    rdfs:comment "RuralDevelopment programs (event:Operations) and activities have the goal of improving the quality of life, economic well-being, and social and economic development of rural communities, which are often isolated and have low population densities. For example, the USDA Office of Rural Development administers loans, offers technical assistance and information, and helps individuals in rural communities to buy, rent or repair housing."@en ;
    rdfs:subClassOf :EconomicDevelopment .

:Sabotage a owl:Class ;
    rdfs:label "Sabotage"@en ;
    rdfs:comment "Sabotage is any act intended to destroy, damage or disrupt equipment."@en ;
    rdfs:subClassOf :DamageOrDestruction .

:Sadness a owl:Class ;
    rdfs:label "Sadness"@en ;
    rdfs:comment "Sadness is an EmotionalResponse where an Actor is sorrowful or unhappy in general, or regarding a situation. To identify the situation, the event:has_topic property is used. The Actor who is sad is identified using the event:has_active_actor property."@en ;
    rdfs:subClassOf :EmotionalResponse .
#   owl:equivalentClass oeceo:Sadness .

:Sanctions a owl:Class ;
    rdfs:label "Sanctions"@en ;
    rdfs:comment "Deals with the restriction of movement (i.e., a sanction) of items or people. Per JP1-02, sanctions concern the 'control the movement of certain types of designated items [or Actors] into or out of a nation or specified area.'"@en ;
    rdfs:subClassOf :ReductionRestrictionOrRemoval .

:SanitaryConditions a owl:Class ;
    rdfs:label "Sanitary conditions"@en ;
    rdfs:comment "SanitaryConditions are a sub-class of LivingCondition indicating that an environment/location is safe and free from elements that 'may transmit, generate or promote disease, injury or sickness to any person'(https://www.allencountyhealth.com/get-informed/environmental-health-hazards/healthy-homes-2/unsanitary-conditions/)"@en ;
    owl:disjointWith :UnsanitaryConditions ;
    rdfs:subClassOf :LivingCondition .

:Savings a owl:Class ;
    rdfs:label "Savings"@en ;
    rdfs:comment "An EconomicFactor providing data (typically, an individual meas:ReportedValue or meas:TimeSeries) on the monies saved/put aside by a GPE, for a population or in a region. The GPE/population/group whose savings are reported is identified using the event:has_actor property, while the region is defined using general:located_at."@en ;
    rdfs:subClassOf :EconomicFactor .

:SearchAndRescue a owl:Class ;
    rdfs:label "Search and rescue operation"@en ;
    rdfs:comment "An Operation occurs over time, has specific goals, and is composed of specific, coordinated acts/Events intended to achieve those goals. The component Events (if known) are associated using the general:has_member property. The goal is identified using the actor:has_objective property."@en ;
    rdfs:comment "From JP1-02, search and rescue deals with 'the use of aircraft, surface craft, submarines, and specialized rescue teams and equipment to search for and rescue distressed persons on land or at sea in a permissive environment'."@en ;
    rdfs:subClassOf :Operation, :RecoveryOrRescue, :Investigation .

:Secrecy a owl:Class ;
    rdfs:label "Secrecy"@en ;
    rdfs:comment "Secrecy is obfuscation, and lack of accountability and openness regarding activities and conditions. Note that the class may be used to describe a specific Event (such as hiding a transfer of funds). Hence, it is defined as a sub-class of event:EventOrFactor."@en ;
    owl:disjointWith :Transparency ;
    rdfs:subClassOf :EventOrFactor .

:SeparationOrDivorce a owl:Class ;
    rdfs:label "Separation or divorce"@en ;
    rdfs:comment "The legal dissolution/ending of a marriage, cohabitation or formal relationship. This may occur due to mutual agreement or be ordered by some authority. The Actors who are separated/divorced are defined as active actors."@en ;
    rdfs:subClassOf :PersonalLifeEvent, :LegalEvent .

:SettlementOfDisagreementOrDispute a owl:Class ;
    rdfs:label "Settlement of disagreement or dispute"@en ;
    rdfs:comment "The ending/resolution of a disagreement or dispute. The Actors who reach the settlement are defined as active actors, while the disagreement/dispute is referenced using event:has_topic."@en ; 
    rdfs:subClassOf :AgreementOrPromise .

:SexualAssault a owl:Class ;
    rdfs:label "Sexual assault"@en ;
    rdfs:comment "A type of PhysicalAssault 'in which a person intentionally sexually touches another person without that person's consent, or coerces or physically forces a person to engage in a sexual act against their will. It is a form of sexual violence which includes rape ..., groping, child sexual abuse or the torture of the person in a sexual manner.' (https://en.wikipedia.org/wiki/Sexual_assault)"@en ;
    rdfs:subClassOf :PhysicalAssault .

:Shame a owl:Class ;
    rdfs:label "Shame"@en ;
    rdfs:comment "Shame is an EmotionalResponse where an Actor feels humiliation or distress over some behavior or situation. The Actor who feels shame is identified using the event:has_active_actor property. If the shame is related to some situation/behavior, that is associated using the event:has_topic property."@en ;
    rdfs:subClassOf :EmotionalResponse .
#   owl:equivalentClass oeceo:Shame .

:SharingOfInformation a owl:Class ;
    rdfs:label "Sharing of information"@en ;
    rdfs:comment "SharingOfInformation may describe either a specific event where two actors share information/intelligence to achieve a goal, or a general environment of sharing. A specific Event is defined by also classifying the individual as a type of event:InformationHandling, while a general/condition is also classified as an event:Factor. A goal of the sharing may be defined using the actor:has_objective property. The Actors that are sharing information/intelligence are identified using the event:has_active_actor property."@en ;
    rdfs:subClassOf :Cooperation .
#   owl:equivalentClass oeevent:Share_intelligence_or_information .

:Shortage a owl:Class ;
    rdfs:label "Shortage/inadequate supply"@en ;
    rdfs:comment "There can be shortages of things/artifacts (such as a shortage of food, water or schools), shortages of services/people in certain roles (such as a shortage of police or teachers), or shortages related to different Factors (such as a shortage of goodwill). The details of the first (shortages of things) are described by a Shortage individual that references the thing/artifact (for example, food in general or a particular type of food such as potatoes, fuel, water, etc.) using the general:involves_goods_or_property object property. The details of the second (shortages of people in roles) are described by a Shortage individual that references a GroupOfPersons using the event:has_actor property with their role defined using the general:position_or_role property. The details of the third (shortages of Factors) are described by a Shortage event that references the Factor using the event:has_topic property."@en ;
    rdfs:subClassOf :Factor .

:ShowOrExhibit a owl:Class ;
    rdfs:label "Show or exhibit"@en ;
    rdfs:comment "Examples of ShowOrExhibit are the screening of a movie or an art exhibit. If the event is related to the arts or an exhibit at a museum, etc., the ArtsAndCulture class should also be used."@en ;
    rdfs:subClassOf :EntertainmentEvent .

:SnowSleetAndWinterConditions a owl:Class ;
    rdfs:label "Snow, sleet and winter conditions"@en ;
    rdfs:comment "A WeatherIssue providing data (typically, an individual meas:ReportedValue or meas:TimeSeries) on the temperatures, or amount of snow or sleet in a GPE or region. Or, the class can be used simply to describe wintery conditions. The Location is identified using the general:located_at property."@en ;
    rdfs:subClassOf :WeatherIssue .

:SocialCondition a owl:Class ;
    rdfs:label "Social condition"@en ;
    rdfs:comment "SocialCondition involves any 'existing circumstance, situation or state affecting the life, welfare and relations of human beings in [a location or] community' (https://www.eionet.europa.eu/gemet/en/concept/7784). Sub-classes of SocialCondition include event:LivingCondition, event:SystemicDiscrimination and event:SystemicExploitation."@en ;
    rdfs:subClassOf :Factor .

:SocialServices a owl:Class ;
    rdfs:label "Social services"@en ;
    rdfs:comment "Social services are broadly defined as aiding individuals and families, enabling access to education/training, health care, housing, food/water, emergency services (such as law enforcement), etc."@en ;
    rdfs:subClassOf :Factor .

:SolarFlare a owl:Class ;
    rdfs:label "Solar flare"@en ;
    rdfs:comment "SolarFlares are a release of radiation from the sun caused by the interaction of magnetic field lines near sunspots. They can disrupt the upper atmosphere and signal transmissions, or induce electric fluctuations blowing out transformers and affecting electronics."@en ;
    rdfs:subClassOf :SpaceEvent .

:SpaceEvent a owl:Class ;
    rdfs:label "Space event"@en ;
    rdfs:comment "Space events include comet, asteroid or meteoroid impacts, meteor showers, burn-up of space debris in the atmosphere, airbursts related to an object's entry into the atmosphere, etc. Also included are events such as solar flares, eclipses, etc."@en ;
    rdfs:subClassOf :Event .

:SpaceSituationalAwareness a owl:Class ;
    rdfs:label "Space situational awareness (SSA)"@en ;
    rdfs:comment "From JP1-02, SSA is 'the requisite foundational, current, and predictive knowledge and characterization of space objects and the operational environment upon which space operations depend'."@en ;
    rdfs:subClassOf :AwarenessOrUnderstanding .

:Spending a owl:Class ;
    rdfs:label "Spending"@en ;
    rdfs:comment "An EconomicFactor providing data (typically, an individual meas:ReportedValue or meas:TimeSeries) on spending by a particular Actor, for a population or in a region. The Actor/population/group whose spending is reported is identified using the event:has_actor property, while the region is defined using general:located_at. The class may also be used to describe changes in spending (in which case, an individual is also typed as an event:Increase/Decrease/Stasis). Instances of type, Spending, may deal with specific artifacts that can be identified using the general:involves_goods_or_property predicate."@en ;
    rdfs:subClassOf :EconomicFactor .

:SponsorOrHost a owl:Class ;
    rdfs:label "Sponsor or host"@en ;
    rdfs:comment "SponsorOrHost involves any act of assuming responsibility for, or providing leadership, resources and/or facilities for a function or event. The function/event is identified using the event:has_topic property."@en ;
    rdfs:subClassOf :Event .

:Starvation a owl:Class ;
    rdfs:label "Starvation"@en ;
    rdfs:comment "Starvation describes either an individual event where someone or something is suffering from extreme hunger for a prolonged period, a general condition in a population or region, or statistics related to famine/starvation. It is a type of event:FoodInsecurity. When describing a change in the conditions in a population or region, an individual should also be classified using event:Increase/Decrease/Stasis. When providing statistics, an individual should also be classified using meas:ReportedValue or meas:TimeSeries."@en ;
    rdfs:subClassOf :FoodInsecurity .

:Stasis a owl:Class ;
    rdfs:label "Stasis"@en ;
    rdfs:comment "The class, Stasis, is used to record no difference/change in the availability/amount of a thing/artifact (such as no change in the amount of food, water or schooling), no difference/change in the number of people in certain roles (such as no change in the number of police or teachers), or no change related to 'general' Events (such as no change in the number of MurderOrHomicide occurrences in a specific location) or Factors (such as no change in the Anger level in a community). If the stasis is related to another Event/Factor, the Stasis individual uses the event:has_topic property to reference that other Event. To identify a stasis in the availability/amount of something, the Stasis individual is related to the artifact using general:involves_goods_or_property. To identify a stasis in the number of people in certain roles, those people are defined as an individual that is a GroupOfPersons with a general:position_or_role property, and that entity is related to Stasis via event:has_actor."@en ;
    rdfs:subClassOf :Factor .

:StateOfEmergencyOrMartialLaw a owl:Class ;
    rdfs:label "State of emergency or martial law"@en ;
    rdfs:comment "A StateOfEmergencyOrMartialLaw is a 'situation in which a government is empowered to perform actions that it would normally not be permitted to do. A government can declare such a state during a disaster, civil unrest, or armed conflict. Such declarations alert citizens to change their normal behavior and orders government agencies to implement emergency plans.' (https://en.wikipedia.org/wiki/State_of_emergency) Martial law is a more severe form of emergency with military control of the functioning of a community/region."@en ;
    rdfs:subClassOf :AlertStatus .
#   owl:equivalentClass oeevent:Impose_state_of_emergency_or_martial_law .

:Stoning a owl:Class ;
    rdfs:label "Stoning"@en ;
    rdfs:comment "Stoning is the act of throwing stones as a form of punishment. It may lead to death."@en ;
    rdfs:subClassOf :PhysicalAssault .

:Storm a owl:Class ;
    rdfs:label "Storm"@en ;
    rdfs:comment "A WeatherIssue providing details related to a specific event, changes in the frequency of storms (event:Increase/Decrease/Stasis) or statistics (typically, an individual meas:ReportedValue or meas:TimeSeries) on the temperatures, winds and/or amount of lightening strikes or rain related to a single storm or over a period of time. The Location of a Storm or Locations included in statistics are identified using the general:located_at property."@en ;
    rdfs:subClassOf :WeatherIssue . 

:Strike a owl:Class ;
    rdfs:label "Strike"@en ;
    rdfs:comment "Strikes are a group's refusal to work in protest against conditions, wages or other grievances. Note that this class is distinct from a military strike which should be classified as an event:Attack with an active actor that is classified as a MilitaryForce."@en ;
    rdfs:subClassOf :Event .

:StructuralDamage a owl:Class ;
    rdfs:label "Structural damage"@en ;
    rdfs:comment "The type, StructuralDamage, describes an on-going condition in the environment. This is distinct from the Event, DamageOrDestruction, which identifies events that result in complete or partial loss in value of goods or property. The thing that is destroyed is indicated using the general:involves_goods_or_property predicate."@en ;
    rdfs:subClassOf :Factor .

:Subversion a owl:Class ;
    rdfs:label "Subversion"@en ;
    rdfs:comment "Subversion covers a broad range of activities that are intended to decrease or destroying someone's (or some group's) honesty or loyalty, to undermine their moral integrity, or to overthrow or destroy a government. From JP1-02, Subversion is related to 'actions designed to undermine the military, economic, psychological, or political strength or morale of a governing authority'."@en ;
    rdfs:subClassOf :Event .

:Suicide a owl:Class ;
    rdfs:label "Suicide"@en ;
    rdfs:comment "Suicide is the act of taking one's own life. Not all suicides result in death. Hence, this class is about the act of suicide and not its result. It does not sub-class from event:Death, although that semantic could be added as an additional classification. To describe an unsuccessful attempt at suicide, the individual Event should also be classified using event:Attempt."@en ;
    rdfs:subClassOf :PersonalLifeEvent .
#   owl:equivalentClass cco:ActOfSuicide .

:SuicideBombing a owl:Class ;
    rdfs:label "Suicide bombing"@en ;
    rdfs:comment "Any bombing event in which the attacker intends to kill themselves in order to cause harm to or damage/destroy a target."@en ;
    rdfs:subClassOf :Bombing, :Suicide .
#   owl:equivalentClass oeevent:Carry_out_suicide_bombing .

:SurrenderOrYielding a owl:Class ;
    rdfs:label "Surrender or yielding"@en ;
    rdfs:comment "SurrenderOrYielding is a FormalAgreement in which one Actor admits defeat and/or agrees to give up fighting or to relinquish power, possession or control of something to another."@en ;
    rdfs:subClassOf :FormalAgreement .
#   owl:equivalentClass oeevent:Yield .

:Suspicion a owl:Class ;
    rdfs:label "Suspicion (deprecated)"@en ;
    owl:deprecated "true"^^xsd:boolean ;
    rdfs:comment "Suspicion is an EmotionalResponse where an Actor has misgivings about someone or something. The Actor who is distrustful/suspicious is identified using the event:has_active_actor property. When the distrust/suspicion is directed toward another Actor, that individual is identified using event:has_affected_actor. If the distrust/suspicion is directed toward a thing (such as doubting a car's brakes/braking ability), the artifact is identified using general:involves_goods_or_property."@en ;
    rdfs:comment "Note that Suspicion has been deprecated in lieu of using its super-class, DistrustOrSuspicion."@en ;
    rdfs:subClassOf :DistrustOrSuspicion .

:SymbolicAct a owl:Class ;
    rdfs:label "Symbolic act"@en ;
    rdfs:comment "An act imbued with deeper meaning or significance that represents a principle or abstract idea. Examples of symbolic acts are hunger strikes to protest abuse or mistreatment in prisons, or lighting of candles in tribute/thanks."@en ;
    rdfs:subClassOf :Event .
#   owl:equivalentClass oeevent:Engage_in_symbolic_act .

:SystemicDiscrimination a owl:Class ;
    rdfs:label "Systemic discrimination"@en ;
    rdfs:comment "Specific acts or general conditions/patterns of behavior/policies/practices that 'create or perpetuate disadvantage for ... persons' (https://definitions.uslegal.com/s/systemic-discrimination/). Increase/decrease or statistics related to discrimination should also be classified using event:Increase/Decrease/Stasis, meas:ReportedValue or meas:TimeSeries."@en ;
    rdfs:subClassOf :SocialCondition .

:SystemicExploitation a owl:Class ;
    rdfs:label "Systemic exploitation"@en ;
    rdfs:comment "Specific acts or general conditions/patterns of behavior/policies/practices that treat a person or populace unfairly, or use/manipulate them to another's advantage. Increase/decrease or statistics related to exploitation should also be classified using event:Increase/Decrease/Stasis, meas:ReportedValue or meas:TimeSeries."@en ;
    rdfs:subClassOf :SocialCondition .

:TariffOrTradeSanctions a owl:Class ;
    rdfs:label "Tariff or trade sanctions"@en ;
    rdfs:comment "TariffOrTradeSanctions place a tax or restriction on import/exports in order to express disapproval or displeasure, or give advantage to a local industry/set of workers. The goods which are sanctioned or tariffed are identified using general:involves_goods_or_property."@en ;
    rdfs:subClassOf :EconomicSanctions .

:Taxation a owl:Class ;
    rdfs:label "Taxation"@en ;
    rdfs:comment "Activities related to the imposition and collection of monies from an individual or organization, by a government to fund its operation, programs, etc. Examples of taxes include income, property and sales taxes."@en ;
    rdfs:subClassOf :PoliticalFactor, :EconomicFactor .

:TensionOrStress a owl:Class ;
    rdfs:label "Tension or stress"@en ;
    rdfs:comment "TensionOrStress is an EmotionalResponse where an Actor is experiencing strain. The Actor who is tense/stressed is identified using the event:has_active_actor property. If the tension/stress is between/directed toward another Actor, that individual is identified using the event:has_affected_actor property."@en ;
    rdfs:subClassOf :EmotionalResponse .

:Terrorism a owl:Class ;
    rdfs:label "Terrorism"@en ;
    rdfs:comment "Activities related to 'the unlawful use of violence or threat of violence, often motivated by religious, political, or other ideological beliefs, to instill fear and coerce governments or societies in pursuit of goals that are usually political' (from JP1-02)."@en ;
    rdfs:subClassOf :IntimidationAndCoercion, :Violence .
#   owl:equivalentClass cco:ActOfTerrorism .

:Testifying a owl:Class ;
    rdfs:label "Testifying"@en ;
    rdfs:comment "Testifying is a DeclarativeCommunication related to providing evidence about something or someone. This is mainly used in legal/court settings. When using the Testifying Event type, it is important to indicate who/what is being discussed in the testimony. This is accomplished using the event:has_affected_actor and event:has_topic object properties."@en ;
    rdfs:subClassOf :DeclarativeCommunication .
#   owl:equivalentClass cco:ActOfTestifying .

:Thanking a owl:Class ;
    rdfs:label "Thanking, conveying gratitude"@en ;
    rdfs:comment "Thanking is a Communication conveying gratitude or appreciation for some act. The act/event is denoted using the event:has_topic property."@en ;
    rdfs:subClassOf :CommunicationConveyingEmotion .
#   owl:equivalentClass cco:ActOfThanking .

:TheftOfAid a owl:Class ;
    rdfs:label "Theft of aid"@en ;
    rdfs:comment "TheftOfAid is any type of taking/stealing of aid-related resources. The resouce(s) that are stolen can be moneties or goods. The affected actor is the one from whom the  aid is taken."@en ;
    rdfs:subClassOf :TheftOrRobbery .

:TheftOrRobbery a owl:Class ;
    rdfs:label "Theft or robbery"@en ;
    rdfs:comment "TheftOrRobbery is any type of taking/stealing of something unlawfully. The thing(s) that are taken can be moneties, goods or even Persons. The affected actor is the one from whom the  aid is taken."@en ;
    rdfs:subClassOf :Event .

:Threatening a owl:Class ;
    rdfs:label "Threatening"@en ;
    rdfs:comment "Threatening is any Communication that menaces or frightens another by expressing the intent to take action in retribution for something done or not done. The action that is threatened is defined using event:has_topic with a tense of 'Future'. The thing that is done/not done is specified using event:has_topic with a tense of 'Past'. The Actor that is threatened is the affected actor."@en ;
    rdfs:subClassOf :Communication .
#   owl:equivalentClass oeevent:Threaten .

:ThreateningNonForce a owl:Class ;
    rdfs:label "Threatening non-force"@en ;
    rdfs:comment "ThreateningNonForce is any Communication that menaces or frightens another by expressing the intent to take action in retribution for something done or not done. The action that is threatened is not violent or physical, and is defined using event:has_topic with a tense of 'Future'. The thing that is done/not done is specified using event:has_topic with a tense of 'Past'. The Actor that is threatened is the affected actor."@en ;
    rdfs:subClassOf :Threatening .
#   owl:equivalentClass oeevent:Threaten_non-force .

:Tornado a owl:Class ;
    rdfs:label "Tornado"@en ;
    rdfs:comment "A sub-class of Storm, HighWind and NaturalDisaster providing details related to a specific event, changes in the frequency of tornadoes (event:Increase/Decrease/Stasis) or statistics (typically, an individual meas:ReportedValue or meas:TimeSeries) related to a single tornado or over a period of time. The Location of a Tornado or Locations included in statistics are identified using the general:located_at property."@en ;
    rdfs:subClassOf :Storm, :HighWind, :NaturalDisaster .

:Torture a owl:Class ;
    rdfs:label "Torture"@en ;
    rdfs:comment "Torture is any act deliberately intended to inflict physical or mental suffering in order to force another Person to provide information, to make a confession or for other reasons."@en ;
    rdfs:subClassOf :Violence .
#   owl:equivalentClass oeevent:Torture .

:Tourism a owl:Class ;
    rdfs:label "Tourism"@en ;
    rdfs:comment "Activities and conditions that promote/prohibit travel for business or pleasure, by peoples within and external to a Geopolitical Entity."@en ;
    rdfs:subClassOf :EconomicFactor .

:TradeBalance a owl:Class ;
    rdfs:label "Trade balance"@en ;
    rdfs:comment "TradeBalance is a sub-class of ImportAndExport since it is the net sum of a country’s exports and imports of goods (without taking other financial elements into account). It deals with the general condition of trade balance increase/decrease (event:Increase/Decrease/Stasis), or various statistics (an individual meas:ReportedValue or meas:TimeSeries) related to a GPE's trade balance."@en ;
    rdfs:subClassOf :ImportAndExport .

:Transaction a owl:Class ;
    rdfs:label "Transaction"@en ;
    rdfs:comment "Deals with any type of agreement or deal that involves exchanging/transferring monies, leadership, ownership, or all of the above. The transfer may be amicable or forced, seamless or not. This class is used when the details of the exchange/transfer are unknown."@en ;
    rdfs:subClassOf :Event ;
    owl:equivalentClass [ a owl:Class ;
                          owl:unionOf ( :TransferOfFunds :TransferOfLeadership :TransferOfOwnership ) ] .

:TransferOfFunds a owl:Class ;
    rdfs:label "Transfer of funds"@en ;
    rdfs:comment "A TransferOfFunds is not a Purchasing Event, but reflects a movement of funds by the active actor. For example, if a person moves monies from one account to another, that is a TransferOfFunds. If the funds are given to another Actor, then that entity is defined as the affected actor."@en ;
    rdfs:subClassOf :FinancialEvent .

:TransferOfLeadership a owl:Class ;
    rdfs:label "Transfer of leadership"@en ;
    rdfs:comment "TransferOfLeadership is any change/turnover of the head of a government, organization, etc. The transfer may be amicable or forced, seamless or not. Note that the Transfer is from the active Actor to the affected Actor."@en ;
    rdfs:subClassOf :Event .

:TransferOfLeadershipOrPolicyChange a owl:Class ;
    rdfs:label "Transfer of leadership or policy change"@en ;
    rdfs:comment "TransferOfLeadershipOrPolicyChange is defined as a mapping aid, based on the combining of the semantics of leadership and policy change in the CAMEO event codes."@en ;
    rdfs:subClassOf :Event ;
    owl:equivalentClass [ a owl:Class ;
                          owl:unionOf ( :TransferOfLeadership :PolicyChange ) ] .

:TransferOfOwnership a owl:Class ;
    rdfs:label "Transfer of ownership of some good or property"@en ;
    rdfs:comment "TransferOfOwnership is any ownership change. The transfer may be amicable or forced, seamless or not. Note that the Transfer is from the active Actor to the affected Actor."@en ;
    rdfs:subClassOf :Event .

:Transparency a owl:Class ;
    rdfs:label "Transparency"@en ; 
    rdfs:comment "Transparency is clarity, lack of obfuscation, accountability and openness regarding activities and conditions. Note that the class may be used to describe a specific Event (such as a divulging the source of funding for a project). Hence, it is defined as a sub-class of event:EventOrFactor."@en ;
    rdfs:subClassOf :EventOrFactor .

:TransportationOfPeopleOrCargo a owl:Class ;
    rdfs:label "Transportation of people, personnel or cargo"@en ; 
    rdfs:comment "Deals with any type of transportation event, when the details of what is transported are unknown. This class is the union of event:CargoTransportation and event:PersonalOrPassengerTransportation."@en ;
    rdfs:subClassOf :LocationChange ;
    owl:equivalentClass [ a owl:Class ;
                          owl:unionOf ( :CargoTransportation :PersonalOrPassengerTransportation ) ] .

:TrespassOrIncursion a owl:Class ;
    rdfs:label "Trespass or incursion"@en ; 
    rdfs:comment "Deals with any type of entry into an area or property without right or permission."@en ;
    general:noun_exemplar "The man was jailed for second degree criminal [[trespass]] following an incident on Tuesday morning."@en ;
    general:verb_exemplar "Troopers responded to the 700 block of Lower Cherry Valley Road, for a report of a squatter [[trespassing]] at a vacant residence."@en ;
    general:verb_exemplar "There had been 200 [[incursions]] into North Korea from the south."@en ;
    rdfs:subClassOf :LocationChange .

:TropicalStorm a owl:Class ;
    rdfs:label "Tropical or cyclonic storm"@en ;
    rdfs:comment "A TropicalStorm is 'a rapidly rotating storm system characterized by a low-pressure center, a closed low-level atmospheric circulation, strong winds, and a spiral arrangement of thunderstorms that produce heavy rain' (https://en.wikipedia.org/wiki/Tropical_cyclone). It is a sub-class of Storm, HighWind and NaturalDisaster providing details related to a specific event, changes in the frequency of storms (event:Increase/Decrease/Stasis) or statistics (typically, an individual meas:ReportedValue or meas:TimeSeries) related to a single storm or over a period of time. The Location of a TropicalStorm or Locations included in statistics are identified using the general:located_at property."@en ;
    rdfs:subClassOf :Storm, :HighWind, :NaturalDisaster .

:Trust a owl:Class ;
    rdfs:label "Trust"@en ;
    rdfs:comment "Trust is an EmotionalResponse where an Actor has confidence or believes in the ability/capabilities of someone or something. The Actor who is trustful is identified using the event:has_active_actor property. When the trust is directed toward another Actor, that individual is identified using event:has_affected_actor. If the trust is directed toward a thing (such as trusting that a lock on a door will hold), the artifact is identified using general:involves_goods_or_property."@en ;
    rdfs:subClassOf :EmotionalResponse .

:Tsunami a owl:Class ;
    rdfs:label "Tsunami"@en ;
    rdfs:comment "A type of NaturalDisaster defined by a sudden displacement event in the ocean that results in a series of destructive ocean waves."@en ;
    rdfs:subClassOf :NaturalDisaster .

:Ultimatum a owl:Class ;
    rdfs:label "Ultimatum"@en ;
    rdfs:comment "Ultimatum is 'a demand whose fulfillment is requested in a specified period of time and which is backed up by a threat ... in case of noncompliance ... An ultimatum is generally the final demand in a series of requests. As such, the time allotted is usually short, and the request is understood not to be open to further negotiation. The threat which backs up the ultimatum can vary depending on the demand in question and on ... other circumstances.  The word is used in diplomacy to signify the final terms submitted by one of the parties in negotiation for settlement of any subject of disagreement. It is accompanied by an intimation as to how refusal will be regarded.' (https://en.wikipedia.org/wiki/Ultimatum)"@en ;
    rdfs:subClassOf :Demand, :Threatening .
#   owl:equivalentClass oeevent:Give_ultimatum .

:UnsanitaryConditions a owl:Class ;
    rdfs:label "Unsanitary conditions (for example, open sewage)"@en ;
    rdfs:comment "UnsanitaryConditions are a sub-class of LivingCondition indicating that an environment/location is not safe and contains elements that 'may transmit, generate or promote disease, injury or sickness to any person'. ... Unsanitary conditions can include insect or rodent infestations, large amounts of animal or human waste, clutter throughout the living area, no operational utilities (heat, electricity or hot water) and/or extreme uncleanliness.' (https://www.allencountyhealth.com/get-informed/environmental-health-hazards/healthy-homes-2/unsanitary-conditions/)"@en ;
    rdfs:subClassOf :LivingCondition .

:UnstableStructure a owl:Class ;
    rdfs:label "Unstable structure such as a building or bridge"@en ;
    rdfs:comment "A structure may be 'unstable' due to damage, in which case, the StructuralDamage type should also be used for an individual, or may be unstable due to its design."@en ;
    rdfs:subClassOf :Factor .

:Vaccination a owl:Class ;
    rdfs:label "Vaccination"@en ;
    rdfs:comment "Vaccination may describe either a specific event, a general condition/factor of increased/decreased vaccinations by a set of people or in a region (event:Increase/Decrease/Stasis), or statistics (an individual meas:ReportedValue or meas: TimeSeries) describing vaccinations in a population/region."@en ;
    rdfs:subClassOf :HealthAndDisease .

:VaccinationProgram a owl:Class ;
    rdfs:label "Vaccination program"@en ;
    rdfs:comment "An Operation with the goal of distributing vaccines to a region or populace. An Operation occurs over time, has specific goals (for example, to eradicate measles), and is composed of specific, coordinated acts/Events intended to achieve those goals. The component Events (if known) are associated using the general:has_member property. The goal is identified using the actor:has_objective property."@en ;
    rdfs:subClassOf :Operation, :HealthAndDisease .

:Veto a owl:Class ;
    rdfs:label "Veto"@en ;
    rdfs:comment "Veto is a DeclarativeCommunication that blocks, refuses to approve/endorse or rejects a decision, proposal or future action. When using the Veto Event type, it is important to indicate who/what is vetoed. This is accomplished using the event:has_affected_actor or event:has_topic object properties."@en ;
    rdfs:subClassOf :RefusalOrRejection .
#   owl:equivalentClass oeevent:Veto .

:Visit a owl:Class ;
    rdfs:label "Visit"@en ;
    rdfs:comment "A Visit is the act of going to see a place or meeting with some person for a short time (in either a professional capacity or for personal reasons). The meeting usually has a specific purpose such as entertainment or sightseeing, to make a request, or to accomplish something. The Actor that is visiting is the active actor, while the one that is visited is the affected actor. The purpose of the visit can be defined using event:has_topic."@en ;
    rdfs:subClassOf :MeetingOrEncounter .
#   owl:equivalentClass oeevent:Make_a_visit .

:ViolationOfAgreement a owl:Class ;
    rdfs:label "Violation of agreement"@en ;
    rdfs:comment "ViolationOfAgreement is any act that disregards or goes against a previous agreement or any of its conditions. The previous agreement is defined using event:preceded_by."@en ;
    rdfs:subClassOf :Event .

:ViolationOfCeasefire a owl:Class ;
    rdfs:label "Violation of ceasefire (deprecated)"@en ;
    owl:deprecated "true"^^xsd:boolean ;
    rdfs:comment "ViolationOfCeasefire is any act that disregards or goes against a previous ceasefire agreement or any of its conditions. The previous agreement is defined using event:preceded_by. This class is deprecated in lieu of using its super-class, event:ViolationOfCeasefireOrTruce."@en ;
    rdfs:subClassOf :ViolationOfCeasefireOrTruce .
#   owl:equivalentClass oeevent:Violate_ceasefire .

:ViolationOfCeasefireOrTruce a owl:Class ;
    rdfs:label "Violation of ceasefire or truce"@en ;
    rdfs:comment "ViolationOfCeasefireOrTruce is any act that disregards or goes against a previous CeasefireOrTruce agreement or any of its conditions. The previous agreement is defined using event:preceded_by."@en ;
    rdfs:subClassOf :ViolationOfAgreement .

:ViolationOfTruce a owl:Class ;
    rdfs:label "Violation of truce (deprecated)"@en ;
    owl:deprecated "true"^^xsd:boolean ;
    rdfs:comment "ViolationOfTruce is any act that disregards or goes against a previous truce agreement or any of its conditions. The previous agreement is defined using event:preceded_by. This class is deprecated in lieu of using its super-class, event:ViolationOfCeasefireOrTruce."@en ;
    rdfs:subClassOf :ViolationOfCeasefireOrTruce .

:Violence a owl:Class ;
    rdfs:label "Violence"@en ;
    rdfs:comment "Any act of aggression an act of aggression that could result in injury and/or destruction."@en ;
    rdfs:subClassOf :Aggression .
#   owl:equivalentClass cco:ActOfViolence .

:VolcanicEruption a owl:Class ;
    rdfs:label "Volcanic eruption"@en ;
    rdfs:subClassOf :NaturalDisaster .

:Volunteering a owl:Class ;
    rdfs:label "Volunteering"@en ;
    rdfs:comment "Volunteering is the performance of (or commitment to perform) work or rendering of a service without pay."@en ;
    rdfs:subClassOf :AgreementOrPromise .
#   owl:equivalentClass cco:ActOfVolunteering .

:Voting a owl:Class ;
    rdfs:label "Voting"@en ;
    rdfs:comment "Voting is meant to address both voting for/against a candidate or on an issue. This is distinct from an Election, which is the process of choosing someone for a position (which may be a political office, but is not necessarily so - e.g., 'John was elected to be the jury foreman'). Although voting is a part of an election, it is defined to distinguish between an individual voting/going to vote, and (for example) Trump and Clinton running two ElectionCampaigns in the 2016 Presidential Election."@en ;
    rdfs:subClassOf :DefenseOrSupport .

:Wages a owl:Class ;
    rdfs:label "Wages"@en ;
    rdfs:comment "Wages define either an individual Actor's renumeration (usually of money) for labor or services (typically specified by contract and based on hourly or daily work, or piecework deliverables), the overall increase/decrease of wages in an area or for a populace, or statistics related to labor. Individuals representing these three semantics are also classified using meas:ReportedValue, meas:TimeSeries, or event:Increase/Decrease/Stasis. The Actor whose wages/statistics are reported is identified using event:has_actor. If the information is relevant to a location, that is defined using general:located_at."@en ;
    rdfs:subClassOf :EconomicFactor .

:War a owl:Class ;
    rdfs:label "War"@en ;
    rdfs:comment "A War is a sub-class of ArmedConflict where the involved Actors have officially declared a state-of-war/hostility towards each other."@en ;
    rdfs:subClassOf :ArmedConflict .

:WarCrime a owl:Class ;
    rdfs:label "War crime"@en ;
    rdfs:comment "A WarCrime is 'an act that constitutes a serious violation of the laws of war that gives rise to individual criminal responsibility. Examples of war crimes include intentionally killing civilians or prisoners, torturing, destroying civilian property, taking hostages, performing a perfidy, raping, using child soldiers, pillaging, declaring that no quarter will be given, and seriously violating the principles of distinction and proportionality, such as strategic bombing of civilian populations.' (https://en.wikipedia.org/wiki/War_crime) Note that WarCrimes can be charged in the case of paramilitary actions."@en ;
    rdfs:subClassOf :Event .

:Warning a owl:Class ;
    rdfs:label "Warning"@en ;
    rdfs:comment "Warning is a Communication informing of coming danger, harm or unpleasantness and may include advice on how to deal with it. When using the Warning Event type, it is important to indicate who/what is being warned. This is accomplished using the event:has_affected_actor and event:has_topic object properties."@en ;
    rdfs:subClassOf :DirectiveCommunication .
#   owl:equivalentClass cco:ActOfWarning .

:WasteManagement a owl:Class ;
    rdfs:label "Waste management/sanitation"@en ;
    rdfs:comment "WasteManagement deals with 'the collection, transportation, and disposal of garbage, sewage, and other waste products. Waste management encompasses management of all processes and resources for proper handling of waste materials, from maintenance of waste transport trucks and dumping facilities to compliance with health codes and environmental regulations.' (http://www.businessdictionary.com/definition/waste-management.html)"@en ;
    rdfs:subClassOf :EventOrFactor .

:WaterInsecurity a owl:Class ;
    rdfs:label "Water insecurity"@en ;
    rdfs:comment "Water insecurity is defined as the insufficient availability of, or insufficient access to, clean water to meet the needs of the population for consumption, sanitation, healthcare and the production of food and goods."@en ;
    rdfs:subClassOf :FoodWaterAndNutrition .

:WaterManagement a owl:Class ;
    rdfs:label "Water management"@en ;
    rdfs:comment "WaterManagement is 'the control and movement of water resources to minimize damage to life and property and to maximize efficient beneficial use. Good water management of dams and levees reduces the risk of harm due to flooding. Irrigation water management systems make the most efficient use of limited water supplies for agriculture. Drainage management involves water budgeting and analysis of surface and sub-surface drainage systems. Sometimes water management involves changing practices, such as groundwater withdrawal rates, or allocation of water to different purposes.' (https://www.nrcs.usda.gov/wps/portal/nrcs/main/national/water/manage/)"@en ;
    rdfs:subClassOf :FoodWaterAndNutrition, :LandUse .

:WaterSecurity a owl:Class ;
    rdfs:label "Water security"@en ;
    rdfs:comment "Water security is defined as a sufficient availability of, and access to, clean water to meet the needs of the population for consumption, sanitation, healthcare and the production of food and goods."@en ;
    rdfs:subClassOf :FoodWaterAndNutrition .

:WeatherIssue a owl:Class ;
    rdfs:label "Weather issue"@en ;
    rdfs:comment "Any environmental condition related to atmospheric conditions in an area. Weather includes temperature, wind, clouds/precipitation, etc. and their effects. Either specific events may be defined, or general conditions/statistics. Instance of the latter are also classified using event:Increase/Decrease/Stasis, meas:ReportedValue or meas:TimeSeries."@en ;
    rdfs:subClassOf :EnvironmentalFactor .

:Wedding a owl:Class ;
    rdfs:label "Wedding"@en ;
    rdfs:comment "The legal binding of two Actors in marriage, which is also usually a social event/ceremony. The Actors who are married are defined as active actors."@en ;
    rdfs:subClassOf :PersonalLifeEvent, :Ceremony, :LegalEvent .
#   owl:equivalentClass cco:Wedding .

:Wildfire a owl:Class ;
    rdfs:label "Wildfire"@en ;
    rdfs:comment "A Wildfire is a fire that spreads rapidly over woodland or brush and destroys a large area of land."@en ;
    rdfs:subClassOf :Fire, :NaturalDisaster .

:Withdrawal a owl:Class ;
    rdfs:label "Withdrawal"@en ;
    rdfs:comment "Withdrawal is a movement out/retraction of a previously held position or ceasing to participate in an activity. Note that specific sub-classes of Withdrawal are not defined (withdrawal of peacekeepers or aid agencies), since this can be specified by defining the active Actors' classification (such as actor:AidOrReliefOrganzation) or general:position_or_role property (e.g., 'https://en.wikipedia.org/wiki/Peacekeeping', 'https://en.wikipedia.org/wiki/Inspection', etc.). Note that the semantic of Withdrawal is a super-class for event:FinancialWithdrawal (the removal of money or capital from an account)."@en ;
    rdfs:subClassOf :ReductionRestrictionOrRemoval .

:Wounding a owl:Class ;
    rdfs:label "Wounding"@en ;
    rdfs:comment "Wounding is the act of causing physical harm or injury. This may be the result of military combat."@en ;
    rdfs:subClassOf :Injury .
